@prefix rdf: <http://www.w3.org/1999/02/22-rdf-syntax-ns#> .
@prefix dataid: <http://dataid.dbpedia.org/ns/core#> .
@prefix dcat: <http://www.w3.org/ns/dcat#> .
@prefix dct: <http://purl.org/dc/terms/> .
@prefix owl: <http://www.w3.org/2002/07/owl#> .
@prefix prov: <http://www.w3.org/ns/prov#> .
@prefix rdfs: <http://www.w3.org/2000/01/rdf-schema#> .
@prefix wsdl: <http://www.w3.org/ns/wsdl-rdf#> .
@prefix void: <http://rdfs.org/ns/void#> .
@prefix xml: <http://www.w3.org/XML/1998/namespace> .
@prefix xsd: <http://www.w3.org/2001/XMLSchema#> .
@prefix foaf: <http://xmlns.com/foaf/0.1/> . 
@prefix lvont: <http://lexvo.org/ontology#> .
@prefix msr: <http://purl.org/ms-rights#> .
@prefix vann: <http://purl.org/vocab/vann/> .
@prefix skos: <http://www.w3.org/2004/02/skos/core#> .
@prefix spdx: <http://spdx.org/rdf/terms/#> .
@prefix datacite: <http://purl.org/spar/datacite/> .
@prefix litre: <http://www.essepuntato.it/2010/06/literalreification/> .

@base <http://dataid.dbpedia.org/ns/core#> .

dataid:
    a owl:Ontology ;
    vann:preferredNamespaceUri "http://dataid.dbpedia.org/ns/core#" ;
    vann:preferredNamespacePrefix "dataid" ;
    owl:versionInfo "2.0" ; 
    dct:modified "2016-04-30" ;
    rdfs:comment "DBpedia Data ID is an ontology with the goal of extensively describing datasets via RDF files in a uniform way. Established vocabularies like DCAT, VoID, Prov-O are used for maximum compatibility."@en ;
    rdfs:label "DataID"@en ;
	dct:license <http://purl.org/NET/rdflicense/cc-by4.0> ;
	dct:creator <http://wiki.dbpedia.org/Association/Persons/Freudenberg> ;
    owl:imports dcat:, prov:, rdfs:, foaf:, void: , dct: .
    #owl:imports <http://www.w3.org/ns/dcat>, rdfs: , <http://www.w3.org/ns/prov-o-20130430> , foaf: ,void: , dct: .
    
<http://wiki.dbpedia.org/Association/Persons/Freudenberg>
        a                        dataid:Agent ;
        foaf:mbox                "freudenberg@informatik.uni-leipzig.de" ;
        foaf:name                "Markus Freudenberg" .
    
########### classes ###########
dataid:Agent
    a owl:Class ;
    rdfs:isDefinedBy <http://dataid.dbpedia.org/ns/core#> ;
    rdfs:comment "Any type of agent without a specific function."@en ;
    rdfs:label "Agent"@en ;
    rdfs:subClassOf prov:Agent, foaf:Agent, dct:Agent.
    
    
dataid:DataId
	a owl:Class ;
    rdfs:isDefinedBy <http://dataid.dbpedia.org/ns/core#> ;
    rdfs:label "DataId"@en ;
	rdfs:comment "A description of one or more datasets. Acts as a dcat:CatalogRecord / void:DatasetDescription."@en ;
	dct:description """DataID is a multi-layerd meta-data system, which, in its core, describes datasets and their different manifestations, 
		as well as relations to agents like persons or organisations, in regard to their rights and responsibilities. 
		Depending on context, type of data and use-case, this core ontology can be augmented by multiple existing extensions 
		(e.g. Linked Data, repository descriptions etc.). By describing datasets including content, authors, licenses and provenance via RDF,
		thereby making data accessible to others, is the basic idea of Linked Open Data and is your contribution to a universal data give and take.
		To create DataIDs alongside datasets is the best way of announcing a new dataset and its updates to a global community by placing 
		it in the LOD cloud. You can create your own DataID files for any type of data at http://dataid.dbpedia.org.
		Validating and delivering metadata files in a uniform way, as well as providing the ability to query for datasets, 
		are main objectives of the DBpedia/DataID project."""@en ;

	rdfs:subClassOf void:DatasetDescription, dcat:CatalogRecord, prov:Entity,
		[
	        a owl:Restriction ;
	        owl:allValuesFrom dataid:DataId ;
	        owl:onProperty dataid:nextVersion
	    ],[
	        a owl:Restriction ;
	        owl:allValuesFrom dataid:DataId ;
	        owl:onProperty dataid:previousVersion
	    ],[
	        a owl:Restriction ;
	        owl:allValuesFrom dataid:DataId ;
	        owl:onProperty dataid:latestVersion
	    ],[
	        a owl:Restriction ;
	        owl:allValuesFrom msr:License ;
	        owl:onProperty dct:license
	    ],[
	        a owl:Restriction ;
	        owl:allValuesFrom lvont:Language ;
	        owl:onProperty dct:language
	    ].	    

dataid:Dataset
    a owl:Class ;
    rdfs:isDefinedBy <http://dataid.dbpedia.org/ns/core#> ;
    rdfs:label "Dataset"@en ;
    rdfs:comment """A collection of data, available for access in one or more formats. Dataset resources describe the concept of the dataset, not it's manifestation (the data itself), which can be acquired as Distribution.
    Datasets are prov:Entities and can be generated by prov:Activities."""@en ;
    rdfs:subClassOf void:Dataset, dcat:Dataset, prov:Entity,
	    [
	        a owl:Restriction ;
	        owl:allValuesFrom dataid:Dataset ;
	        owl:onProperty dataid:nextVersion
	    ],[
	        a owl:Restriction ;
	        owl:allValuesFrom dataid:Dataset ;
	        owl:onProperty dataid:previousVersion
	    ],[
	        a owl:Restriction ;
	        owl:allValuesFrom dataid:Dataset ;
	        owl:onProperty dataid:latestVersion
	    ],[
	        a owl:Restriction ;
	        owl:allValuesFrom msr:License ;
	        owl:onProperty dct:license
	    ],[
	        a owl:Restriction ;
	        owl:allValuesFrom lvont:Language ;
	        owl:onProperty dct:language
	    ],[ 
			a owl:Restriction ;
			owl:onProperty void:subset ;
		 	owl:allValuesFrom dataid:Dataset
	 	],[
	        a owl:Restriction ;
	        owl:onProperty dcat:distribution ;
	        owl:allValuesFrom dataid:Distribution 
	    ].

dataid:Distribution
    a owl:Class ;
    rdfs:isDefinedBy <http://dataid.dbpedia.org/ns/core#> ;
    rdfs:comment "A way to access a dataset, like a dump file, an endpoint, an API etc."@en ;
    rdfs:label "Distribution"@en ;
    rdfs:subClassOf dcat:Distribution, prov:Entity,
    	[
	        a owl:Restriction ;
	        owl:allValuesFrom dataid:Distribution ;
	        owl:onProperty dataid:nextVersion
	    ],[
	        a owl:Restriction ;
	        owl:allValuesFrom dataid:Distribution ;
	        owl:onProperty dataid:previousVersion
	    ],[
	        a owl:Restriction ;
	        owl:allValuesFrom dataid:Distribution ;
	        owl:onProperty dataid:latestVersion
	    ],[
	        a owl:Restriction ;
	        owl:allValuesFrom msr:License ;
	        owl:onProperty dct:license
	    ],[
	        a owl:Restriction ;
	        owl:allValuesFrom lvont:Language ;
	        owl:onProperty dct:language
	    ],[
	        a owl:Restriction ;
	        owl:allValuesFrom spdx:Checksum ;
	        owl:onProperty dcat:checksum
	    ].

dataid:ServiceEndpoint
    a owl:Class ;
    rdfs:isDefinedBy <http://dataid.dbpedia.org/ns/core#> ;
    rdfs:comment "A specific distribution, which is accessible via an access url and provides data as a web service in a certain format."@en ;
    rdfs:label "Service Endpoint"@en ;
    rdfs:subClassOf dataid:Distribution, wsdl:Service.

dataid:SingleFile
    a owl:Class ;
    rdfs:isDefinedBy <http://dataid.dbpedia.org/ns/core#> ;
    rdfs:comment "A single data dump file representing your dataset."@en ;
    rdfs:label "single dump file"@en ;
    rdfs:subClassOf dataid:Distribution.

dataid:Directory
    a owl:Class ;
    rdfs:isDefinedBy <http://dataid.dbpedia.org/ns/core#> ;
    rdfs:comment "A dedicated directory holding multiple files of the same dataset."@en ;
    rdfs:label "dataset files in one directory"@en ;
    rdfs:subClassOf dataid:Distribution.

dataid:FileCollection
    a owl:Class ;
    rdfs:isDefinedBy <http://dataid.dbpedia.org/ns/core#> ;
    rdfs:comment "Multiple files of a distribution constituting one dataset."@en ;
    rdfs:label "dataset files in differnt paths of a distribution"@en ;
    rdfs:subClassOf dataid:Distribution.

dataid:Authorization
	a owl:Class ;
    rdfs:isDefinedBy <http://dataid.dbpedia.org/ns/core#> ;
    rdfs:label "Authorization"@en ;
	rdfs:comment """This concept defines a scope of Entities and links it to an Agent who has certain rights for those entities (defined by the AgentRole/AuthorizedAction). The scope consists of all Entities directly linked to the dataid:Authorization, as well as transitively dependent Entities."""@en ;
	rdfs:subClassOf prov:Attribution .

dataid:AgentRole
	a owl:Class ;
    rdfs:isDefinedBy <http://dataid.dbpedia.org/ns/core#> ;
    rdfs:label "Agent role"@en ;
	rdfs:comment """Instances of this class define an array of rights and responsibilities an agent, assigned with this role for a given scope of entities, has to address or can execute."""@en ;
	rdfs:subClassOf prov:Role.

dataid:AuthorizedAction
	a owl:Class ;
    rdfs:isDefinedBy <http://dataid.dbpedia.org/ns/core#> ;
    rdfs:label "Authorized action"@en ;
    rdfs:comment """AgentRoles provide agents with the ability to execute certain actions as well as demand certain responsibilities, which are defines by the instances of this concept."""@en .

dataid:ResponsibleAction
	a owl:Class ;
    rdfs:isDefinedBy <http://dataid.dbpedia.org/ns/core#> ;
    rdfs:label "responsible actions"@en ;
	rdfs:comment """AgentRoles provide access rights as well as responsibilities an agent has to attend to in order to fullfill this role. Responsible actions should describe actions pertaining to responsibilities an agent is supposed to do."""@en ;
	rdfs:subClassOf dataid:AuthorizedAction ;
	owl:disjointWith dataid:EntitledAction .

dataid:EntitledAction
	a owl:Class ;
    rdfs:isDefinedBy <http://dataid.dbpedia.org/ns/core#> ;
    rdfs:label "Entitled action"@en ;
	rdfs:comment """AgentRoles provide access and modification rights to an agent. Entitled actions should comprise actions pertaining to access/modification restrictions."""@en ;
	rdfs:subClassOf dataid:AuthorizedAction ;
	owl:disjointWith dataid:ResponsibleAction .

dataid:AccessLevel
	a owl:Class ;
	rdfs:isDefinedBy <http://dataid.dbpedia.org/ns/core#> ;
	rdfs:label "Access level"@en ;
	rdfs:comment "The level of openness of access to a particular groups of agents"@en ;
	owl:subClassOf [
		a owl:Class ;
		owl:oneOf (
			dataid:PrivateAccess
			dataid:SemiPrivateAccess
			dataid:PublicAccess
		)
	].
	
dataid:SimpleStatement
	a owl:Class;
	rdfs:isDefinedBy <http://dataid.dbpedia.org/ns/core#> ;
	rdfs:label "Simple Statement"@en ;
	rdfs:comment "Implements the Statement and Standard classes of Dublin Core, containing a textual statement and a reference pointer."@en ;
	rdfs:subClassOf dct:ProvenanceStatement, dct:RightsStatement, dct:Standard ,
	[
        a owl:Restriction ;
        owl:allValuesFrom foaf:Document ;
        owl:onProperty dct:references
    ].

dataid:Identifier
	a owl:Class ;
	rdfs:isDefinedBy <http://dataid.dbpedia.org/ns/core#> ;
	rdfs:label "identifier"@en ;
	rdfs:comment "Uniquly identifies any resource, given an identifier as literal and a correspondng aid/pid scheme (ORCID, ResearcherID etc.). "@en ;
	rdfs:subClassOf datacite:Identifier,
	[
		a owl:Restriction ;
		owl:maxQualifiedCardinality "1"^^xsd:nonNegativeInteger ;
		owl:onProperty litre:hasLiteralValue ;
		owl:onDatatype rdfs:Literal
    ] ,
	[
		a owl:Restriction ;
		owl:maxQualifiedCardinality "1"^^xsd:nonNegativeInteger ;
		owl:onProperty datacite:usesIdentifierScheme ;
		owl:onClass datacite:identifierScheme
    ] .
	    
dataid:MediaType
	a owl:Class;
	rdfs:isDefinedBy <http://dataid.dbpedia.org/ns/core#> ;
	rdfs:label "Iana Media Type"@en ;
	rdfs:comment "Extends the dct:MediaType class of Dublin Core by implementing the Iana media type description and adding a pointer to inner media types to deal with (multiple) compressions of a serialized file."@en ;
	rdfs:subClassOf dct:MediaType.
		
		
########## properties #########

dataid:isDistributionOf
	a	owl:ObjectProperty ;
	rdfs:isDefinedBy <http://dataid.dbpedia.org/ns/core#> ;
	rdfs:label "Is distribution of"@en ;
	rdfs:comment "Inverse property of dcat:distribution, linking a Distribution to a Dataset"@en ;
	owl:inverseOf	dcat:distribution;
	rdfs:domain		dataid:Distribution;
	rdfs:range		dataid:Dataset.

dataid:uncompressed  #will be faced out probably...
	a	owl:DatatypeProperty ;
	rdfs:subPropertyOf dcat:byteSize ;
	rdfs:isDefinedBy <http://dataid.dbpedia.org/ns/core#> ;
	rdfs:label "uncompressed"@en ;
	rdfs:comment "Records the byte size of the uncompressed version of this file."@en ;
	rdfs:domain		dataid:Distribution ;
    rdfs:range      xsd:integer.

dataid:isInheritable
	a	owl:DatatypeProperty ;
	rdfs:isDefinedBy <http://dataid.dbpedia.org/ns/core#> ;
	rdfs:label "is inheritable"@en ;
	rdfs:comment "The property of certain dataid:Authorization to be able to be inherited"@en ;
	rdfs:domain		dataid:Authorization ;
    rdfs:range      xsd:boolean.

dataid:similarData
    a owl:ObjectProperty ;
    rdfs:subPropertyOf dct:relation ;
    rdfs:isDefinedBy <http://dataid.dbpedia.org/ns/core#> ;
    rdfs:comment 	"Points to other dataset containing related data."@en ;
    rdfs:domain 	dataid:Dataset ;
    rdfs:label 		"similar data"@en ;
    rdfs:range  	dcat:Dataset .

dataid:preview
    a owl:ObjectProperty ;
    rdfs:isDefinedBy <http://dataid.dbpedia.org/ns/core#> ;
    rdfs:comment 	"Provides the uri of a short preview of the data provided by a distribution (do not link to the download or accessURL with this property)."@en ;
    rdfs:domain 	dataid:Distribution ;
    rdfs:label 		"data preview"@en ;
    rdfs:range  	foaf:Document .
    
dataid:associatedAgent
    a owl:ObjectProperty ;
    rdfs:subPropertyOf prov:wasAttributedTo ;
    rdfs:isDefinedBy <http://dataid.dbpedia.org/ns/core#> ;
    rdfs:comment "some agent generally connected to the dataset, their function to be specified by their rdf:type"@en ;
    rdfs:domain prov:Entity ;
    rdfs:label "associated agent"@en ;
    rdfs:range dataid:Agent ;
    owl:propertyChainAxiom (
	   dataid:underAuthorization
	   dataid:authorizedAgent
	) .

dataid:softwareRquirement
    a owl:ObjectProperty ;
    rdfs:isDefinedBy <http://dataid.dbpedia.org/ns/core#> ;
    rdfs:comment "software needed to access the data in this distribution"@en ;
    rdfs:domain dataid:Distribution ;
    rdfs:label "software requirement"@en ;
    rdfs:range foaf:Document .

dataid:accessProcedure
	a owl:DatatypeProperty ;
	rdfs:isDefinedBy <http://dataid.dbpedia.org/ns/core#> ;
	rdfs:comment "Describes the steps which have to be taken to gain access to the described data at the location of a distribution (e.g. register an account to gain dct:accessRights)."@en ;
    rdfs:domain dataid:Distribution ;
    rdfs:label "access procedure"@en ;
    rdfs:range rdfs:Literal .

dataid:nextVersion
    a owl:ObjectProperty ;
    rdfs:isDefinedBy <http://dataid.dbpedia.org/ns/core#> ;
    rdfs:comment "Next version of a DataIdPart"@en ;
    rdfs:domain prov:Entity ;
    rdfs:label "next version"@en ;
    rdfs:range prov:Entity .

dataid:previousVersion
    a owl:ObjectProperty ;
    rdfs:isDefinedBy <http://dataid.dbpedia.org/ns/core#> ;
    rdfs:comment "previous version of a DataIdPart"@en ;
    rdfs:domain prov:Entity ;
    rdfs:label "previous version"@en ;
    rdfs:range prov:Entity .

dataid:latestVersion
    a owl:ObjectProperty ;
    rdfs:isDefinedBy <http://dataid.dbpedia.org/ns/core#> ;
    rdfs:comment "Latest version of a DataIdPart"@en ;
    rdfs:domain prov:Entity ;
    rdfs:label "latest version"@en ;
    rdfs:range prov:Entity .

dataid:innerMediaType a owl:ObjectProperty, owl:FunctionalProperty ;
	rdfs:subPropertyOf dcat:mediaType;
	rdfs:isDefinedBy <http://dataid.dbpedia.org/ns/core#> ;
    rdfs:comment "Points out the MediaType of the (compressed) file inside this one."@en ;
    rdfs:domain dataid:MediaType ;
    rdfs:label "inner media type"@en ;
    rdfs:range dataid:MediaType .
    
dataid:typeTemplate
	a owl:DatatypeProperty, owl:FunctionalProperty ;
	rdfs:isDefinedBy <http://dataid.dbpedia.org/ns/core#> ;
	rdfs:comment "The template (or mime type string) of a media Type."@en ;
    rdfs:domain dataid:MediaType ;
    rdfs:label "media type template"@en ;
    rdfs:range rdfs:Literal .
    
dataid:typeReference
	a owl:ObjectProperty;
	rdfs:isDefinedBy <http://dataid.dbpedia.org/ns/core#> ;
	rdfs:comment "Refers to a standard associated with this mime type."@en ;
    rdfs:domain dataid:MediaType ;
    rdfs:label "media type reference"@en ;
    rdfs:range rdfs:Resource .
    
dataid:typeExtension
	a owl:DatatypeProperty;
	rdfs:isDefinedBy <http://dataid.dbpedia.org/ns/core#> ;
	rdfs:comment "Lists file extensions commonly used with this mime type."@en ;
    rdfs:domain dataid:MediaType ;
    rdfs:label "media type file extension"@en ;
    rdfs:range rdfs:Literal .
	    
dataid:typeName
	a owl:DatatypeProperty;
	rdfs:isDefinedBy <http://dataid.dbpedia.org/ns/core#> ;
	rdfs:comment "Names the media types described."@en ;
    rdfs:domain dataid:MediaType ;
    rdfs:label "media type name"@en ;
    rdfs:range rdfs:Literal .
    
dataid:statement
	a owl:DatatypeProperty ;
	rdfs:isDefinedBy <http://dataid.dbpedia.org/ns/core#> ;
    rdfs:comment 	"An actual textual statment"@en ;
    rdfs:label "statement"@en ;
    rdfs:domain dataid:SimpleStatement ;
    rdfs:range rdfs:Literal.

dataid:identifier
    a owl:InverseFunctionalProperty ;
    rdfs:subPropertyOf datacite:hasIdentifier, foaf:isPrimaryTopicOf ;
    rdfs:isDefinedBy <http://dataid.dbpedia.org/ns/core#> ;
    rdfs:comment "An unique identifier which was created by a SchemaAgency for an agent or entity."@en ;
    rdfs:label "(additional) identifier"@en ;
    rdfs:range dataid:Identifier .

dataid:identifierURL
    a owl:ObjectProperty ;
    rdfs:isDefinedBy <http://dataid.dbpedia.org/ns/core#> ;
    rdfs:comment 	"uri/url provided as, or in addition to an id"@en ;
    rdfs:domain 	dataid:Identifier ;
    rdfs:label 		"URL of a page pertaining to this identifier (usualy on a website of the SchemaAgency)."@en ;
    rdfs:range  	foaf:Document .

dataid:hasAccessLevel
    a owl:FunctionalProperty ;
    rdfs:isDefinedBy <http://dataid.dbpedia.org/ns/core#> ;
    rdfs:comment "defines the access rights for DataId related entities"@en ;
    rdfs:domain prov:Entity ;
    rdfs:label "access level"@en ;
    rdfs:range dataid:AccessLevel .

dataid:authorizedFor
	a owl:ObjectProperty ;
    owl:inverseOf  dataid:underAuthorization ;
    rdfs:isDefinedBy <http://dataid.dbpedia.org/ns/core#> ;
    rdfs:comment "Defines the scope of an dataid:Authorization. An Agent has the right to execute authorized actions in this scope (e.g. a single DataId and all it's datasets)."@en ;
    rdfs:label "authorized for"@en .

dataid:authorizedAgent
   	a owl:ObjectProperty ;
    rdfs:subPropertyOf prov:agent ;
   	rdfs:isDefinedBy <http://dataid.dbpedia.org/ns/core#> ;
    rdfs:comment "Points out the Agent the dataid:Authorization is defined for (e.g. to modify the metadata of a dataset)."@en ;
    rdfs:domain prov:AgentInfluence ;
    rdfs:label "authorized agent"@en ;
    rdfs:range dataid:Agent .

dataid:hasAuthorization
   	a owl:ObjectProperty ;
   	owl:inverseOf dataid:authorizedAgent ;
   	rdfs:isDefinedBy <http://dataid.dbpedia.org/ns/core#> ;
    rdfs:comment "Provides an dataid:Agent with the dataid:Authorization for a given scope of entities (e.g. Dataset, Distribution etc.), to execute certain actions."@en ;
    rdfs:label "has authorization"@en .
    
dataid:authorityAgentRole
   	a owl:ObjectProperty ;
    rdfs:subPropertyOf prov:hadRole ;
    rdfs:isDefinedBy <http://dataid.dbpedia.org/ns/core#> ;
    rdfs:comment "Adds a role an agent can administer in the scope provided by the Authorization, thereby allowing for certain actions an agent can execute."@en ;
    rdfs:domain prov:AgentInfluence ;
    rdfs:label "authority agent role"@en ;
    rdfs:range dataid:AgentRole .

dataid:validForAccessLevel
    a owl:ObjectProperty ;
    rdfs:isDefinedBy <http://dataid.dbpedia.org/ns/core#> ;
    rdfs:comment "Limits rights and actions an Agent is allowed to take depending on the AccessLevel chosen for this Authorization."@en ;
    rdfs:domain dataid:Authorization ;
    rdfs:label "valid for access level"@en ;
    rdfs:range dataid:AccessLevel .

dataid:allowsFor
   	a owl:ObjectProperty ;
    rdfs:isDefinedBy <http://dataid.dbpedia.org/ns/core#> ;
    rdfs:comment "AgentRoles allows an agent to execute certain actions."@en ;
    rdfs:domain dataid:AgentRole ;
    rdfs:label "allowes for"@en ;
    rdfs:range dataid:AuthorizedAction .

dataid:authorizedAction
   	a owl:ObjectProperty ;
    rdfs:isDefinedBy <http://dataid.dbpedia.org/ns/core#> ;
    rdfs:comment "Actions, agents are allowed to execute under a given Authorization, without regard to an AgentRole optionally specified in addition."@en ;
    rdfs:domain prov:AgentInfluence ;
    rdfs:label "authorized action"@en ;
    rdfs:range dataid:AuthorizedAction ;
    owl:propertyChainAxiom (
	   dataid:authorityAgentRole
	   dataid:allowsFor
	) .

dataid:underAuthorization
    a owl:ObjectProperty ;
    rdfs:subPropertyOf prov:qualifiedAttribution ;
    rdfs:isDefinedBy <http://dataid.dbpedia.org/ns/core#> ;
    rdfs:comment "Points out a dataid:Authorization with some degree of authority over this resource."@en ;
    rdfs:label "under an authorization of"@en ;
    rdfs:range dataid:Authorization .

dataid:validFrom
    a owl:DatatypeProperty, owl:FunctionalProperty ;
    rdfs:isDefinedBy <http://dataid.dbpedia.org/ns/core#> ;
    rdfs:comment 	"An Authorization is valid for a specific Agent from a certain point in time."@en ;
    rdfs:domain 	prov:AgentInfluence ;
    rdfs:label 		"valid from"@en ;
    rdfs:range  	xsd:dateTime .
    
dataid:validUntil
    a owl:DatatypeProperty, owl:FunctionalProperty ;
    rdfs:isDefinedBy <http://dataid.dbpedia.org/ns/core#> ;
    rdfs:comment 	"An Authorization is valid for a specific Agent until a certain point in time."@en ;
    rdfs:domain 	prov:AgentInfluence ;
    rdfs:label 		"valid until"@en ;
    rdfs:range  	xsd:dateTime .

dataid:isInheritable
    a owl:DatatypeProperty, owl:FunctionalProperty ;
    rdfs:isDefinedBy <http://dataid.dbpedia.org/ns/core#> ;
    rdfs:comment 	"Defines that a dataid:Authorization is also valid for the next version of a DataID (if set to 'true' - which should be the default)."@en ;
    rdfs:domain 	dataid:Authorization ;
    rdfs:label 		"is inheritable"@en ;
    rdfs:range  	xsd:boolean .


#The follwing properties are only inferred by the the existence of property paths of foaf:primaryTopc, void:subset and dcat:distribution.
dataid:authorityChain
	a	owl:ObjectProperty ;
	rdfs:isDefinedBy <http://dataid.dbpedia.org/ns/core#> ;
	rdfs:label "authority chain"@en ;
	rdfs:comment """This property (with its sub-properties) describes how an dataid:Authorization is spread to other entities (lower level entities, like Dataset & Distribution). 
		This inferred chain of authority can be overwritten by introducing other dataid:Authorization objects with the scope of lower level entities. See the example in Github for more information."""@en .
	
dataid:authoritySubChain1	
	a	owl:ObjectProperty ;
	rdfs:subPropertyOf dataid:authorityChain ;
	rdfs:isDefinedBy <http://dataid.dbpedia.org/ns/core#> ;
	rdfs:label "authority chain axiom with subset"@en ;
	rdfs:comment "Represents the authority link between the DataID and a Dataset (if connectd via a Subset)."@en ;
    owl:propertyChainAxiom (
	   foaf:primaryTopic	
	   dataid:transitiveSubset
	   dcat:distribution
	) .
	
dataid:authoritySubChain2	
	a	owl:ObjectProperty ;
	rdfs:subPropertyOf dataid:authorityChain ;
	rdfs:isDefinedBy <http://dataid.dbpedia.org/ns/core#> ;
	rdfs:label "authority chain axiom without subset"@en ;
	rdfs:comment "Represents the authority link between the DataID and a Dataset (if connectd without a Subset)."@en ;
    owl:propertyChainAxiom (
	   foaf:primaryTopic	
	   dcat:distribution
	) .
	
dataid:transitiveSubset	
	a	owl:ObjectProperty, owl:TransitiveProperty ;
	rdfs:isDefinedBy <http://dataid.dbpedia.org/ns/core#> ;
	rdfs:label "transitive super property of void:subset"@en ;
	rdfs:comment "Represents the authority link between two Datsets (if connectd by void:subset)."@en .	
	
void:subset rdfs:subPropertyOf dataid:transitiveSubset.
	
#status testing
#dataid:accessProtocol
#    a owl:DatatypeProperty, owl:FunctionalProperty ;
#    rdfs:isDefinedBy <http://dataid.dbpedia.org/ns/core#> ;
#    rdfs:comment 	"Defines the protocol used by the distribution provider (e.g. repository). By default dataid-hub assumes tcp."@en ;
#    rdfs:domain 	dataid:Distribution ;
#    rdfs:label 		"access protocol"@en ;
#    rdfs:range  	rdfs:Literal ;
#    owl:equivalentClass [
#    	a owl:Class ;
#    	owl:oneOf( "tcp" "udp" "dccp" "sctp" )
#    ].

################### Instances ####################
dataid:PrivateAccess
	a dataid:AccessLevel ;
	rdfs:isDefinedBy <http://dataid.dbpedia.org/ns/core#> ;
	rdfs:label "private"@en ;
	rdfs:comment "Provides an agent with unrestricted access and all rights of a resource."@en .

dataid:SemiPrivateAccess
	a dataid:AccessLevel ;
	rdfs:isDefinedBy <http://dataid.dbpedia.org/ns/core#> ;
	rdfs:label "semi-private"@en ;
	rdfs:comment "Limits the rights an agent has on a resource to read and modify."@en .

dataid:PublicAccess
	a dataid:AccessLevel ;
	rdfs:isDefinedBy <http://dataid.dbpedia.org/ns/core#> ;
	rdfs:label "public"@en;
	rdfs:comment "Limits the rights an agent has on a resource to read rights."@en .

dataid:ResponseToContact
	a dataid:ResponsibleAction ;
	rdfs:isDefinedBy <http://dataid.dbpedia.org/ns/core#> ;
	rdfs:comment "The responsibility to respond to contact attempts by external agents. A contact point for the entity."@en ;
	rdfs:label "response to contact attempt"@en .

dataid:ResponseToLifeCycleEvent
	a dataid:ResponsibleAction ;
	rdfs:isDefinedBy <http://dataid.dbpedia.org/ns/core#> ;
	rdfs:comment "The responsibility to manage changes and react to bugs and issues that are reported"@en ;
	rdfs:label "response to life-cycle event"@en .

dataid:PublishingDecision
	a dataid:ResponsibleAction ;
	rdfs:isDefinedBy <http://dataid.dbpedia.org/ns/core#> ;
	rdfs:comment "The responsibility decide if the entity should be published"@en ;
	rdfs:label "publishing decision"@en .

dataid:UpdateDataId
	a dataid:ResponsibleAction ;
	rdfs:isDefinedBy <http://dataid.dbpedia.org/ns/core#> ;
	rdfs:comment "The responsibility to update dataset metadata."@en ;
	rdfs:label "update DataId"@en .

dataid:AgentSupervision
	a dataid:ResponsibleAction ;
	rdfs:isDefinedBy <http://dataid.dbpedia.org/ns/core#> ;
	rdfs:comment "The responsibility to supervise other agents."@en ;
	rdfs:label "agent supervision"@en .

dataid:ReadDataId
	a dataid:EntitledAction;
	rdfs:isDefinedBy <http://dataid.dbpedia.org/ns/core#> ;
	rdfs:comment "Entitled action to read the DataID dataset metadata"@en ;
	rdfs:label "read DataID right"@en .

dataid:ReadContent
	a dataid:EntitledAction;
	rdfs:isDefinedBy <http://dataid.dbpedia.org/ns/core#> ;
	rdfs:comment "Entitled action to read the content of an entity."@en ;
	rdfs:label "read content right"@en .

dataid:ModifyContent
	a dataid:EntitledAction;
	rdfs:isDefinedBy <http://dataid.dbpedia.org/ns/core#> ;
	rdfs:comment "Entitled action to modify the content of an entity."@en ;
	rdfs:label "modify content right"@en .

dataid:DeleteContent
	a dataid:EntitledAction;
	rdfs:isDefinedBy <http://dataid.dbpedia.org/ns/core#> ;
	rdfs:comment "Entitled action to delete some content of an entity."@en ;
	rdfs:label "delete content right"@en .

dataid:ModifyAuthorizedAgents
	a dataid:EntitledAction ;
	rdfs:comment "Entitled action to modify which agents are authorized on certain entities."@en ;
	rdfs:isDefinedBy <http://dataid.dbpedia.org/ns/core#> ;
	rdfs:label "modify authorized agents"@en .

dataid:ModifyAccessLevel
	a dataid:EntitledAction ;
	rdfs:comment "Entitled action to modify access level of an entity."@en ;
	rdfs:isDefinedBy <http://dataid.dbpedia.org/ns/core#> ;
	rdfs:label "modify entity access level"@en .

dataid:ModifyAgentRoles
	a dataid:EntitledAction ;
	rdfs:comment "Entitled action to modify the role of agents on certain entities."@en ;
	rdfs:isDefinedBy <http://dataid.dbpedia.org/ns/core#> ;
	rdfs:label "modify agent roles"@en .

dataid:Guest
	a dataid:AgentRole;
	dataid:allowsFor dataid:ReadDataId;
	dataid:allowsFor dataid:ReadContent;
	rdfs:isDefinedBy <http://dataid.dbpedia.org/ns/core#> ;
    rdfs:comment "A visitor/anonymous agent has only read rights on public and semi-private documents"@en ;
	rdfs:label "guest"@en .

dataid:Creator
	a dataid:AgentRole;
	rdfs:isDefinedBy <http://dataid.dbpedia.org/ns/core#> ;
	dataid:allowsFor dataid:ReadDataId;
	dataid:allowsFor dataid:UpdateDataId;
	dataid:allowsFor dataid:ModifyContent;
	dataid:allowsFor dataid:DeleteContent;
	dataid:allowsFor dataid:ReadContent;
	dataid:allowsFor dataid:ModifyAuthorizedAgents;
	dataid:allowsFor dataid:ResponseToLifeCycleEvent;
	dataid:allowsFor dataid:ResponseToContact;
	dataid:allowsFor dataid:AgentSupervision;
	dataid:allowsFor dataid:PublishingDecision;
	dataid:allowsFor dataid:ModifyAccessLevel;
	dataid:allowsFor dataid:ModifyAgentRoles;
    rdfs:comment "Creator of the resource. An agent that is credited with a main part in the initial creation of the resource."@en ;
	rdfs:label "creator"@en .

dataid:Maintainer
	a dataid:AgentRole;
	rdfs:isDefinedBy <http://dataid.dbpedia.org/ns/core#> ;
	dataid:allowsFor dataid:ReadDataId;
	dataid:allowsFor dataid:UpdateDataId;
	dataid:allowsFor dataid:ModifyContent;
	dataid:allowsFor dataid:DeleteContent;
	dataid:allowsFor dataid:ReadContent;
	dataid:allowsFor dataid:ModifyAuthorizedAgents;
	dataid:allowsFor dataid:ResponseToLifeCycleEvent;
	dataid:allowsFor dataid:ResponseToContact;
    rdfs:comment "Maintainer of the dataset. An agent that ensures the technical correctness, accessibility and up-to-dateness of a dataset."@en ;
	rdfs:label "maintainer"@en .

dataid:Contributor
	a dataid:AgentRole;
	rdfs:isDefinedBy <http://dataid.dbpedia.org/ns/core#> ;
	dataid:allowsFor dataid:ReadDataId;
	dataid:allowsFor dataid:ReadContent;
	rdfs:comment "Contributor to the resource. An agent that was involved in creating or maintaining the resource but does not have the main part in this activity."@en ;
	rdfs:label "contributor"@en .

dataid:Contact
	a dataid:AgentRole;
	rdfs:isDefinedBy <http://dataid.dbpedia.org/ns/core#> ;
	dataid:allowsFor dataid:ReadDataId;
	dataid:allowsFor dataid:ModifyContent;
	dataid:allowsFor dataid:ReadContent;
	dataid:allowsFor dataid:ResponseToContact;
    rdfs:comment "Contact agent. An agent that can be contacted for general requests about the resource."@en ;
	rdfs:label "contact"@en .

dataid:Publisher
	a dataid:AgentRole;
	rdfs:isDefinedBy <http://dataid.dbpedia.org/ns/core#> ;
	dataid:allowsFor dataid:ReadDataId;
	dataid:allowsFor dataid:UpdateDataId;
	dataid:allowsFor dataid:ModifyContent;
	dataid:allowsFor dataid:DeleteContent;
	dataid:allowsFor dataid:ReadContent;
	dataid:allowsFor dataid:ModifyAuthorizedAgents;
	dataid:allowsFor dataid:ResponseToLifeCycleEvent;
	dataid:allowsFor dataid:ResponseToContact;
	dataid:allowsFor dataid:AgentSupervision;
	dataid:allowsFor dataid:PublishingDecision;
	dataid:allowsFor dataid:ModifyAccessLevel;
    rdfs:comment "Publisher of the dataset. An agent that makes the dataset accessible online on a server or repository without necessarily being involved in its creation."@en ;
	rdfs:label "publisher"@en .

#defining the generic Agent for any Agent not specifically defined
dataid:GuestAgent
    a dataid:Agent;
    rdfs:isDefinedBy <http://dataid.dbpedia.org/ns/core#> ;
    foaf:mbox 		<mailto:address@alibi.com> ;
    foaf:homepage  <http://dataid.dbpedia.org>;
    foaf:name   "Guest Actor".
