<?xml version="1.0" encoding="utf-8"?>
<rdf:RDF xmlns:datacite="http://purl.org/spar/datacite/"
   xmlns:dataid="http://dataid.dbpedia.org/ns/core#"
   xmlns:dcat="http://www.w3.org/ns/dcat#"
   xmlns:dct="http://purl.org/dc/terms/"
   xmlns:foaf="http://xmlns.com/foaf/0.1/"
   xmlns:litre="http://www.essepuntato.it/2010/06/literalreification/"
   xmlns:lvont="http://lexvo.org/ontology#"
   xmlns:odrl="http://www.w3.org/ns/odrl/2/"
   xmlns:owl="http://www.w3.org/2002/07/owl#"
   xmlns:prov="http://www.w3.org/ns/prov#"
   xmlns:rdf="http://www.w3.org/1999/02/22-rdf-syntax-ns#"
   xmlns:rdfs="http://www.w3.org/2000/01/rdf-schema#"
   xmlns:skos="http://www.w3.org/2004/02/skos/core#"
   xmlns:spdx="http://spdx.org/rdf/terms/#"
   xmlns:vann="http://purl.org/vocab/vann/"
   xmlns:void="http://rdfs.org/ns/void#"
   xmlns:xml="http://www.w3.org/XML/1998/namespace"
   xmlns:xsd="http://www.w3.org/2001/XMLSchema#">
  <owl:Ontology rdf:about="http://dataid.dbpedia.org/ns/core#">
    <dct:creator rdf:resource="http://wiki.dbpedia.org/Association/Persons/Freudenberg"/>
    <dct:license rdf:resource="http://purl.org/NET/rdflicense/cc-by4.0"/>
    <dct:modified>2016-07-21</dct:modified>
    <vann:preferredNamespacePrefix>dataid</vann:preferredNamespacePrefix>
    <vann:preferredNamespaceUri>http://dataid.dbpedia.org/ns/core#</vann:preferredNamespaceUri>
    <rdfs:comment xml:lang="en">The DataID core ontology is the central part of the DataID multi-layered metadata system. &#xD;
Its goal is to extensively describes datasets and their different manifestations in a uniform way, &#xD;
as well as relations to agents like persons or organisations, in regard to their rights and responsibilities. &#xD;
Established vocabularies like DCAT, VoID, Prov-O are used for maximum compatibility.&#xD;
We introduced a multilayer concept of supporting ontologies extending DataID core to fit different &#xD;
use case scenarios (for Linked Data, providing statistical data about datasets etc.).&#xD;
By describing datasets including content, authors, licenses and provenance via RDF, thereby making data &#xD;
accessible to others, is the basic idea of Linked Open Data and is your contribution to a &#xD;
universal data give and take. You can create your own DataID files for any type of data at http://dataid.dbpedia.org.&#xD;
Validating and delivering metadata files in a uniform way, as well as providing the ability to query for datasets, &#xD;
are main objectives of the DBpedia/DataID project.</rdfs:comment>
    <rdfs:label xml:lang="en">DataID</rdfs:label>
    <owl:imports rdf:resource="http://rdfs.org/ns/void#"/>
    <owl:imports rdf:resource="http://www.w3.org/ns/dcat#"/>
    <owl:imports rdf:resource="http://www.w3.org/ns/prov#"/>
    <owl:versionInfo>2.0.0</owl:versionInfo>
    <foaf:depiction rdf:resource="https://raw.githubusercontent.com/dbpedia/DataId-Ontology/master/DataIdOntology.png"/>
  </owl:Ontology>
  <owl:Class rdf:about="http://dataid.dbpedia.org/ns/core#Agent">
    <rdfs:comment xml:lang="en">Agents are general entities representing persons, legal persons or organisations.</rdfs:comment>
    <rdfs:isDefinedBy rdf:resource="http://dataid.dbpedia.org/ns/core#"/>
    <rdfs:label xml:lang="en">Agent</rdfs:label>
    <rdfs:subClassOf rdf:resource="http://purl.org/dc/terms/Agent"/>
    <rdfs:subClassOf rdf:resource="http://www.w3.org/ns/prov#Agent"/>
    <rdfs:subClassOf rdf:resource="http://xmlns.com/foaf/0.1/Agent"/>
  </owl:Class>
  <owl:Class rdf:about="http://dataid.dbpedia.org/ns/core#AgentRole">
    <rdfs:comment xml:lang="en">Agent roles are defined by a set of rights and responsibilities (see AuthorizedAction) an agent, assigned with this role, has to address or can execute.</rdfs:comment>
    <rdfs:isDefinedBy rdf:resource="http://dataid.dbpedia.org/ns/core#"/>
    <rdfs:label xml:lang="en">Agent Role</rdfs:label>
    <rdfs:subClassOf rdf:resource="http://www.w3.org/2004/02/skos/core#Concept"/>
    <rdfs:subClassOf rdf:resource="http://www.w3.org/ns/prov#Role"/>
  </owl:Class>
  <owl:NamedIndividual rdf:about="http://dataid.dbpedia.org/ns/core#AgentRoleScheme">
    <rdf:type rdf:resource="http://www.w3.org/2004/02/skos/core#ConceptScheme"/>
    <rdfs:comment xml:lang="en">Description of the agent role hierarchy.</rdfs:comment>
    <rdfs:label xml:lang="en">agent role scheme</rdfs:label>
    <skos:hasTopConcept rdf:resource="http://dataid.dbpedia.org/ns/core#Creator"/>
  </owl:NamedIndividual>
  <owl:NamedIndividual rdf:about="http://dataid.dbpedia.org/ns/core#AgentSupervision">
    <rdf:type rdf:resource="http://dataid.dbpedia.org/ns/core#ResponsibleAction"/>
    <rdfs:comment xml:lang="en">The responsibility to supervise other agents.</rdfs:comment>
    <rdfs:isDefinedBy rdf:resource="http://dataid.dbpedia.org/ns/core#"/>
    <rdfs:label xml:lang="en">agent supervision</rdfs:label>
    <skos:broader rdf:resource="http://dataid.dbpedia.org/ns/core#AllResponsibilities"/>
    <skos:inScheme rdf:resource="http://dataid.dbpedia.org/ns/core#AuthorizedActionScheme"/>
    <skos:prefLabel xml:lang="en">agent supervision</skos:prefLabel>
  </owl:NamedIndividual>
  <owl:NamedIndividual rdf:about="http://dataid.dbpedia.org/ns/core#AllEntitlements">
    <rdf:type rdf:resource="http://dataid.dbpedia.org/ns/core#ResponsibleAction"/>
    <rdfs:comment xml:lang="en">Encompasses all entitlements.</rdfs:comment>
    <rdfs:isDefinedBy rdf:resource="http://dataid.dbpedia.org/ns/core#"/>
    <rdfs:label xml:lang="en">all entitlements</rdfs:label>
    <skos:prefLabel xml:lang="en">all entitlements</skos:prefLabel>
    <skos:topConceptOf rdf:resource="http://dataid.dbpedia.org/ns/core#AuthorizedActionScheme"/>
  </owl:NamedIndividual>
  <owl:NamedIndividual rdf:about="http://dataid.dbpedia.org/ns/core#AllResponsibilities">
    <rdf:type rdf:resource="http://dataid.dbpedia.org/ns/core#ResponsibleAction"/>
    <rdfs:comment xml:lang="en">Encompasses all responsibilities.</rdfs:comment>
    <rdfs:isDefinedBy rdf:resource="http://dataid.dbpedia.org/ns/core#"/>
    <rdfs:label xml:lang="en">all responsibilities</rdfs:label>
    <skos:prefLabel xml:lang="en">all responsibilities</skos:prefLabel>
    <skos:topConceptOf rdf:resource="http://dataid.dbpedia.org/ns/core#AuthorizedActionScheme"/>
  </owl:NamedIndividual>
  <owl:Class rdf:about="http://dataid.dbpedia.org/ns/core#Authorization">
    <rdfs:comment xml:lang="en">This concept is a mediator between a set of entities (or scope) defines by the property dataid:authorizedFor,&#xD;
	a set of AgentRoles defining rights and responsibilities and Agents, fulfilling the AgentRoles, in regard to the collection of entities.&#xD;
	This subclass of prov:Attribution qualifies the relation prov:wasAttributedTo between prov:Entity and prov:Agent with the AgentRoles &#xD;
	and AuthorizedActions of the DataID-domain.</rdfs:comment>
    <rdfs:isDefinedBy rdf:resource="http://dataid.dbpedia.org/ns/core#"/>
    <rdfs:label xml:lang="en">Authorization</rdfs:label>
    <rdfs:subClassOf rdf:resource="http://www.w3.org/ns/prov#Attribution"/>
  </owl:Class>
  <owl:Class rdf:about="http://dataid.dbpedia.org/ns/core#AuthorizedAction">
    <rdfs:comment xml:lang="en">Authorized actions may constiute either of activities an Agent can execute in regard to a collection of prov:Entities or of &#xD;
    responsibilities an Agent should act upon (e.g. make certain decisions if necessary or act upon certain events).</rdfs:comment>
    <rdfs:isDefinedBy rdf:resource="http://dataid.dbpedia.org/ns/core#"/>
    <rdfs:label xml:lang="en">Authorized Action</rdfs:label>
    <rdfs:subClassOf rdf:resource="http://www.w3.org/2004/02/skos/core#Concept"/>
  </owl:Class>
  <owl:NamedIndividual rdf:about="http://dataid.dbpedia.org/ns/core#AuthorizedActionScheme">
    <rdf:type rdf:resource="http://www.w3.org/2004/02/skos/core#ConceptScheme"/>
    <rdfs:comment xml:lang="en">Description of the authorized action hierarchy.</rdfs:comment>
    <rdfs:label xml:lang="en">authorized action scheme</rdfs:label>
    <skos:hasTopConcept rdf:resource="http://dataid.dbpedia.org/ns/core#AllEntitlements"/>
    <skos:hasTopConcept rdf:resource="http://dataid.dbpedia.org/ns/core#AllResponsibilities"/>
  </owl:NamedIndividual>
  <owl:NamedIndividual rdf:about="http://dataid.dbpedia.org/ns/core#Contact">
    <dataid:allowsFor rdf:resource="http://dataid.dbpedia.org/ns/core#ModifyContent"/>
    <dataid:allowsFor rdf:resource="http://dataid.dbpedia.org/ns/core#ReadContent"/>
    <dataid:allowsFor rdf:resource="http://dataid.dbpedia.org/ns/core#ReadDataId"/>
    <dataid:allowsFor rdf:resource="http://dataid.dbpedia.org/ns/core#ResponseToContact"/>
    <rdf:type rdf:resource="http://dataid.dbpedia.org/ns/core#AgentRole"/>
    <rdfs:comment xml:lang="en">Contact agent. An agent that can be contacted for general requests about the resource.</rdfs:comment>
    <rdfs:isDefinedBy rdf:resource="http://dataid.dbpedia.org/ns/core#"/>
    <rdfs:label xml:lang="en">contact</rdfs:label>
    <skos:broader rdf:resource="http://dataid.dbpedia.org/ns/core#Maintainer"/>
    <skos:broader rdf:resource="http://dataid.dbpedia.org/ns/core#Publisher"/>
    <skos:inScheme rdf:resource="http://dataid.dbpedia.org/ns/core#AgentRoleScheme"/>
    <skos:prefLabel xml:lang="en">contact</skos:prefLabel>
  </owl:NamedIndividual>
  <owl:NamedIndividual rdf:about="http://dataid.dbpedia.org/ns/core#Contributor">
    <dataid:allowsFor rdf:resource="http://dataid.dbpedia.org/ns/core#ReadContent"/>
    <dataid:allowsFor rdf:resource="http://dataid.dbpedia.org/ns/core#ReadDataId"/>
    <rdf:type rdf:resource="http://dataid.dbpedia.org/ns/core#AgentRole"/>
    <rdfs:comment xml:lang="en">Contributor to the resource. An agent that was involved in creating or maintaining the resource but does not have the main part in this activity.</rdfs:comment>
    <rdfs:isDefinedBy rdf:resource="http://dataid.dbpedia.org/ns/core#"/>
    <rdfs:label xml:lang="en">contributor</rdfs:label>
    <skos:broader rdf:resource="http://dataid.dbpedia.org/ns/core#Publisher"/>
    <skos:inScheme rdf:resource="http://dataid.dbpedia.org/ns/core#AgentRoleScheme"/>
    <skos:prefLabel xml:lang="en">contributor</skos:prefLabel>
  </owl:NamedIndividual>
  <owl:NamedIndividual rdf:about="http://dataid.dbpedia.org/ns/core#Creator">
    <dataid:allowsFor rdf:resource="http://dataid.dbpedia.org/ns/core#AllEntitlements"/>
    <dataid:allowsFor rdf:resource="http://dataid.dbpedia.org/ns/core#AllResponsibilities"/>
    <rdf:type rdf:resource="http://dataid.dbpedia.org/ns/core#AgentRole"/>
    <rdfs:comment xml:lang="en">Creator of the resource. An agent that is credited with a main part in the initial creation of the resource.</rdfs:comment>
    <rdfs:isDefinedBy rdf:resource="http://dataid.dbpedia.org/ns/core#"/>
    <rdfs:label xml:lang="en">creator</rdfs:label>
    <skos:prefLabel xml:lang="en">creator</skos:prefLabel>
    <skos:topConceptOf rdf:resource="http://dataid.dbpedia.org/ns/core#AgentRoleScheme"/>
  </owl:NamedIndividual>
  <owl:Class rdf:about="http://dataid.dbpedia.org/ns/core#DataId">
    <rdfs:comment xml:lang="en">A DataId Induvidual serves as a root Entity for every DataID document describing one or more datasets. As a subclass of dcat:CatalogRecord / void:DatasetDescription it describes not a dataset itself but provides metadata about its entry in a dcat:Catalog and/or its relations to repositories or other data collections .</rdfs:comment>
    <rdfs:isDefinedBy rdf:resource="http://dataid.dbpedia.org/ns/core#"/>
    <rdfs:label xml:lang="en">DataId</rdfs:label>
    <rdfs:subClassOf rdf:resource="http://rdfs.org/ns/void#DatasetDescription"/>
    <rdfs:subClassOf rdf:resource="http://www.w3.org/ns/dcat#CatalogRecord"/>
    <rdfs:subClassOf rdf:resource="http://www.w3.org/ns/prov#Entity"/>
    <rdfs:subClassOf>
      <owl:Restriction>
        <owl:allValuesFrom rdf:resource="http://dataid.dbpedia.org/ns/core#Dataset"/>
        <owl:onProperty rdf:resource="http://xmlns.com/foaf/0.1/primaryTopic"/>
      </owl:Restriction>
    </rdfs:subClassOf>
    <rdfs:subClassOf>
      <owl:Restriction>
        <owl:allValuesFrom rdf:resource="http://dataid.dbpedia.org/ns/core#DataId"/>
        <owl:onProperty rdf:resource="http://dataid.dbpedia.org/ns/core#nextVersion"/>
      </owl:Restriction>
    </rdfs:subClassOf>
    <rdfs:subClassOf>
      <owl:Restriction>
        <owl:allValuesFrom rdf:resource="http://dataid.dbpedia.org/ns/core#DataId"/>
        <owl:onProperty rdf:resource="http://dataid.dbpedia.org/ns/core#previousVersion"/>
      </owl:Restriction>
    </rdfs:subClassOf>
    <rdfs:subClassOf>
      <owl:Restriction>
        <owl:allValuesFrom rdf:resource="http://dataid.dbpedia.org/ns/core#DataId"/>
        <owl:onProperty rdf:resource="http://dataid.dbpedia.org/ns/core#latestVersion"/>
      </owl:Restriction>
    </rdfs:subClassOf>
    <rdfs:subClassOf>
      <owl:Restriction>
        <owl:allValuesFrom rdf:resource="http://www.w3.org/ns/odrl/2/Policy"/>
        <owl:onProperty rdf:resource="http://purl.org/dc/terms/license"/>
      </owl:Restriction>
    </rdfs:subClassOf>
    <rdfs:subClassOf>
      <owl:Restriction>
        <owl:allValuesFrom rdf:resource="http://lexvo.org/ontology#Language"/>
        <owl:onProperty rdf:resource="http://purl.org/dc/terms/language"/>
      </owl:Restriction>
    </rdfs:subClassOf>
  </owl:Class>
  <owl:Class rdf:about="http://dataid.dbpedia.org/ns/core#Dataset">
    <rdfs:comment xml:lang="en">A collection of data, available for access in one or more formats. Dataset resources describe the &#xD;
    concept of the dataset, not it's manifestation (the data itself), which can be acquired as a dataid:Distribution.&#xD;
    Datasets are prov:Entities and can be generated by prov:Activities.</rdfs:comment>
    <rdfs:isDefinedBy rdf:resource="http://dataid.dbpedia.org/ns/core#"/>
    <rdfs:label xml:lang="en">Dataset</rdfs:label>
    <rdfs:subClassOf rdf:resource="http://rdfs.org/ns/void#Dataset"/>
    <rdfs:subClassOf rdf:resource="http://www.w3.org/ns/dcat#Dataset"/>
    <rdfs:subClassOf rdf:resource="http://www.w3.org/ns/prov#Entity"/>
    <rdfs:subClassOf>
      <owl:Restriction>
        <owl:allValuesFrom rdf:resource="http://dataid.dbpedia.org/ns/core#Dataset"/>
        <owl:onProperty rdf:resource="http://dataid.dbpedia.org/ns/core#latestVersion"/>
      </owl:Restriction>
    </rdfs:subClassOf>
    <rdfs:subClassOf>
      <owl:Restriction>
        <owl:allValuesFrom rdf:resource="http://www.w3.org/ns/odrl/2/Policy"/>
        <owl:onProperty rdf:resource="http://purl.org/dc/terms/license"/>
      </owl:Restriction>
    </rdfs:subClassOf>
    <rdfs:subClassOf>
      <owl:Restriction>
        <owl:allValuesFrom rdf:resource="http://lexvo.org/ontology#Language"/>
        <owl:onProperty rdf:resource="http://purl.org/dc/terms/language"/>
      </owl:Restriction>
    </rdfs:subClassOf>
    <rdfs:subClassOf>
      <owl:Restriction>
        <owl:allValuesFrom rdf:resource="http://dataid.dbpedia.org/ns/core#Dataset"/>
        <owl:onProperty rdf:resource="http://purl.org/dc/terms/isPartOf"/>
      </owl:Restriction>
    </rdfs:subClassOf>
    <rdfs:subClassOf>
      <owl:Restriction>
        <owl:allValuesFrom rdf:resource="http://dataid.dbpedia.org/ns/core#Dataset"/>
        <owl:onProperty rdf:resource="http://rdfs.org/ns/void#subset"/>
      </owl:Restriction>
    </rdfs:subClassOf>
    <rdfs:subClassOf>
      <owl:Restriction>
        <owl:allValuesFrom rdf:resource="http://dataid.dbpedia.org/ns/core#Distribution"/>
        <owl:onProperty rdf:resource="http://www.w3.org/ns/dcat#distribution"/>
      </owl:Restriction>
    </rdfs:subClassOf>
    <rdfs:subClassOf>
      <owl:Restriction>
        <owl:allValuesFrom rdf:resource="http://www.w3.org/2006/time#Interval"/>
        <owl:onProperty rdf:resource="http://purl.org/dc/terms/temporal"/>
      </owl:Restriction>
    </rdfs:subClassOf>
    <rdfs:subClassOf>
      <owl:Restriction>
        <owl:allValuesFrom rdf:resource="http://www.geonames.org/ontology#Feature"/>
        <owl:onProperty rdf:resource="http://purl.org/dc/terms/spatial"/>
      </owl:Restriction>
    </rdfs:subClassOf>
    <rdfs:subClassOf>
      <owl:Restriction>
        <owl:allValuesFrom rdf:resource="http://dataid.dbpedia.org/ns/core#DataId"/>
        <owl:onProperty rdf:resource="http://xmlns.com/foaf/0.1/isPrimaryTopicOf"/>
      </owl:Restriction>
    </rdfs:subClassOf>
    <rdfs:subClassOf>
      <owl:Restriction>
        <owl:allValuesFrom rdf:resource="http://dataid.dbpedia.org/ns/core#Dataset"/>
        <owl:onProperty rdf:resource="http://dataid.dbpedia.org/ns/core#nextVersion"/>
      </owl:Restriction>
    </rdfs:subClassOf>
    <rdfs:subClassOf>
      <owl:Restriction>
        <owl:allValuesFrom rdf:resource="http://dataid.dbpedia.org/ns/core#Dataset"/>
        <owl:onProperty rdf:resource="http://dataid.dbpedia.org/ns/core#previousVersion"/>
      </owl:Restriction>
    </rdfs:subClassOf>
  </owl:Class>
  <owl:NamedIndividual rdf:about="http://dataid.dbpedia.org/ns/core#DeleteContent">
    <rdf:type rdf:resource="http://dataid.dbpedia.org/ns/core#EntitledAction"/>
    <rdfs:comment xml:lang="en">Entitled action to delete some content of an entity.</rdfs:comment>
    <rdfs:isDefinedBy rdf:resource="http://dataid.dbpedia.org/ns/core#"/>
    <rdfs:label xml:lang="en">delete content right</rdfs:label>
    <skos:broader rdf:resource="http://dataid.dbpedia.org/ns/core#AllEntitlements"/>
    <skos:inScheme rdf:resource="http://dataid.dbpedia.org/ns/core#AuthorizedActionScheme"/>
    <skos:prefLabel xml:lang="en">delete content right</skos:prefLabel>
  </owl:NamedIndividual>
  <owl:Class rdf:about="http://dataid.dbpedia.org/ns/core#Directory">
    <rdfs:comment xml:lang="en">A dedicated directory holding (multiple) files of the same dataset, which, when put together, make up the whole dataset.</rdfs:comment>
    <rdfs:isDefinedBy rdf:resource="http://dataid.dbpedia.org/ns/core#"/>
    <rdfs:label xml:lang="en">Directory</rdfs:label>
    <rdfs:subClassOf rdf:resource="http://dataid.dbpedia.org/ns/core#Distribution"/>
  </owl:Class>
  <owl:Class rdf:about="http://dataid.dbpedia.org/ns/core#Distribution">
    <rdfs:comment xml:lang="en">Distributions describe a single manifestation of the pertaining Dataset (for example; its data format/serialization or a service endpoint including the procedure required to acces the data).</rdfs:comment>
    <rdfs:isDefinedBy rdf:resource="http://dataid.dbpedia.org/ns/core#"/>
    <rdfs:label xml:lang="en">Distribution</rdfs:label>
    <rdfs:subClassOf rdf:resource="http://www.w3.org/ns/dcat#Distribution"/>
    <rdfs:subClassOf rdf:resource="http://www.w3.org/ns/prov#Entity"/>
    <rdfs:subClassOf>
      <owl:Restriction>
        <owl:allValuesFrom rdf:resource="http://dataid.dbpedia.org/ns/core#Distribution"/>
        <owl:onProperty rdf:resource="http://dataid.dbpedia.org/ns/core#nextVersion"/>
      </owl:Restriction>
    </rdfs:subClassOf>
    <rdfs:subClassOf>
      <owl:Restriction>
        <owl:allValuesFrom rdf:resource="http://dataid.dbpedia.org/ns/core#Distribution"/>
        <owl:onProperty rdf:resource="http://dataid.dbpedia.org/ns/core#previousVersion"/>
      </owl:Restriction>
    </rdfs:subClassOf>
    <rdfs:subClassOf>
      <owl:Restriction>
        <owl:allValuesFrom rdf:resource="http://dataid.dbpedia.org/ns/core#Distribution"/>
        <owl:onProperty rdf:resource="http://dataid.dbpedia.org/ns/core#latestVersion"/>
      </owl:Restriction>
    </rdfs:subClassOf>
    <rdfs:subClassOf>
      <owl:Restriction>
        <owl:allValuesFrom rdf:resource="http://www.w3.org/ns/odrl/2/Policy"/>
        <owl:onProperty rdf:resource="http://purl.org/dc/terms/license"/>
      </owl:Restriction>
    </rdfs:subClassOf>
    <rdfs:subClassOf>
      <owl:Restriction>
        <owl:allValuesFrom rdf:resource="http://lexvo.org/ontology#Language"/>
        <owl:onProperty rdf:resource="http://purl.org/dc/terms/language"/>
      </owl:Restriction>
    </rdfs:subClassOf>
  </owl:Class>
  <owl:Class rdf:about="http://dataid.dbpedia.org/ns/core#EntitledAction">
    <rdfs:comment xml:lang="en">EntitledActions describe actions an Agent is allowed to perform when holding a certain AgentRole. &#xD;
	These actions may address restricted matters like access, modification rights and others.</rdfs:comment>
    <rdfs:isDefinedBy rdf:resource="http://dataid.dbpedia.org/ns/core#"/>
    <rdfs:label xml:lang="en">Entitled Action</rdfs:label>
    <rdfs:subClassOf rdf:resource="http://dataid.dbpedia.org/ns/core#AuthorizedAction"/>
    <owl:disjointWith rdf:resource="http://dataid.dbpedia.org/ns/core#ResponsibleAction"/>
  </owl:Class>
  <owl:Class rdf:about="http://dataid.dbpedia.org/ns/core#FileCollection">
    <rdfs:comment xml:lang="en">Multiple files constituting one (complete) dataset (files in different locations are possible).</rdfs:comment>
    <rdfs:isDefinedBy rdf:resource="http://dataid.dbpedia.org/ns/core#"/>
    <rdfs:label xml:lang="en">File Collection</rdfs:label>
    <rdfs:subClassOf rdf:resource="http://dataid.dbpedia.org/ns/core#Distribution"/>
  </owl:Class>
  <owl:NamedIndividual rdf:about="http://dataid.dbpedia.org/ns/core#Guest">
    <dataid:allowsFor rdf:resource="http://dataid.dbpedia.org/ns/core#ReadContent"/>
    <dataid:allowsFor rdf:resource="http://dataid.dbpedia.org/ns/core#ReadDataId"/>
    <rdf:type rdf:resource="http://dataid.dbpedia.org/ns/core#AgentRole"/>
    <rdfs:comment xml:lang="en">A visitor/anonymous agent has only read rights on public and semi-private documents</rdfs:comment>
    <rdfs:isDefinedBy rdf:resource="http://dataid.dbpedia.org/ns/core#"/>
    <rdfs:label xml:lang="en">guest</rdfs:label>
    <skos:broader rdf:resource="http://dataid.dbpedia.org/ns/core#Contributor"/>
    <skos:inScheme rdf:resource="http://dataid.dbpedia.org/ns/core#AgentRoleScheme"/>
    <skos:prefLabel xml:lang="en">guest</skos:prefLabel>
  </owl:NamedIndividual>
  <owl:NamedIndividual rdf:about="http://dataid.dbpedia.org/ns/core#GuestAgent">
    <rdf:type rdf:resource="http://dataid.dbpedia.org/ns/core#Agent"/>
    <rdfs:comment xml:lang="en">Use this agent as a stand in for any agent not specifically defined in a domain, granting public access to an entity.</rdfs:comment>
    <rdfs:isDefinedBy rdf:resource="http://dataid.dbpedia.org/ns/core#"/>
    <rdfs:label xml:lang="en">guest agent</rdfs:label>
    <foaf:homepage rdf:resource="http://dataid.dbpedia.org"/>
    <foaf:mbox rdf:resource="mailto:address@alibi.com"/>
    <foaf:name>Guest Agent</foaf:name>
  </owl:NamedIndividual>
  <owl:NamedIndividual rdf:about="http://dataid.dbpedia.org/ns/core#GuestAuthorization">
    <dataid:authorityAgentRole rdf:resource="http://dataid.dbpedia.org/ns/core#Guest"/>
    <dataid:authorizedAgent rdf:resource="http://dataid.dbpedia.org/ns/core#GuestAgent"/>
    <dataid:isInheritable rdf:datatype="http://www.w3.org/2001/XMLSchema#boolean">true</dataid:isInheritable>
    <rdf:type rdf:resource="http://dataid.dbpedia.org/ns/core#Authorization"/>
    <rdfs:comment xml:lang="en">This authorization can be used to point out that the content of an entity is public an can be read by anyone (see also dataid:Guest).</rdfs:comment>
    <rdfs:isDefinedBy rdf:resource="http://dataid.dbpedia.org/ns/core#"/>
    <rdfs:label xml:lang="en">guest authority</rdfs:label>
  </owl:NamedIndividual>
  <owl:Class rdf:about="http://dataid.dbpedia.org/ns/core#Identifier">
    <rdfs:comment xml:lang="en">Uniquely identifies any resource, given an identifier as literal (see dataid:statement) and a corresponding aid/pid scheme &#xD;
(ORCID, ResearcherID etc. pointed out via datacite:usesIdentifierScheme). Optionally it can point out a reference document on the web (about this identifier) using dct:references.</rdfs:comment>
    <rdfs:isDefinedBy rdf:resource="http://dataid.dbpedia.org/ns/core#"/>
    <rdfs:label xml:lang="en">Identifier</rdfs:label>
    <rdfs:subClassOf rdf:resource="http://purl.org/spar/datacite/Identifier"/>
    <rdfs:subClassOf>
      <owl:Restriction>
        <owl:allValuesFrom rdf:resource="http://xmlns.com/foaf/0.1/Document"/>
        <owl:onProperty rdf:resource="http://purl.org/dc/terms/references"/>
      </owl:Restriction>
    </rdfs:subClassOf>
  </owl:Class>
  <owl:NamedIndividual rdf:about="http://dataid.dbpedia.org/ns/core#Maintainer">
    <dataid:allowsFor rdf:resource="http://dataid.dbpedia.org/ns/core#DeleteContent"/>
    <dataid:allowsFor rdf:resource="http://dataid.dbpedia.org/ns/core#ModifyAuthorizedAgents"/>
    <dataid:allowsFor rdf:resource="http://dataid.dbpedia.org/ns/core#ModifyContent"/>
    <dataid:allowsFor rdf:resource="http://dataid.dbpedia.org/ns/core#ReadContent"/>
    <dataid:allowsFor rdf:resource="http://dataid.dbpedia.org/ns/core#ReadDataId"/>
    <dataid:allowsFor rdf:resource="http://dataid.dbpedia.org/ns/core#ResponseToContact"/>
    <dataid:allowsFor rdf:resource="http://dataid.dbpedia.org/ns/core#ResponseToLifeCycleEvent"/>
    <dataid:allowsFor rdf:resource="http://dataid.dbpedia.org/ns/core#UpdateDataId"/>
    <rdf:type rdf:resource="http://dataid.dbpedia.org/ns/core#AgentRole"/>
    <rdfs:comment xml:lang="en">Maintainer of the dataset. An agent that ensures the technical correctness, accessibility and up-to-dateness of a dataset.</rdfs:comment>
    <rdfs:isDefinedBy rdf:resource="http://dataid.dbpedia.org/ns/core#"/>
    <rdfs:label xml:lang="en">maintainer</rdfs:label>
    <skos:broader rdf:resource="http://dataid.dbpedia.org/ns/core#Creator"/>
    <skos:inScheme rdf:resource="http://dataid.dbpedia.org/ns/core#AgentRoleScheme"/>
    <skos:prefLabel xml:lang="en">maintainer</skos:prefLabel>
  </owl:NamedIndividual>
  <owl:Class rdf:about="http://dataid.dbpedia.org/ns/core#MediaType">
    <rdfs:comment xml:lang="en">Extends the dct:MediaType class of Dublin Core, providing the Iana media type description (or mime type) and common file extensions used. &#xD;
A pointer to an inner media types can describe (multiple) layers of compressions and all internal media types.</rdfs:comment>
    <rdfs:isDefinedBy rdf:resource="http://dataid.dbpedia.org/ns/core#"/>
    <rdfs:label xml:lang="en">Media Type</rdfs:label>
    <rdfs:subClassOf rdf:resource="http://purl.org/dc/terms/MediaType"/>
  </owl:Class>
  <owl:NamedIndividual rdf:about="http://dataid.dbpedia.org/ns/core#ModifyAgentRoles">
    <rdf:type rdf:resource="http://dataid.dbpedia.org/ns/core#EntitledAction"/>
    <rdfs:comment xml:lang="en">Entitled action to modify the role of agents on certain entities.</rdfs:comment>
    <rdfs:isDefinedBy rdf:resource="http://dataid.dbpedia.org/ns/core#"/>
    <rdfs:label xml:lang="en">modify agent roles</rdfs:label>
    <skos:broader rdf:resource="http://dataid.dbpedia.org/ns/core#AllEntitlements"/>
    <skos:inScheme rdf:resource="http://dataid.dbpedia.org/ns/core#AuthorizedActionScheme"/>
    <skos:prefLabel xml:lang="en">modify agent roles</skos:prefLabel>
  </owl:NamedIndividual>
  <owl:NamedIndividual rdf:about="http://dataid.dbpedia.org/ns/core#ModifyAuthorization">
    <rdf:type rdf:resource="http://dataid.dbpedia.org/ns/core#EntitledAction"/>
    <rdfs:comment xml:lang="en">Entitled action to modify an authorization.</rdfs:comment>
    <rdfs:isDefinedBy rdf:resource="http://dataid.dbpedia.org/ns/core#"/>
    <rdfs:label xml:lang="en">modify authorization</rdfs:label>
    <skos:broader rdf:resource="http://dataid.dbpedia.org/ns/core#AllEntitlements"/>
    <skos:inScheme rdf:resource="http://dataid.dbpedia.org/ns/core#AuthorizedActionScheme"/>
    <skos:prefLabel xml:lang="en">modify authorization</skos:prefLabel>
  </owl:NamedIndividual>
  <owl:NamedIndividual rdf:about="http://dataid.dbpedia.org/ns/core#ModifyAuthorizedAgents">
    <rdf:type rdf:resource="http://dataid.dbpedia.org/ns/core#EntitledAction"/>
    <rdfs:comment xml:lang="en">Entitled action to modify which agents are authorized on certain entities.</rdfs:comment>
    <rdfs:isDefinedBy rdf:resource="http://dataid.dbpedia.org/ns/core#"/>
    <rdfs:label xml:lang="en">modify authorized agents</rdfs:label>
    <skos:broader rdf:resource="http://dataid.dbpedia.org/ns/core#AllEntitlements"/>
    <skos:inScheme rdf:resource="http://dataid.dbpedia.org/ns/core#AuthorizedActionScheme"/>
    <skos:prefLabel xml:lang="en">modify authorized agents</skos:prefLabel>
  </owl:NamedIndividual>
  <owl:NamedIndividual rdf:about="http://dataid.dbpedia.org/ns/core#ModifyContent">
    <rdf:type rdf:resource="http://dataid.dbpedia.org/ns/core#EntitledAction"/>
    <rdfs:comment xml:lang="en">Entitled action to modify the content of an entity.</rdfs:comment>
    <rdfs:isDefinedBy rdf:resource="http://dataid.dbpedia.org/ns/core#"/>
    <rdfs:label xml:lang="en">modify content right</rdfs:label>
    <skos:broader rdf:resource="http://dataid.dbpedia.org/ns/core#DeleteContent"/>
    <skos:inScheme rdf:resource="http://dataid.dbpedia.org/ns/core#AuthorizedActionScheme"/>
    <skos:prefLabel xml:lang="en">modify content right</skos:prefLabel>
  </owl:NamedIndividual>
  <owl:NamedIndividual rdf:about="http://dataid.dbpedia.org/ns/core#Publisher">
    <dataid:allowsFor rdf:resource="http://dataid.dbpedia.org/ns/core#AgentSupervision"/>
    <dataid:allowsFor rdf:resource="http://dataid.dbpedia.org/ns/core#DeleteContent"/>
    <dataid:allowsFor rdf:resource="http://dataid.dbpedia.org/ns/core#ModifyAuthorization"/>
    <dataid:allowsFor rdf:resource="http://dataid.dbpedia.org/ns/core#ModifyAuthorizedAgents"/>
    <dataid:allowsFor rdf:resource="http://dataid.dbpedia.org/ns/core#ModifyContent"/>
    <dataid:allowsFor rdf:resource="http://dataid.dbpedia.org/ns/core#PublishingDecision"/>
    <dataid:allowsFor rdf:resource="http://dataid.dbpedia.org/ns/core#ReadContent"/>
    <dataid:allowsFor rdf:resource="http://dataid.dbpedia.org/ns/core#ReadDataId"/>
    <dataid:allowsFor rdf:resource="http://dataid.dbpedia.org/ns/core#ResponseToContact"/>
    <dataid:allowsFor rdf:resource="http://dataid.dbpedia.org/ns/core#ResponseToLifeCycleEvent"/>
    <dataid:allowsFor rdf:resource="http://dataid.dbpedia.org/ns/core#UpdateDataId"/>
    <rdf:type rdf:resource="http://dataid.dbpedia.org/ns/core#AgentRole"/>
    <rdfs:comment xml:lang="en">Publisher of the dataset. An agent that makes the dataset accessible online on a server or repository without necessarily being involved in its creation.</rdfs:comment>
    <rdfs:isDefinedBy rdf:resource="http://dataid.dbpedia.org/ns/core#"/>
    <rdfs:label xml:lang="en">publisher</rdfs:label>
    <skos:broader rdf:resource="http://dataid.dbpedia.org/ns/core#Creator"/>
    <skos:inScheme rdf:resource="http://dataid.dbpedia.org/ns/core#AgentRoleScheme"/>
    <skos:prefLabel xml:lang="en">publisher</skos:prefLabel>
  </owl:NamedIndividual>
  <owl:NamedIndividual rdf:about="http://dataid.dbpedia.org/ns/core#PublishingDecision">
    <rdf:type rdf:resource="http://dataid.dbpedia.org/ns/core#ResponsibleAction"/>
    <rdfs:comment xml:lang="en">The responsibility decide if the entity should be published</rdfs:comment>
    <rdfs:isDefinedBy rdf:resource="http://dataid.dbpedia.org/ns/core#"/>
    <rdfs:label xml:lang="en">publishing decision</rdfs:label>
    <skos:broader rdf:resource="http://dataid.dbpedia.org/ns/core#AllResponsibilities"/>
    <skos:inScheme rdf:resource="http://dataid.dbpedia.org/ns/core#AuthorizedActionScheme"/>
    <skos:prefLabel xml:lang="en">publishing decision</skos:prefLabel>
  </owl:NamedIndividual>
  <owl:NamedIndividual rdf:about="http://dataid.dbpedia.org/ns/core#ReadContent">
    <rdf:type rdf:resource="http://dataid.dbpedia.org/ns/core#EntitledAction"/>
    <rdfs:comment xml:lang="en">Entitled action to read the content of an entity.</rdfs:comment>
    <rdfs:isDefinedBy rdf:resource="http://dataid.dbpedia.org/ns/core#"/>
    <rdfs:label xml:lang="en">read content right</rdfs:label>
    <skos:broader rdf:resource="http://dataid.dbpedia.org/ns/core#ModifyContent"/>
    <skos:inScheme rdf:resource="http://dataid.dbpedia.org/ns/core#AuthorizedActionScheme"/>
    <skos:prefLabel xml:lang="en">read content right</skos:prefLabel>
  </owl:NamedIndividual>
  <owl:NamedIndividual rdf:about="http://dataid.dbpedia.org/ns/core#ReadDataId">
    <rdf:type rdf:resource="http://dataid.dbpedia.org/ns/core#EntitledAction"/>
    <rdfs:comment xml:lang="en">Entitled action to read the DataID dataset metadata</rdfs:comment>
    <rdfs:isDefinedBy rdf:resource="http://dataid.dbpedia.org/ns/core#"/>
    <rdfs:label xml:lang="en">read DataID right</rdfs:label>
    <skos:broader rdf:resource="http://dataid.dbpedia.org/ns/core#AllEntitlements"/>
    <skos:inScheme rdf:resource="http://dataid.dbpedia.org/ns/core#AuthorizedActionScheme"/>
    <skos:prefLabel xml:lang="en">read DataID right</skos:prefLabel>
  </owl:NamedIndividual>
  <owl:NamedIndividual rdf:about="http://dataid.dbpedia.org/ns/core#ResponseToContact">
    <rdf:type rdf:resource="http://dataid.dbpedia.org/ns/core#ResponsibleAction"/>
    <rdfs:comment xml:lang="en">The responsibility to respond to contact attempts by external agents. A contact point for the entity.</rdfs:comment>
    <rdfs:isDefinedBy rdf:resource="http://dataid.dbpedia.org/ns/core#"/>
    <rdfs:label xml:lang="en">response to contact attempt</rdfs:label>
    <skos:broader rdf:resource="http://dataid.dbpedia.org/ns/core#AllResponsibilities"/>
    <skos:inScheme rdf:resource="http://dataid.dbpedia.org/ns/core#AuthorizedActionScheme"/>
    <skos:prefLabel xml:lang="en">response to contact attempt</skos:prefLabel>
  </owl:NamedIndividual>
  <owl:NamedIndividual rdf:about="http://dataid.dbpedia.org/ns/core#ResponseToLifeCycleEvent">
    <rdf:type rdf:resource="http://dataid.dbpedia.org/ns/core#ResponsibleAction"/>
    <rdfs:comment xml:lang="en">The responsibility to manage changes and react to bugs and issues that are reported</rdfs:comment>
    <rdfs:isDefinedBy rdf:resource="http://dataid.dbpedia.org/ns/core#"/>
    <rdfs:label xml:lang="en">response to life-cycle event</rdfs:label>
    <skos:broader rdf:resource="http://dataid.dbpedia.org/ns/core#AllResponsibilities"/>
    <skos:inScheme rdf:resource="http://dataid.dbpedia.org/ns/core#AuthorizedActionScheme"/>
    <skos:prefLabel xml:lang="en">response to life-cycle event</skos:prefLabel>
  </owl:NamedIndividual>
  <owl:Class rdf:about="http://dataid.dbpedia.org/ns/core#ResponsibleAction">
    <rdfs:comment xml:lang="en">AgentRoles provide rights as well as responsibilities an agent has to attend to in order to fulfill this role. &#xD;
	Responsible actions should describe actions pertaining to responsibilities an agent is supposed to do when holding a specific AgentRole.</rdfs:comment>
    <rdfs:isDefinedBy rdf:resource="http://dataid.dbpedia.org/ns/core#"/>
    <rdfs:label xml:lang="en">Responsible Action</rdfs:label>
    <rdfs:subClassOf rdf:resource="http://dataid.dbpedia.org/ns/core#AuthorizedAction"/>
    <owl:disjointWith rdf:resource="http://dataid.dbpedia.org/ns/core#EntitledAction"/>
  </owl:Class>
  <owl:Class rdf:about="http://dataid.dbpedia.org/ns/core#ServiceEndpoint">
    <rdfs:comment xml:lang="en">A specific distribution, which is accessible via an access url and provides data as a web service in a certain format.</rdfs:comment>
    <rdfs:isDefinedBy rdf:resource="http://dataid.dbpedia.org/ns/core#"/>
    <rdfs:label xml:lang="en">Service Endpoint</rdfs:label>
    <rdfs:subClassOf rdf:resource="http://dataid.dbpedia.org/ns/core#Distribution"/>
  </owl:Class>
  <owl:Class rdf:about="http://dataid.dbpedia.org/ns/core#SimpleStatement">
    <rdfs:comment xml:lang="en">A SimpleStatement either a primitive literal containing unstructured text (see dataid:statement), or a web reference to a statment (using dct:references).&#xD;
	This class implements several classes of Dublin Core which are not further specified within DC.</rdfs:comment>
    <rdfs:isDefinedBy rdf:resource="http://dataid.dbpedia.org/ns/core#"/>
    <rdfs:label xml:lang="en">Simple Statement</rdfs:label>
    <rdfs:subClassOf rdf:resource="http://purl.org/dc/terms/ProvenanceStatement"/>
    <rdfs:subClassOf rdf:resource="http://purl.org/dc/terms/RightsStatement"/>
    <rdfs:subClassOf rdf:resource="http://purl.org/dc/terms/Standard"/>
    <rdfs:subClassOf rdf:resource="http://www.essepuntato.it/2010/06/literalreification/Literal"/>
    <rdfs:subClassOf>
      <owl:Restriction>
        <owl:allValuesFrom rdf:resource="http://xmlns.com/foaf/0.1/Document"/>
        <owl:onProperty rdf:resource="http://purl.org/dc/terms/references"/>
      </owl:Restriction>
    </rdfs:subClassOf>
  </owl:Class>
  <owl:Class rdf:about="http://dataid.dbpedia.org/ns/core#SingleFile">
    <rdfs:comment xml:lang="en">A single data dump file representing the whole dataset, in a certain format/serialization.</rdfs:comment>
    <rdfs:isDefinedBy rdf:resource="http://dataid.dbpedia.org/ns/core#"/>
    <rdfs:label xml:lang="en">Single File</rdfs:label>
    <rdfs:subClassOf rdf:resource="http://dataid.dbpedia.org/ns/core#Distribution"/>
  </owl:Class>
  <owl:NamedIndividual rdf:about="http://dataid.dbpedia.org/ns/core#UpdateDataId">
    <rdf:type rdf:resource="http://dataid.dbpedia.org/ns/core#ResponsibleAction"/>
    <rdfs:comment xml:lang="en">The responsibility to update dataset metadata.</rdfs:comment>
    <rdfs:isDefinedBy rdf:resource="http://dataid.dbpedia.org/ns/core#"/>
    <rdfs:label xml:lang="en">update DataId</rdfs:label>
    <skos:broader rdf:resource="http://dataid.dbpedia.org/ns/core#AllResponsibilities"/>
    <skos:inScheme rdf:resource="http://dataid.dbpedia.org/ns/core#AuthorizedActionScheme"/>
    <skos:prefLabel xml:lang="en">update DataId</skos:prefLabel>
  </owl:NamedIndividual>
  <owl:ObjectProperty rdf:about="http://dataid.dbpedia.org/ns/core#accessProcedure">
    <rdfs:comment xml:lang="en">Describes the steps which have to be taken to gain access to the described data at the location of a Distribution (e.g. register an account to gain dct:accessRights).</rdfs:comment>
    <rdfs:domain rdf:resource="http://dataid.dbpedia.org/ns/core#Distribution"/>
    <rdfs:isDefinedBy rdf:resource="http://dataid.dbpedia.org/ns/core#"/>
    <rdfs:label xml:lang="en">access procedure</rdfs:label>
    <rdfs:range rdf:resource="http://dataid.dbpedia.org/ns/core#SimpleStatement"/>
  </owl:ObjectProperty>
  <owl:ObjectProperty rdf:about="http://dataid.dbpedia.org/ns/core#allowsFor">
    <rdfs:comment xml:lang="en">An dataid:AgentRole allows an agent to execute certain AuthorizedActions.</rdfs:comment>
    <rdfs:domain rdf:resource="http://dataid.dbpedia.org/ns/core#AgentRole"/>
    <rdfs:isDefinedBy rdf:resource="http://dataid.dbpedia.org/ns/core#"/>
    <rdfs:label xml:lang="en">allows for</rdfs:label>
    <rdfs:range rdf:resource="http://dataid.dbpedia.org/ns/core#AuthorizedAction"/>
  </owl:ObjectProperty>
  <owl:ObjectProperty rdf:about="http://dataid.dbpedia.org/ns/core#associatedAgent">
    <rdfs:comment xml:lang="en">An agent which is generally connected to the dataset, their exact function in regard to the Entity has to be specified by the qualification dataid:Authorization.</rdfs:comment>
    <rdfs:domain rdf:resource="http://www.w3.org/ns/prov#Entity"/>
    <rdfs:isDefinedBy rdf:resource="http://dataid.dbpedia.org/ns/core#"/>
    <rdfs:label xml:lang="en">associated agent</rdfs:label>
    <rdfs:range rdf:resource="http://dataid.dbpedia.org/ns/core#Agent"/>
    <rdfs:subPropertyOf rdf:resource="http://www.w3.org/ns/prov#wasAttributedTo"/>
    <owl:propertyChainAxiom>
      <rdf:Description>
        <rdf:first rdf:resource="http://dataid.dbpedia.org/ns/core#underAuthorization"/>
        <rdf:rest>
          <rdf:Description>
            <rdf:first rdf:resource="http://dataid.dbpedia.org/ns/core#authorizedAgent"/>
            <rdf:rest rdf:resource="http://www.w3.org/1999/02/22-rdf-syntax-ns#nil"/>
          </rdf:Description>
        </rdf:rest>
      </rdf:Description>
    </owl:propertyChainAxiom>
  </owl:ObjectProperty>
  <owl:ObjectProperty rdf:about="http://dataid.dbpedia.org/ns/core#authorityAgentRole">
    <rdfs:comment xml:lang="en">Provides a role an Agent fills out in the scope provided by the dataid:Authorization, thereby allowing for certain AuthorizedActions an agent can execute.</rdfs:comment>
    <rdfs:domain rdf:resource="http://www.w3.org/ns/prov#AgentInfluence"/>
    <rdfs:isDefinedBy rdf:resource="http://dataid.dbpedia.org/ns/core#"/>
    <rdfs:label xml:lang="en">authority agent role</rdfs:label>
    <rdfs:range rdf:resource="http://dataid.dbpedia.org/ns/core#AgentRole"/>
    <rdfs:subPropertyOf rdf:resource="http://www.w3.org/ns/prov#hadRole"/>
  </owl:ObjectProperty>
  <owl:ObjectProperty rdf:about="http://dataid.dbpedia.org/ns/core#authoritySubChain1">
    <rdfs:comment xml:lang="en">This sub-property of dataid:authorizedFor provides a property chain axiom, extending the reach of dataid:authorizedFor to other entities.</rdfs:comment>
    <rdfs:isDefinedBy rdf:resource="http://dataid.dbpedia.org/ns/core#"/>
    <rdfs:subPropertyOf rdf:resource="http://dataid.dbpedia.org/ns/core#authorizedFor"/>
    <owl:propertyChainAxiom>
      <rdf:Description>
        <rdf:first rdf:resource="http://dataid.dbpedia.org/ns/core#authorizedFor"/>
        <rdf:rest>
          <rdf:Description>
            <rdf:first rdf:resource="http://xmlns.com/foaf/0.1/primaryTopic"/>
            <rdf:rest>
              <rdf:Description>
                <rdf:first rdf:resource="http://dataid.dbpedia.org/ns/core#transitiveSubset"/>
                <rdf:rest>
                  <rdf:Description>
                    <rdf:first rdf:resource="http://www.w3.org/ns/dcat#distribution"/>
                    <rdf:rest rdf:resource="http://www.w3.org/1999/02/22-rdf-syntax-ns#nil"/>
                  </rdf:Description>
                </rdf:rest>
              </rdf:Description>
            </rdf:rest>
          </rdf:Description>
        </rdf:rest>
      </rdf:Description>
    </owl:propertyChainAxiom>
  </owl:ObjectProperty>
  <owl:ObjectProperty rdf:about="http://dataid.dbpedia.org/ns/core#authoritySubChain2">
    <rdfs:comment xml:lang="en">This sub-property of dataid:authorizedFor provides a property chain axiom, extending the reach of dataid:authorizedFor to other entities.</rdfs:comment>
    <rdfs:isDefinedBy rdf:resource="http://dataid.dbpedia.org/ns/core#"/>
    <rdfs:subPropertyOf rdf:resource="http://dataid.dbpedia.org/ns/core#authorizedFor"/>
    <owl:propertyChainAxiom>
      <rdf:Description>
        <rdf:first rdf:resource="http://dataid.dbpedia.org/ns/core#authorizedFor"/>
        <rdf:rest>
          <rdf:Description>
            <rdf:first rdf:resource="http://xmlns.com/foaf/0.1/primaryTopic"/>
            <rdf:rest>
              <rdf:Description>
                <rdf:first rdf:resource="http://www.w3.org/ns/dcat#distribution"/>
                <rdf:rest rdf:resource="http://www.w3.org/1999/02/22-rdf-syntax-ns#nil"/>
              </rdf:Description>
            </rdf:rest>
          </rdf:Description>
        </rdf:rest>
      </rdf:Description>
    </owl:propertyChainAxiom>
  </owl:ObjectProperty>
  <owl:ObjectProperty rdf:about="http://dataid.dbpedia.org/ns/core#authoritySubChain3">
    <rdfs:comment xml:lang="en">This sub-property of dataid:authorizedFor provides a property chain axiom, extending the reach of dataid:authorizedFor to other entities.</rdfs:comment>
    <rdfs:isDefinedBy rdf:resource="http://dataid.dbpedia.org/ns/core#"/>
    <rdfs:subPropertyOf rdf:resource="http://dataid.dbpedia.org/ns/core#authorizedFor"/>
    <owl:propertyChainAxiom>
      <rdf:Description>
        <rdf:first rdf:resource="http://dataid.dbpedia.org/ns/core#authorizedFor"/>
        <rdf:rest>
          <rdf:Description>
            <rdf:first rdf:resource="http://dataid.dbpedia.org/ns/core#transitiveSubset"/>
            <rdf:rest>
              <rdf:Description>
                <rdf:first rdf:resource="http://www.w3.org/ns/dcat#distribution"/>
                <rdf:rest rdf:resource="http://www.w3.org/1999/02/22-rdf-syntax-ns#nil"/>
              </rdf:Description>
            </rdf:rest>
          </rdf:Description>
        </rdf:rest>
      </rdf:Description>
    </owl:propertyChainAxiom>
  </owl:ObjectProperty>
  <owl:ObjectProperty rdf:about="http://dataid.dbpedia.org/ns/core#authoritySubChain4">
    <rdfs:comment xml:lang="en">This sub-property of dataid:authorizedFor provides a property chain axiom, extending the reach of dataid:authorizedFor to other entities.</rdfs:comment>
    <rdfs:isDefinedBy rdf:resource="http://dataid.dbpedia.org/ns/core#"/>
    <rdfs:subPropertyOf rdf:resource="http://dataid.dbpedia.org/ns/core#authorizedFor"/>
    <owl:propertyChainAxiom>
      <rdf:Description>
        <rdf:first rdf:resource="http://dataid.dbpedia.org/ns/core#authorizedFor"/>
        <rdf:rest>
          <rdf:Description>
            <rdf:first rdf:resource="http://dataid.dbpedia.org/ns/core#transitiveSubset"/>
            <rdf:rest rdf:resource="http://www.w3.org/1999/02/22-rdf-syntax-ns#nil"/>
          </rdf:Description>
        </rdf:rest>
      </rdf:Description>
    </owl:propertyChainAxiom>
  </owl:ObjectProperty>
  <owl:ObjectProperty rdf:about="http://dataid.dbpedia.org/ns/core#authoritySubChain5">
    <rdfs:comment xml:lang="en">This sub-property of dataid:authorizedFor provides a property chain axiom, extending the reach of dataid:authorizedFor to other entities.</rdfs:comment>
    <rdfs:isDefinedBy rdf:resource="http://dataid.dbpedia.org/ns/core#"/>
    <rdfs:subPropertyOf rdf:resource="http://dataid.dbpedia.org/ns/core#authorizedFor"/>
    <owl:propertyChainAxiom>
      <rdf:Description>
        <rdf:first rdf:resource="http://dataid.dbpedia.org/ns/core#authorizedFor"/>
        <rdf:rest>
          <rdf:Description>
            <rdf:first rdf:resource="http://xmlns.com/foaf/0.1/primaryTopic"/>
            <rdf:rest rdf:resource="http://www.w3.org/1999/02/22-rdf-syntax-ns#nil"/>
          </rdf:Description>
        </rdf:rest>
      </rdf:Description>
    </owl:propertyChainAxiom>
  </owl:ObjectProperty>
  <owl:ObjectProperty rdf:about="http://dataid.dbpedia.org/ns/core#authoritySubChain6">
    <rdfs:comment xml:lang="en">This sub-property of dataid:authorizedFor provides a property chain axiom, extending the reach of dataid:authorizedFor to other entities.</rdfs:comment>
    <rdfs:isDefinedBy rdf:resource="http://dataid.dbpedia.org/ns/core#"/>
    <rdfs:subPropertyOf rdf:resource="http://dataid.dbpedia.org/ns/core#authorizedFor"/>
    <owl:propertyChainAxiom>
      <rdf:Description>
        <rdf:first rdf:resource="http://dataid.dbpedia.org/ns/core#authorizedFor"/>
        <rdf:rest>
          <rdf:Description>
            <rdf:first rdf:resource="http://www.w3.org/ns/dcat#distribution"/>
            <rdf:rest rdf:resource="http://www.w3.org/1999/02/22-rdf-syntax-ns#nil"/>
          </rdf:Description>
        </rdf:rest>
      </rdf:Description>
    </owl:propertyChainAxiom>
  </owl:ObjectProperty>
  <owl:ObjectProperty rdf:about="http://dataid.dbpedia.org/ns/core#authoritySubChain7">
    <rdfs:comment xml:lang="en">This sub-property of dataid:authorizedFor provides a property chain axiom, extending the reach of dataid:authorizedFor to other entities.</rdfs:comment>
    <rdfs:isDefinedBy rdf:resource="http://dataid.dbpedia.org/ns/core#"/>
    <rdfs:subPropertyOf rdf:resource="http://dataid.dbpedia.org/ns/core#authorizedFor"/>
    <owl:propertyChainAxiom>
      <rdf:Description>
        <rdf:first rdf:resource="http://dataid.dbpedia.org/ns/core#authorizedFor"/>
        <rdf:rest>
          <rdf:Description>
            <rdf:first rdf:resource="http://xmlns.com/foaf/0.1/primaryTopic"/>
            <rdf:rest>
              <rdf:Description>
                <rdf:first rdf:resource="http://dataid.dbpedia.org/ns/core#transitiveSubset"/>
                <rdf:rest rdf:resource="http://www.w3.org/1999/02/22-rdf-syntax-ns#nil"/>
              </rdf:Description>
            </rdf:rest>
          </rdf:Description>
        </rdf:rest>
      </rdf:Description>
    </owl:propertyChainAxiom>
  </owl:ObjectProperty>
  <owl:ObjectProperty rdf:about="http://dataid.dbpedia.org/ns/core#authorizedAction">
    <rdfs:comment xml:lang="en">Points out AuthorizedActions, Agents are allowed to execute under a given dataid:Authorization (and its chosen AgentRoles).</rdfs:comment>
    <rdfs:domain rdf:resource="http://www.w3.org/ns/prov#AgentInfluence"/>
    <rdfs:isDefinedBy rdf:resource="http://dataid.dbpedia.org/ns/core#"/>
    <rdfs:label xml:lang="en">authorized action</rdfs:label>
    <rdfs:range rdf:resource="http://dataid.dbpedia.org/ns/core#AuthorizedAction"/>
    <owl:propertyChainAxiom>
      <rdf:Description>
        <rdf:first rdf:resource="http://dataid.dbpedia.org/ns/core#authorityAgentRole"/>
        <rdf:rest>
          <rdf:Description>
            <rdf:first rdf:resource="http://dataid.dbpedia.org/ns/core#allowsFor"/>
            <rdf:rest rdf:resource="http://www.w3.org/1999/02/22-rdf-syntax-ns#nil"/>
          </rdf:Description>
        </rdf:rest>
      </rdf:Description>
    </owl:propertyChainAxiom>
  </owl:ObjectProperty>
  <owl:ObjectProperty rdf:about="http://dataid.dbpedia.org/ns/core#authorizedAgent">
    <rdfs:comment xml:lang="en">Points out an Agent which holds the rights granted by a dataid:Authorization (e.g. to modify the metadata of a Dataset).</rdfs:comment>
    <rdfs:domain rdf:resource="http://www.w3.org/ns/prov#AgentInfluence"/>
    <rdfs:isDefinedBy rdf:resource="http://dataid.dbpedia.org/ns/core#"/>
    <rdfs:label xml:lang="en">authorized agent</rdfs:label>
    <rdfs:range rdf:resource="http://dataid.dbpedia.org/ns/core#Agent"/>
    <rdfs:subPropertyOf rdf:resource="http://www.w3.org/ns/prov#agent"/>
  </owl:ObjectProperty>
  <owl:ObjectProperty rdf:about="http://dataid.dbpedia.org/ns/core#authorizedFor">
    <rdfs:comment xml:lang="en">Defines the scope of a dataid:Authorization. An Agent has the right to execute AuthorizedActions for all Entities of this scope. &#xD;
The property chain axioms in its subproperties define how the scope of an dataid:Authorization is spread to other Entities.</rdfs:comment>
    <rdfs:domain rdf:resource="http://dataid.dbpedia.org/ns/core#Authorization"/>
    <rdfs:isDefinedBy rdf:resource="http://dataid.dbpedia.org/ns/core#"/>
    <rdfs:label xml:lang="en">authorized for</rdfs:label>
    <rdfs:range rdf:resource="http://www.w3.org/ns/prov#Entity"/>
  </owl:ObjectProperty>
  <owl:ObjectProperty rdf:about="http://dataid.dbpedia.org/ns/core#checksum">
    <rdfs:comment xml:lang="en">The Checksum value allows the contents of a file to be authenticated, since it shifts even with small changes to the file.</rdfs:comment>
    <rdfs:domain rdf:resource="http://dataid.dbpedia.org/ns/core#Distribution"/>
    <rdfs:isDefinedBy rdf:resource="http://dataid.dbpedia.org/ns/core#"/>
    <rdfs:label xml:lang="en">checksum</rdfs:label>
    <rdfs:range rdf:resource="http://spdx.org/rdf/terms/#Checksum"/>
  </owl:ObjectProperty>
  <owl:ObjectProperty rdf:about="http://dataid.dbpedia.org/ns/core#dataDescription">
    <rdfs:comment xml:lang="en">Provides a general description of the data represented by this dataset.</rdfs:comment>
    <rdfs:domain rdf:resource="http://dataid.dbpedia.org/ns/core#Dataset"/>
    <rdfs:isDefinedBy rdf:resource="http://dataid.dbpedia.org/ns/dmp#"/>
    <rdfs:label xml:lang="en">data description</rdfs:label>
    <rdfs:range rdf:resource="http://dataid.dbpedia.org/ns/core#SimpleStatement"/>
  </owl:ObjectProperty>
  <owl:ObjectProperty rdf:about="http://dataid.dbpedia.org/ns/core#growth">
    <rdfs:comment xml:lang="en">Indication of what size the approximated end volume of the data is.</rdfs:comment>
    <rdfs:domain rdf:resource="http://dataid.dbpedia.org/ns/core#Dataset"/>
    <rdfs:isDefinedBy rdf:resource="http://dataid.dbpedia.org/ns/dmp#"/>
    <rdfs:label xml:lang="en">growth</rdfs:label>
    <rdfs:range rdf:resource="http://dataid.dbpedia.org/ns/core#SimpleStatement"/>
  </owl:ObjectProperty>
  <owl:ObjectProperty rdf:about="http://dataid.dbpedia.org/ns/core#hasAuthorization">
    <rdfs:comment xml:lang="en">Provides an dataid:Agent with the dataid:Authorization for a given scope of Entities (e.g. Dataset, Distribution etc.), granting rights to certain AuthorizedActions.</rdfs:comment>
    <rdfs:isDefinedBy rdf:resource="http://dataid.dbpedia.org/ns/core#"/>
    <rdfs:label xml:lang="en">has authorization</rdfs:label>
    <owl:inverseOf rdf:resource="http://dataid.dbpedia.org/ns/core#authorizedAgent"/>
  </owl:ObjectProperty>
  <owl:InverseFunctionalProperty rdf:about="http://dataid.dbpedia.org/ns/core#identifier">
    <rdfs:comment xml:lang="en">An unique identifier for an Agent or Entity (for other, non DataID related identifiers).</rdfs:comment>
    <rdfs:isDefinedBy rdf:resource="http://dataid.dbpedia.org/ns/core#"/>
    <rdfs:label xml:lang="en">identifier</rdfs:label>
    <rdfs:range rdf:resource="http://purl.org/spar/datacite/Identifier"/>
    <rdfs:subPropertyOf rdf:resource="http://purl.org/spar/datacite/hasIdentifier"/>
    <rdfs:subPropertyOf rdf:resource="http://xmlns.com/foaf/0.1/isPrimaryTopicOf"/>
  </owl:InverseFunctionalProperty>
  <owl:ObjectProperty rdf:about="http://dataid.dbpedia.org/ns/core#identifierScheme">
    <rdfs:comment xml:lang="en">Points out which scheme of identifiers is used to uniquely identify resources inside a Dataset.</rdfs:comment>
    <rdfs:domain rdf:resource="http://dataid.dbpedia.org/ns/core#Dataset"/>
    <rdfs:isDefinedBy rdf:resource="http://dataid.dbpedia.org/ns/core#"/>
    <rdfs:label xml:lang="en">identifier scheme</rdfs:label>
    <rdfs:range rdf:resource="http://purl.org/spar/datacite/IdentifierScheme"/>
  </owl:ObjectProperty>
  <owl:ObjectProperty rdf:about="http://dataid.dbpedia.org/ns/core#inCatalog">
    <rdfs:comment xml:lang="en">The inverse property of dcat:record, pointing back to the dcat:Catalog.</rdfs:comment>
    <rdfs:domain rdf:resource="http://dataid.dbpedia.org/ns/core#DataId"/>
    <rdfs:isDefinedBy rdf:resource="http://dataid.dbpedia.org/ns/core#"/>
    <rdfs:label xml:lang="en">in catalog</rdfs:label>
    <rdfs:range rdf:resource="http://www.w3.org/ns/dcat#Catalog"/>
    <owl:inverseOf rdf:resource="http://www.w3.org/ns/dcat#record"/>
  </owl:ObjectProperty>
  <owl:ObjectProperty rdf:about="http://dataid.dbpedia.org/ns/core#innerMediaType">
    <rdf:type rdf:resource="http://www.w3.org/2002/07/owl#FunctionalProperty"/>
    <rdfs:comment xml:lang="en">Points out the MediaType of the (compressed) file inside another file (relevant for archive files).</rdfs:comment>
    <rdfs:domain rdf:resource="http://dataid.dbpedia.org/ns/core#MediaType"/>
    <rdfs:isDefinedBy rdf:resource="http://dataid.dbpedia.org/ns/core#"/>
    <rdfs:label xml:lang="en">inner media type</rdfs:label>
    <rdfs:range rdf:resource="http://dataid.dbpedia.org/ns/core#MediaType"/>
    <rdfs:subPropertyOf rdf:resource="http://www.w3.org/ns/dcat#mediaType"/>
  </owl:ObjectProperty>
  <owl:ObjectProperty rdf:about="http://dataid.dbpedia.org/ns/core#isDistributionOf">
    <rdfs:comment xml:lang="en">Inverse property of dcat:distribution, linking a Distribution to a Dataset</rdfs:comment>
    <rdfs:domain rdf:resource="http://dataid.dbpedia.org/ns/core#Distribution"/>
    <rdfs:isDefinedBy rdf:resource="http://dataid.dbpedia.org/ns/core#"/>
    <rdfs:label xml:lang="en">is distribution of</rdfs:label>
    <rdfs:range rdf:resource="http://dataid.dbpedia.org/ns/core#Dataset"/>
    <owl:inverseOf rdf:resource="http://www.w3.org/ns/dcat#distribution"/>
  </owl:ObjectProperty>
  <owl:DatatypeProperty rdf:about="http://dataid.dbpedia.org/ns/core#isInheritable">
    <rdf:type rdf:resource="http://www.w3.org/2002/07/owl#FunctionalProperty"/>
    <rdfs:comment xml:lang="en">Indicated whether this dataid:Authorization will be valid after an update to the DataID or a scope element (by default this property should be 'true').</rdfs:comment>
    <rdfs:domain rdf:resource="http://dataid.dbpedia.org/ns/core#Authorization"/>
    <rdfs:isDefinedBy rdf:resource="http://dataid.dbpedia.org/ns/core#"/>
    <rdfs:label xml:lang="en">is inheritable</rdfs:label>
    <rdfs:range rdf:resource="http://www.w3.org/2001/XMLSchema#boolean"/>
  </owl:DatatypeProperty>
  <owl:ObjectProperty rdf:about="http://dataid.dbpedia.org/ns/core#latestVersion">
    <rdfs:comment xml:lang="en">Latest version of a DataID/Dataset/Distribution.</rdfs:comment>
    <rdfs:domain rdf:resource="http://www.w3.org/ns/prov#Entity"/>
    <rdfs:isDefinedBy rdf:resource="http://dataid.dbpedia.org/ns/core#"/>
    <rdfs:label xml:lang="en">latest version</rdfs:label>
    <rdfs:range rdf:resource="http://www.w3.org/ns/prov#Entity"/>
  </owl:ObjectProperty>
  <owl:ObjectProperty rdf:about="http://dataid.dbpedia.org/ns/core#needsSpecialAuthorization">
    <rdfs:comment xml:lang="en">Points out a dataid:Authorization which grants some degree of authority over this resource to the exclusion of other dataid:Authorizations which are not specified with this property.</rdfs:comment>
    <rdfs:domain rdf:resource="http://www.w3.org/ns/prov#Entity"/>
    <rdfs:isDefinedBy rdf:resource="http://dataid.dbpedia.org/ns/core#"/>
    <rdfs:label xml:lang="en">needs special authorization</rdfs:label>
    <rdfs:range rdf:resource="http://dataid.dbpedia.org/ns/core#Authorization"/>
    <rdfs:subPropertyOf rdf:resource="http://dataid.dbpedia.org/ns/core#underAuthorization"/>
  </owl:ObjectProperty>
  <owl:ObjectProperty rdf:about="http://dataid.dbpedia.org/ns/core#nextVersion">
    <rdfs:comment xml:lang="en">Next version of a DataID/Dataset/Distribution.</rdfs:comment>
    <rdfs:domain rdf:resource="http://www.w3.org/ns/prov#Entity"/>
    <rdfs:isDefinedBy rdf:resource="http://dataid.dbpedia.org/ns/core#"/>
    <rdfs:label xml:lang="en">next version</rdfs:label>
    <rdfs:range rdf:resource="http://www.w3.org/ns/prov#Entity"/>
  </owl:ObjectProperty>
  <owl:ObjectProperty rdf:about="http://dataid.dbpedia.org/ns/core#openness">
    <rdfs:comment xml:lang="en">General description of how data will be shared. &#xD;
	For example: embargo periods (if any), outlines of technical mechanisms for dissemination or a definition of whether access will be widely open or restricted to specific groups. &#xD;
	In case the dataset cannot be shared, the reasons for this should be mentioned (e.g. ethical, rules of personal data, intellectual property, commercial, privacy-related, security-related).</rdfs:comment>
    <rdfs:domain rdf:resource="http://dataid.dbpedia.org/ns/core#Dataset"/>
    <rdfs:isDefinedBy rdf:resource="http://dataid.dbpedia.org/ns/dmp#"/>
    <rdfs:label xml:lang="en">openness</rdfs:label>
    <rdfs:range rdf:resource="http://dataid.dbpedia.org/ns/core#SimpleStatement"/>
  </owl:ObjectProperty>
  <owl:ObjectProperty rdf:about="http://dataid.dbpedia.org/ns/core#preview">
    <rdfs:comment xml:lang="en">Provides the url of a short preview of the data provided by a distribution, helpful when conveying type and format of the data provided.</rdfs:comment>
    <rdfs:domain rdf:resource="http://dataid.dbpedia.org/ns/core#Distribution"/>
    <rdfs:isDefinedBy rdf:resource="http://dataid.dbpedia.org/ns/core#"/>
    <rdfs:label xml:lang="en">preview</rdfs:label>
    <rdfs:range rdf:resource="http://xmlns.com/foaf/0.1/Document"/>
  </owl:ObjectProperty>
  <owl:ObjectProperty rdf:about="http://dataid.dbpedia.org/ns/core#previousVersion">
    <rdfs:comment xml:lang="en">Previous version of a DataID/Dataset/Distribution.</rdfs:comment>
    <rdfs:domain rdf:resource="http://www.w3.org/ns/prov#Entity"/>
    <rdfs:isDefinedBy rdf:resource="http://dataid.dbpedia.org/ns/core#"/>
    <rdfs:label xml:lang="en">previous version</rdfs:label>
    <rdfs:range rdf:resource="http://www.w3.org/ns/prov#Entity"/>
  </owl:ObjectProperty>
  <owl:ObjectProperty rdf:about="http://dataid.dbpedia.org/ns/core#reuseAndIntegration">
    <rdfs:comment xml:lang="en">Information on the possibilities for integration and reuse of the dataset.</rdfs:comment>
    <rdfs:domain rdf:resource="http://dataid.dbpedia.org/ns/core#Dataset"/>
    <rdfs:isDefinedBy rdf:resource="http://dataid.dbpedia.org/ns/dmp#"/>
    <rdfs:label xml:lang="en">reuse and integration</rdfs:label>
    <rdfs:range rdf:resource="http://dataid.dbpedia.org/ns/core#SimpleStatement"/>
  </owl:ObjectProperty>
  <owl:ObjectProperty rdf:about="http://dataid.dbpedia.org/ns/core#similarData">
    <rdfs:comment xml:lang="en">Information on the existence (or not) of similar data (see also dataid:similarDataset).</rdfs:comment>
    <rdfs:domain rdf:resource="http://dataid.dbpedia.org/ns/core#Dataset"/>
    <rdfs:isDefinedBy rdf:resource="http://dataid.dbpedia.org/ns/dmp#"/>
    <rdfs:label xml:lang="en">similar data</rdfs:label>
    <rdfs:range rdf:resource="http://dataid.dbpedia.org/ns/core#SimpleStatement"/>
  </owl:ObjectProperty>
  <owl:ObjectProperty rdf:about="http://dataid.dbpedia.org/ns/core#similarDataset">
    <rdfs:comment xml:lang="en">Points to other dataset containing related data.</rdfs:comment>
    <rdfs:domain rdf:resource="http://dataid.dbpedia.org/ns/core#Dataset"/>
    <rdfs:isDefinedBy rdf:resource="http://dataid.dbpedia.org/ns/core#"/>
    <rdfs:label xml:lang="en">similar dataset</rdfs:label>
    <rdfs:range rdf:resource="http://www.w3.org/ns/dcat#Dataset"/>
    <rdfs:subPropertyOf rdf:resource="http://purl.org/dc/terms/relation"/>
  </owl:ObjectProperty>
  <owl:ObjectProperty rdf:about="http://dataid.dbpedia.org/ns/core#softwareRquirement">
    <rdfs:comment xml:lang="en">Software needed to access the data provided via this Distribution or otherwise relevant for consuming the data.</rdfs:comment>
    <rdfs:domain rdf:resource="http://dataid.dbpedia.org/ns/core#Distribution"/>
    <rdfs:isDefinedBy rdf:resource="http://dataid.dbpedia.org/ns/core#"/>
    <rdfs:label xml:lang="en">software requirement</rdfs:label>
    <rdfs:range rdf:resource="http://dataid.dbpedia.org/ns/core#SimpleStatement"/>
  </owl:ObjectProperty>
  <owl:DatatypeProperty rdf:about="http://dataid.dbpedia.org/ns/core#statement">
    <rdfs:comment xml:lang="en">An actual textual statement (or string).</rdfs:comment>
    <rdfs:isDefinedBy rdf:resource="http://dataid.dbpedia.org/ns/core#"/>
    <rdfs:label xml:lang="en">statement</rdfs:label>
    <rdfs:range rdf:resource="http://www.w3.org/2000/01/rdf-schema#Literal"/>
    <rdfs:subPropertyOf rdf:resource="http://www.essepuntato.it/2010/06/literalreification/hasLiteralValue"/>
  </owl:DatatypeProperty>
  <owl:ObjectProperty rdf:about="http://dataid.dbpedia.org/ns/core#transitiveSubset">
    <rdf:type rdf:resource="http://www.w3.org/2002/07/owl#TransitiveProperty"/>
    <rdfs:comment xml:lang="en">Transitive super property of void:subset. This property is used to infer dataid:authorizedFor statements transitively over dataset hierarchies of arbitrary depth.</rdfs:comment>
    <rdfs:isDefinedBy rdf:resource="http://dataid.dbpedia.org/ns/core#"/>
    <rdfs:label xml:lang="en">transitive super property of void:subset</rdfs:label>
  </owl:ObjectProperty>
  <owl:DatatypeProperty rdf:about="http://dataid.dbpedia.org/ns/core#typeExtension">
    <rdfs:comment xml:lang="en">Lists file extensions commonly used with this mime type.</rdfs:comment>
    <rdfs:domain rdf:resource="http://dataid.dbpedia.org/ns/core#MediaType"/>
    <rdfs:isDefinedBy rdf:resource="http://dataid.dbpedia.org/ns/core#"/>
    <rdfs:label xml:lang="en">media type file extension</rdfs:label>
    <rdfs:range rdf:resource="http://www.w3.org/2000/01/rdf-schema#Literal"/>
  </owl:DatatypeProperty>
  <owl:DatatypeProperty rdf:about="http://dataid.dbpedia.org/ns/core#typeName">
    <rdfs:comment xml:lang="en">Names the MediaType described.</rdfs:comment>
    <rdfs:domain rdf:resource="http://dataid.dbpedia.org/ns/core#MediaType"/>
    <rdfs:isDefinedBy rdf:resource="http://dataid.dbpedia.org/ns/core#"/>
    <rdfs:label xml:lang="en">media type name</rdfs:label>
    <rdfs:range rdf:resource="http://www.w3.org/2000/01/rdf-schema#Literal"/>
  </owl:DatatypeProperty>
  <owl:ObjectProperty rdf:about="http://dataid.dbpedia.org/ns/core#typeReference">
    <rdfs:comment xml:lang="en">Refers to a standard document of the mime type described.</rdfs:comment>
    <rdfs:domain rdf:resource="http://dataid.dbpedia.org/ns/core#MediaType"/>
    <rdfs:isDefinedBy rdf:resource="http://dataid.dbpedia.org/ns/core#"/>
    <rdfs:label xml:lang="en">media type reference</rdfs:label>
    <rdfs:subPropertyOf rdf:resource="http://xmlns.com/foaf/0.1/page"/>
  </owl:ObjectProperty>
  <owl:DatatypeProperty rdf:about="http://dataid.dbpedia.org/ns/core#typeTemplate">
    <rdf:type rdf:resource="http://www.w3.org/2002/07/owl#FunctionalProperty"/>
    <rdfs:comment xml:lang="en">The template (or mime type string) of a MediaType.</rdfs:comment>
    <rdfs:domain rdf:resource="http://dataid.dbpedia.org/ns/core#MediaType"/>
    <rdfs:isDefinedBy rdf:resource="http://dataid.dbpedia.org/ns/core#"/>
    <rdfs:label xml:lang="en">media type template</rdfs:label>
    <rdfs:range rdf:resource="http://www.w3.org/2000/01/rdf-schema#Literal"/>
  </owl:DatatypeProperty>
  <owl:DatatypeProperty rdf:about="http://dataid.dbpedia.org/ns/core#uncompressedByteSize">
    <rdfs:comment xml:lang="en">Records the byte size of the uncompressed content of an archive file.</rdfs:comment>
    <rdfs:domain rdf:resource="http://dataid.dbpedia.org/ns/core#Distribution"/>
    <rdfs:isDefinedBy rdf:resource="http://dataid.dbpedia.org/ns/core#"/>
    <rdfs:label xml:lang="en">uncompressed byte size</rdfs:label>
    <rdfs:range rdf:resource="http://www.w3.org/2001/XMLSchema#integer"/>
    <rdfs:subPropertyOf rdf:resource="http://www.w3.org/ns/dcat#byteSize"/>
  </owl:DatatypeProperty>
  <owl:ObjectProperty rdf:about="http://dataid.dbpedia.org/ns/core#underAuthorization">
    <rdfs:comment xml:lang="en">Points out a dataid:Authorization which grants some degree of authority over this resource (inverse property of dataid:authorizedFor).</rdfs:comment>
    <rdfs:domain rdf:resource="http://www.w3.org/ns/prov#Entity"/>
    <rdfs:isDefinedBy rdf:resource="http://dataid.dbpedia.org/ns/core#"/>
    <rdfs:label xml:lang="en">under authorization</rdfs:label>
    <rdfs:range rdf:resource="http://dataid.dbpedia.org/ns/core#Authorization"/>
    <rdfs:subPropertyOf rdf:resource="http://www.w3.org/ns/prov#qualifiedAttribution"/>
    <owl:inverseOf rdf:resource="http://dataid.dbpedia.org/ns/core#authorizedFor"/>
  </owl:ObjectProperty>
  <owl:ObjectProperty rdf:about="http://dataid.dbpedia.org/ns/core#usefulness">
    <rdfs:comment xml:lang="en">Description of to whom the data could be useful, and whether it underpins a scientific publication.</rdfs:comment>
    <rdfs:domain rdf:resource="http://dataid.dbpedia.org/ns/core#Dataset"/>
    <rdfs:isDefinedBy rdf:resource="http://dataid.dbpedia.org/ns/dmp#"/>
    <rdfs:label xml:lang="en">usefulness</rdfs:label>
    <rdfs:range rdf:resource="http://dataid.dbpedia.org/ns/core#SimpleStatement"/>
  </owl:ObjectProperty>
  <owl:DatatypeProperty rdf:about="http://dataid.dbpedia.org/ns/core#validFrom">
    <rdf:type rdf:resource="http://www.w3.org/2002/07/owl#FunctionalProperty"/>
    <rdfs:comment xml:lang="en">The influence an agent has over an Entity is valid from a certain point in time.</rdfs:comment>
    <rdfs:domain rdf:resource="http://www.w3.org/ns/prov#AgentInfluence"/>
    <rdfs:isDefinedBy rdf:resource="http://dataid.dbpedia.org/ns/core#"/>
    <rdfs:label xml:lang="en">valid from</rdfs:label>
    <rdfs:range rdf:resource="http://www.w3.org/2001/XMLSchema#datetime"/>
  </owl:DatatypeProperty>
  <owl:DatatypeProperty rdf:about="http://dataid.dbpedia.org/ns/core#validUntil">
    <rdf:type rdf:resource="http://www.w3.org/2002/07/owl#FunctionalProperty"/>
    <rdfs:comment xml:lang="en">The influence an agent has over an Entity is valid until a certain point in time.</rdfs:comment>
    <rdfs:domain rdf:resource="http://www.w3.org/ns/prov#AgentInfluence"/>
    <rdfs:isDefinedBy rdf:resource="http://dataid.dbpedia.org/ns/core#"/>
    <rdfs:label xml:lang="en">valid until</rdfs:label>
    <rdfs:range rdf:resource="http://www.w3.org/2001/XMLSchema#datetime"/>
  </owl:DatatypeProperty>
  <rdf:Description rdf:about="http://rdfs.org/ns/void#subset">
    <rdfs:subPropertyOf rdf:resource="http://dataid.dbpedia.org/ns/core#transitiveSubset"/>
  </rdf:Description>
  <dataid:Agent rdf:about="http://wiki.dbpedia.org/Association/Persons/Freudenberg">
    <foaf:homepage rdf:resource="http://wiki.dbpedia.org/Association/Persons/Freudenberg"/>
    <foaf:mbox>freudenberg@informatik.uni-leipzig.de</foaf:mbox>
    <foaf:name>Markus Freudenberg</foaf:name>
  </dataid:Agent>
  <rdf:Description rdf:about="http://www.geonames.org/ontology#Feature">
    <rdfs:subClassOf rdf:resource="http://purl.org/dc/terms/Location"/>
  </rdf:Description>
  <rdf:Description rdf:about="http://www.w3.org/2006/time#Interval">
    <rdfs:subClassOf rdf:resource="http://purl.org/dc/terms/PeriodOfTime"/>
  </rdf:Description>
</rdf:RDF>
