### re3data.org controlled vocabularies ###

@prefix rdf: <http://www.w3.org/1999/02/22-rdf-syntax-ns#> .
@prefix rdfs: <http://www.w3.org/2000/01/rdf-schema#> .
@prefix owl: <http://www.w3.org/2002/07/owl#> .
@prefix dct: <http://purl.org/dc/terms/> .
@prefix xsd: <http://www.w3.org/2001/XMLSchema#> .
@prefix foaf: <http://xmlns.com/foaf/0.1/> . 
@prefix skos: <http://www.w3.org/2004/02/skos/core#> .
@prefix r3d: <http://www.re3data.org/schema/3-0#> .
@prefix datacite: <http://purl.org/spar/datacite/> .
@prefix vann: <http://purl.org/vocab/vann/> .
@prefix : <http://www.re3data.org/vocab/> .		#TODO define uri for vocabs

@base	<http://www.re3data.org/vocab/> .
 
<http://www.re3data.org/vocab>
    a owl:Ontology ;
    vann:preferredNamespaceUri "http://www.re3data.org/vocab/" ;		#TODO
    vann:preferredNamespacePrefix "r3voc" ;								#TODO
    owl:versionInfo "1.0.0" ; 
    dct:modified "2016-06-12" ;
    rdfs:comment "This ontology contains multiple controlled vocabularies of the re3data.org domain and accompanying concepts."@en ;		#todo
    rdfs:label "re3data controlled vocabularies"@en ;
	dct:license <http://purl.org/NET/rdflicense/cc-by4.0> ;#todo
	dct:publisher <http://re3data.org>	;
	owl:import	<http://www.re3data.org/vocab/common>	.
    
    
############### Publisher #################
<http://re3data.org>		#TODO change uri , mbox, name if necessary
	a                        foaf:Agent ;
	foaf:mbox                "someBeautifuleAddress@re3data.org" ;
	foaf:homepage			 <http://www.re3data.org>	;
	foaf:name                "re3data.org" .

############# r3d:RepoType ################
:RepositoryType 
	a	owl:Class, skos:ConceptScheme	;
	rdfs:subClassOf skos:Concept		;
	dct:title		"Repository Type vocabulary"@en	;
	rdfs:label		"repository type"@en	;
	dct:description	"The type of the RDR."@en	;		#TODO copied from schema doc 3.0 
	dct:modified	"12-07-2016"^^xsd:date	;	
	dct:publisher	<http://re3data.org>	;
	dct:hasVersion	<http://version/specification/you/can/look/up/on/the/web> ;	#TODO
	skos:prefLabel	"repository type"@en	;
	skos:altLabel	"TODO"@de	.
	
:Disciplinary
	a	:RepositoryType 	;
	dct:title	"disciplinary"@en ;
	rdfs:label "disciplinary"@en	;
	skos:prefLabel "disciplinary"@en	;
	skos:inScheme	:RepositoryType 	;
	skos:definition	"""This is a collection of research outputs with a common link to a
particular subject discipline. Subject repositories are likely to cover one
broad-based discipline, with contributors from many different
institutions supported by a variety of funders; the repositories
themselves are likely to be funded from one or more sources within the
subject community. Although for some subject repositories the funding
may be fragile, if they are of enough importance to the community
then funding crises are usually weathered"""@en	;
	skos:note	"TODO"@en .
	
:Governmental
	a	:RepositoryType 	;
	rdfs:label "governmental"@en	;
	skos:prefLabel "governmental"@en	;
	skos:inScheme	:RepositoryType 	;
	skos:definition	"""This is a collection of outputs from projects and programmes related to
governmental institutions. The repository is primarily supported by a
federal agency. These repositories are likely closed for external
contributions. """@en	;
	skos:note	"TODO"@en .
	
:Institutional
	a	:RepositoryType 	;
	rdfs:label "institutional"@en	;
	skos:prefLabel "institutional"@en	;
	skos:inScheme	:RepositoryType 	;
	skos:definition	""""This is a collection of research outputs with a common link to a
particular institution, usually by authorship. These repositories are
likely to cover more than one research discipline, to have funders in
many if not all the Research Councils and support communities who
have different approaches to research dissemination. Whether deposit
of content is mandatory is a decision that will be made by each
institution. The institutions may have many requirements for the
content of the repository, from open access dissemination, through
metrics, marketing to strategic planning. It is likely that many of these
processes in the past were undertaken through collection of
bibliographic information."""@en	;
	skos:note	"TODO"@en .
	
:Multidisciplinary
	a	:RepositoryType 	;
	rdfs:label "multidisciplinary"@en	;
	skos:prefLabel "multidisciplinary"@en	;
	skos:inScheme	:RepositoryType 	;
	skos:definition	"""This is a collection of research outputs serving multidisciplinary needs.
These repositories cover several research disciplines. Contributors from
many different institutions and communities are likely accepted."""@en	;
	skos:note	"TODO"@en .
	
:ProjectRelated
	a	:RepositoryType 	;
	rdfs:label "project-related"@en	;
	skos:prefLabel "project-related"@en	;
	skos:inScheme	:RepositoryType 	;
	skos:definition	"""This is a collection of research outputs with a specific focus on the
research data resulting from particular research projects. All
contributions must be linked to the particular project, mission, etc."""@en	;
	skos:note	"TODO"@en .
	
:OtherRepoTypes
	a	:RepositoryType 	;
	rdfs:label "other repository types"@en	;
	skos:prefLabel "other repository types"@en	;
	skos:inScheme	:RepositoryType 	;
	skos:definition	"A research data repository that is not one of the listed repository types, e.g. a funder repository."@en	;
	skos:note	"TODO"@en .
	
############# :ProviderType ################
:ProviderType
	a	owl:Class, skos:ConceptScheme	;
	rdfs:subClassOf skos:Concept	;
	dct:title		"Provider Type vocabulary"@en	;
	dct:description	"The type of the RDR."@en	;		#TODO copied from schema doc 3.0 
	dct:modified	"12-07-2016"^^xsd:date	;	
	dct:publisher	<http://re3data.org>	;
	dct:hasVersion	<http://version/specification/you/can/look/up/on/the/web> ;	#TODO
	rdfs:label	"provider type"@en ;
	skos:prefLabel	"provider type"@en ;
	skos:altLabel	"TODO"@de	;
	skos:note	"TODO"@en	.
	
:DataProvider
	a	:ProviderType	;
	rdfs:label "data provider"@en	;
	skos:prefLabel "dataProvider"@en	;
	skos:inScheme	:ProviderType	;
	skos:definition	"A research data repository is a data provider if it offers research data and its metadata (ideally exposing metadata via interfaces)."@en	;
	skos:note	"TODO"@en .
	
:ServiceProvider
	a	:ProviderType	;
	rdfs:label "service provider"@en	;
	skos:prefLabel "serviceProvider"@en	;
	skos:inScheme	:ProviderType	;
	skos:definition	"A research data repository is a service provider if it harvests the metadata of research data from data providers as a basis for building value-added services."@en	;
	skos:note	"TODO"@en .
	
############# :ResponsibilityType ################
:ResponsibilityType
	a	owl:Class, skos:ConceptScheme	;
	rdfs:subClassOf skos:Concept	;
	rdfs:label		"institution responsibility type vocabulary"@en ;
	dct:title		"institution responsibility type vocabulary"@en ;
	rdfs:label		"institution responsibility type"@en ;
	dct:description	"The type of the RDR."@en	;		#TODO copied from schema doc 3.0 
	dct:modified	"12-07-2016"^^xsd:date	;	
	dct:publisher	<http://re3data.org>	;
	dct:hasVersion	<http://version/specification/you/can/look/up/on/the/web> ;	#TODO
	skos:prefLabel	"institution responsibility type"@en ;
	skos:altLabel	"TODO"@de	;
	skos:note		"TODO"@en	.
	
:Funding
	a	:ResponsibilityType	;
	rdfs:label "funding"@en	;
	skos:prefLabel "funding"@en	;
	skos:inScheme	:ResponsibilityType	;
	skos:definition	"Funding responsibility refers to the institution that funds / funded the setup or running of the research data repository."@en	;
	skos:note	"TODO"@en .
	
:General
	a	:ResponsibilityType	;
	rdfs:label "general"@en	;
	skos:prefLabel "general"@en	;
	skos:inScheme	:ResponsibilityType	;
	skos:definition	"General responsibility refers to the institution that is generally responsible for providing services and content of the research data repository"@en	;
	skos:note	"TODO"@en .
	
:Main
	a	:ResponsibilityType	;
	rdfs:label "main"@en	;
	skos:prefLabel "main"@en	;
	skos:inScheme	:ResponsibilityType	;
	skos:definition	"Main responsibility refers to the leading institution operating and maintaining the research data repository."@en	;
	skos:note	"TODO"@en .
	
:Sponsoring
	a	:ResponsibilityType	;
	rdfs:label "sponsoring"@en	;
	skos:prefLabel "sponsoring"@en	;
	skos:inScheme	:ResponsibilityType	;
	skos:definition	"Sponsoring responsibility (in contrast to funding responsibility) refers to financial support of a research data repository in return for e.g. advertising on the website."@en	;
	skos:note	"TODO"@en .
	
:Technical
	a	:ResponsibilityType	;
	rdfs:label "technical"@en	;
	skos:prefLabel "technical"@en	;
	skos:inScheme	:ResponsibilityType	;
	skos:definition	"General responsibility refers to the institution that is responsible for the technical matters of the research data repository, e.g. hosting."@en	;
	skos:note	"TODO"@en .
	
:Commercial
	a	:ResponsibilityType	;
	rdfs:label "commercial"@en	;
	skos:prefLabel "commercial"@en	;
	skos:inScheme	:ResponsibilityType	;
	skos:definition	"A commercial institution is an institution that distributes surplus revenues as profit or dividends."@en	;
	skos:note	"TODO"@en .
	
:NonProfit
	a	:ResponsibilityType	;
	rdfs:label "non-profit"@en	;
	skos:prefLabel "non-profit"@en	;
	skos:inScheme	:ResponsibilityType	;
	skos:definition	"The institution does not aim at economic profits but at non-profit (e.g. social, cultural and academic) goals of its members."@en	;
	skos:note	"TODO"@en .
	
############# :ContentType ################
:ContentType		#TODO need the mappings to the current DFG scheme
	a	owl:Class, skos:ConceptScheme	;
	rdfs:subClassOf skos:Concept	;
	dct:title		"content type vocabulary"@en ;
	rdfs:label		"content type"@en ;
	dct:description	"The type of the RDR."@en	;		#TODO copied from schema doc 3.0 
	dct:modified	"12-07-2016"^^xsd:date	;	
	dct:publisher	<http://re3data.org>	;
	dct:hasVersion	<http://version/specification/you/can/look/up/on/the/web> ;	#TODO
	skos:prefLabel	"content type"@en ;
	skos:altLabel	"TODO"@de	;
	skos:note		"TODO"@en	.
	
:StandardOfficeDocuments 
	a	:ContentType	;
	rdfs:label "Standard office documents"@en	;
	skos:prefLabel "Standard office documents"@en	;
	skos:inScheme	:ContentType	;
	skos:note	"TODO"@en .
		
:NetworkbasedData 
	a	:ContentType	;
	rdfs:label "Networkbased data"@en	;
	skos:prefLabel "Networkbased data"@en	;
	skos:inScheme	:ContentType	;
	skos:note	"TODO"@en .
	
	#TODO add induviduals
		
############# :ApiType ################
:ApiType	
	a	owl:Class, skos:ConceptScheme	;
	rdfs:subClassOf skos:Concept	;
	rdfs:label	"API type vocabulary"@en ;
	skos:prefLabel	"API type vocabulary"@en ;
	skos:altLabel	"TODO"@de	;
	skos:note	"TODO"@en	.
	
	#TODO add induviduals
		
############# :InstitutionType ################
:InstitutionType
	a	owl:Class, skos:ConceptScheme	;
	rdfs:subClassOf skos:Concept	;
	rdfs:label	"institution type vocabulary"@en ;
	skos:prefLabel	"institution type vocabulary"@en ;
	skos:altLabel	"TODO"@de	;
	skos:note	"TODO"@en	.
	
	#TODO add induviduals
		
############# :AidSystem ################
:AidSystem
	a	owl:Class, skos:ConceptScheme	;
	rdfs:subClassOf skos:Concept	;
	rdfs:label	"AID system vocabulary"@en ;
	skos:prefLabel	"AID system vocabulary"@en ;
	skos:altLabel	"TODO"@de	;
	skos:note	"TODO"@en	.
	
	#TODO add induviduals
		
############# :PidSystem ################
:PidSystem
	a	owl:Class, skos:ConceptScheme	;
	rdfs:subClassOf skos:Concept	;
	rdfs:label	"PID system vocabulary"@en ;
	skos:prefLabel	"PID system vocabulary"@en ;
	skos:altLabel	"TODO"@de	;
	skos:note	"TODO"@en	.
	
	#TODO add induviduals
		
############# :CitationReference ################
:CitationReference
	a	owl:Class, skos:ConceptScheme	;
	rdfs:subClassOf skos:Concept	;
	rdfs:label	"Citation Reference vocabulary"@en ;
	skos:prefLabel	"Citation Reference vocabulary"@en ;
	skos:altLabel	"TODO"@de	;
	skos:note	"TODO"@en	.
	
	#TODO add induviduals
		
############# :AccessType ################
:AccessType
	a	owl:Class, skos:ConceptScheme	;
	rdfs:subClassOf skos:Concept	;
	rdfs:label	"Access Type vocabulary"@en ;
	skos:prefLabel	"Access Type vocabulary"@en ;
	skos:altLabel	"TODO"@de	;
	skos:note	"TODO"@en	.
	
	#TODO add induviduals
		
############# :AccessRestriction ################
:AccessRestriction
	a	owl:Class, skos:ConceptScheme	;
	rdfs:subClassOf skos:Concept	;
	rdfs:label	"Access Restriction vocabulary"@en ;
	skos:prefLabel	"Access Restriction vocabulary"@en ;
	skos:altLabel	"TODO"@de	;
	skos:note	"TODO"@en	.
	
	#TODO add induviduals
		
############# :PolicyType ################
:PolicyType
	a	owl:Class, skos:ConceptScheme	;
	rdfs:subClassOf skos:Concept	;
	rdfs:label	"Policy Type vocabulary"@en ;
	skos:prefLabel	"Policy Type vocabulary"@en ;
	skos:altLabel	"TODO"@de	;
	skos:note	"TODO"@en	.
	
	#TODO add induviduals
		
