@prefix rdf: <http://www.w3.org/1999/02/22-rdf-syntax-ns#> .
@prefix dataid: <http://dataid.dbpedia.org/ns/core#> .
@prefix acp: <http://dataid.dbpedia.org/ns/acp#> .
@prefix dcat: <http://www.w3.org/ns/dcat#> .
@prefix dct: <http://purl.org/dc/terms/> .
@prefix odrl: <http://www.w3.org/ns/odrl/2/> .
@prefix owl: <http://www.w3.org/2002/07/owl#> .
@prefix prov: <http://www.w3.org/ns/prov#> .
@prefix rdfs: <http://www.w3.org/2000/01/rdf-schema#> .
@prefix void: <http://rdfs.org/ns/void#> .
@prefix xml: <http://www.w3.org/XML/1998/namespace> .
@prefix xsd: <http://www.w3.org/2001/XMLSchema#> .
@prefix foaf: <http://xmlns.com/foaf/0.1/> . 
@prefix vann: <http://purl.org/vocab/vann/> .
@prefix dlo: <http://aligned-project.eu/ontologies/dlo#> .
@prefix dctype: <http://purl.org/dc/dcmitype/> .
@prefix org: <http://www.w3.org/ns/org#> .

acp:
    a owl:Ontology ;
    vann:preferredNamespaceUri "http://dataid.dbpedia.org/ns/acp#" ;
    vann:preferredNamespacePrefix "dataid-acp"^^xsd:string ;
    owl:versionInfo "1.0.0" ; 
    rdfs:comment "This mid-level extension to DataID provides detaild provenance information about (planned) activities related to datasets described by a DataID."@en ;
    rdfs:label "DataID"@en ;
    owl:imports dataid:, prov:, dlo:, org:.
    
############# classes ################

dataid:Dataset rdfs:subClassOf dlo:DataEntity.

dataid:Distribution rdfs:subClassOf dlo:DataEntity.

dataid:AgentRole rdfs:subClassOf org:Role.

acp:ActivityAssociation
	a	owl:Class;
    rdfs:isDefinedBy <http://dataid.dbpedia.org/ns/acp#> ;
    rdfs:label "activity association"@en ;
    rdfs:comment """A qualification of the prov:wasAssociatedWith property, relating this association of an activity with an agent to the role of that agent or a plan related to the activity. 
    Note: As a sub-class of prov:AgentInfluence, this class inherits multiple properties defined in the DataID ontoloy."""@en ;
	rdfs:subClassOf		prov:Association.
	
acp:PlanResponsibility
	a	owl:Class;
    rdfs:isDefinedBy <http://dataid.dbpedia.org/ns/acp#> ;
    rdfs:label "plan responsibility"@en ;
    rdfs:comment """A qualification of the dataid:associatedAgent property, relating a plan with an agent to the role of that agent and the subsequent acitions allowed. 
    Note: The roles are refering to roles in regard to a plan, not roles related to a specific activity (which are covered by the ActivityAssociation class)."""@en ;
	rdfs:subClassOf		prov:AgentInfluence .
	
acp:DataLifecyclePlan
	a	owl:Class;
    rdfs:isDefinedBy <http://dataid.dbpedia.org/ns/acp#> ;
    rdfs:label "data lifecycle plan"@en ;
    rdfs:comment """A specific sort of plan only concerned with lifecycle specific activities of a dataset."""@en ;
	rdfs:subClassOf		prov:Plan, 
	[
        a owl:Restriction ;
        owl:allValuesFrom dlo:DataLifecycleProcess ;
        owl:onProperty acp:planned
    ]	.
 	
acp:SupportingEntity
	a	owl:Class;
    rdfs:isDefinedBy <http://dataid.dbpedia.org/ns/acp#> ;
    rdfs:label "supporting entity"@en ;
    rdfs:comment """Describes entities which are no DataEntities (like Documentation or Software), but have some influence on activities or plans related to DataEntities."""@en ;
	rdfs:subClassOf		prov:Entity, dlo:DataArtifact .   
 	
acp:Document
	a	owl:Class;
    rdfs:isDefinedBy <http://dataid.dbpedia.org/ns/acp#> ;
    rdfs:label "supporting document"@en ;
    rdfs:comment """A document related to a dataset or activities which have influence on such a dataset."""@en ;
	rdfs:subClassOf		acp:SupportingEntity, dctype:Text .  
 	
acp:PhysicalObject
	a	owl:Class;
    rdfs:isDefinedBy <http://dataid.dbpedia.org/ns/acp#> ;
    rdfs:label "supporting physical object"@en ;
    rdfs:comment """A physical object (like a tool or specimen) related to a dataset or activities which have influence on such a dataset."""@en ;
	rdfs:subClassOf		acp:SupportingEntity, dctype:PhysicalObject.  
 	
acp:Software
	a	owl:Class;
    rdfs:isDefinedBy <http://dataid.dbpedia.org/ns/acp#> ;
    rdfs:label "supporting software"@en ;
    rdfs:comment """A software related to a dataset or activities which have influence on such a dataset."""@en ;
	rdfs:subClassOf		acp:SupportingEntity, dctype:Software .  
 	
acp:Service
	a	owl:Class;
    rdfs:isDefinedBy <http://dataid.dbpedia.org/ns/acp#> ;
    rdfs:label "supporting service"@en ;
    rdfs:comment """A service related to a dataset or activities which have influence on such a dataset."""@en ;
	rdfs:subClassOf		acp:SupportingEntity, dctype:Service .  
 	
acp:StandardOrMethod
	a	owl:Class;
    rdfs:isDefinedBy <http://dataid.dbpedia.org/ns/acp#> ;
    rdfs:label "supporting standard"@en ;
    rdfs:comment """A standard or established method related to a dataset or activities which have influence on such a dataset."""@en ;
	rdfs:subClassOf		acp:SupportingEntity, dct:Standard.  
	
############## properties ################
acp:augmentedBy
    a owl:ObjectProperty ;
    rdfs:subPropertyOf prov:used ;
    rdfs:isDefinedBy <http://dataid.dbpedia.org/ns/acp#> ;
    rdfs:comment 	"Specifies entities which had some supportive role in the execution of an activity."@en ;
    rdfs:domain 	prov:Activity ;
    rdfs:label 		"augmented by"@en ;
    rdfs:range  	acp:SupportingEntity .
	
acp:augments
    a owl:ObjectProperty ;
    owl:inverseOf acp:augmentedBy ;
    rdfs:isDefinedBy <http://dataid.dbpedia.org/ns/acp#> ;
    rdfs:comment 	"Specifies an activity in which's execution this entity which had some supportive role."@en ;
    rdfs:label 		"augments"@en .
    
acp:willResultIn
    a owl:ObjectProperty ;
    rdfs:isDefinedBy <http://dataid.dbpedia.org/ns/acp#> ;
    rdfs:comment 	"Describes the expected result of the planned activities."@en ;
    rdfs:domain 	prov:Plan ;
    rdfs:label 		"will result in"@en ;
    rdfs:range  	prov:Entity .
    
acp:hasSubPlan
    a owl:ObjectProperty ;
    rdfs:subPropertyOf prov:wasDerivedFrom ;
    rdfs:isDefinedBy <http://dataid.dbpedia.org/ns/acp#> ;
    rdfs:comment 	"Partitions the plan."@en ;
    rdfs:domain 	prov:Plan ;
    rdfs:label 		"has sub-plan"@en ;
    rdfs:range  	prov:Plan .
    
acp:planned
    a owl:ObjectProperty ;
    rdfs:subPropertyOf [
    	a owl:ObjectProperty;
    	owl:inverseOf prov:wasStartedBy
	];
    rdfs:isDefinedBy <http://dataid.dbpedia.org/ns/acp#> ;
    rdfs:comment 	"Points out the activities planned, which make up the plan."@en ;
    rdfs:domain 	prov:Plan ;
    rdfs:label 		"planned"@en ;
    rdfs:range  	prov:Activity .
    
acp:planResponsibility
    a owl:ObjectProperty ;
    rdfs:subPropertyOf dataid:underAuthorization ;
    rdfs:isDefinedBy <http://dataid.dbpedia.org/ns/acp#> ;
    rdfs:comment 	"Points out agents responsible for this plan and the role they fill out."@en ;
    rdfs:domain 	prov:Plan ;
    rdfs:label 		"plan responsibility"@en ;
    rdfs:range  	acp:PlanResponsibility .
     
acp:involved
    a owl:ObjectProperty ;
    rdfs:subPropertyOf dataid:associatedAgent ;
    rdfs:isDefinedBy <http://dataid.dbpedia.org/ns/acp#> ;
    rdfs:comment 	"Points out agents somehow involved in a Plan."@en ;
    rdfs:label 		"involved"@en ;
    owl:propertyChainAxiom (
	   acp:planResponsibility
	   dataid:authorizedAgent
	) .
 	
acp:involvedIn
    a owl:ObjectProperty ;
    owl:inverseOf acp:involved ;
    rdfs:isDefinedBy <http://dataid.dbpedia.org/ns/acp#> ;
    rdfs:comment 	"Attributes a plan in which an agent was somehow involved in."@en ;
    rdfs:label 		"involved in"@en .
    
acp:associatedWith
    a owl:ObjectProperty ;
    rdfs:subPropertyOf prov:qualifiedAssociation ;
    rdfs:isDefinedBy <http://dataid.dbpedia.org/ns/acp#> ;
    rdfs:comment 	"Qualifies the prov:wasAssociatedWith property by pointing out the related Association."@en ;
    rdfs:domain 	prov:Activity ;
    rdfs:label 		"associated with"@en ;
    rdfs:range  	acp:ActivityAssociation .
   
acp:isPartOfAction
    a owl:ObjectProperty ;
    rdfs:subPropertyOf dct:isPartOf ;
    rdfs:isDefinedBy <http://dataid.dbpedia.org/ns/acp#> ;
    rdfs:comment 	"Associates an activity to an dataid:AuthorizedAction, thereby further defining the AuthorizedAction."@en ;
    rdfs:domain 	prov:Activity ;
    rdfs:label 		"is part of action"@en ;
    rdfs:range  	dataid:AuthorizedAction .
   
acp:deputyAgent
    a owl:ObjectProperty ;
    rdfs:subPropertyOf dataid:AuthorizedAgent ;
    rdfs:isDefinedBy <http://dataid.dbpedia.org/ns/acp#> ;
    rdfs:comment 	"Adds a substitute (deputy) agent to a responsibility, which steps in if the primary agent leaves the project or is otherwise absent."@en ;
    rdfs:domain 	acp:PlanResponsibility ;
    rdfs:label 		"deputy agent"@en ;
    rdfs:range  	dataid:Agent .
   
acp:inception
    a owl:DatatypeProperty ;
    rdfs:isDefinedBy <http://dataid.dbpedia.org/ns/acp#> ;
    rdfs:comment 	"States the (intended) starting date of the implementation of a plan."@en ;
    rdfs:domain 	prov:Plan ;
    rdfs:label 		"inception"@en ;
    rdfs:range  	xsd:datetime .
   
acp:conclusion
    a owl:DatatypeProperty ;
    rdfs:isDefinedBy <http://dataid.dbpedia.org/ns/acp#> ;
    rdfs:comment 	"States the (intended) date of the conclusion of a plan."@en ;
    rdfs:domain 	prov:Plan ;
    rdfs:label 		"conclusion"@en ;
    rdfs:range  	xsd:datetime .