@prefix rdf: <http://www.w3.org/1999/02/22-rdf-syntax-ns#> .
@prefix dataid: <http://dataid.dbpedia.org/ns/core#> .
@prefix dataid-acp: <http://dataid.dbpedia.org/ns/acp#> .
@prefix dmp: <http://dataid.dbpedia.org/ns/dmp#> .
@prefix dcat: <http://www.w3.org/ns/dcat#> .
@prefix dct: <http://purl.org/dc/terms/> .
@prefix odrl: <http://www.w3.org/ns/odrl/2/> .
@prefix owl: <http://www.w3.org/2002/07/owl#> .
@prefix prov: <http://www.w3.org/ns/prov#> .
@prefix rdfs: <http://www.w3.org/2000/01/rdf-schema#> .
@prefix void: <http://rdfs.org/ns/void#> .
@prefix xml: <http://www.w3.org/XML/1998/namespace> .
@prefix xsd: <http://www.w3.org/2001/XMLSchema#> .
@prefix foaf: <http://xmlns.com/foaf/0.1/> . 
@prefix vann: <http://purl.org/vocab/vann/> .
@prefix dlo: <http://aligned-project.eu/ontologies/dlo#> .
@prefix org: <http://www.w3.org/ns/org#> .
@prefix r3d: <http://www.re3data.org/schema/3-0#> .
@prefix obeu: <http://data.openbudgets.eu/ontology/> .

dmp:
    a owl:Ontology ;
    vann:preferredNamespaceUri "http://dataid.dbpedia.org/ns/dmp#" ;
    vann:preferredNamespacePrefix "dataid-dmp"^^xsd:string ;
    owl:versionInfo "1.0.0" ; 
    rdfs:comment "This mid-level extension to DataID provides detaild provenance information about (planned) activities related to datasets described by a DataID."@en ;
    rdfs:label "DataID"@en ;
    owl:imports dataid:, dataid-acp:, prov:, dlo:, org: .
    
############# classes ################
dmp:DataManagementPlan 
	a owl:Class ;
	rdfs:subClassOf prov:Plan ;
    rdfs:isDefinedBy <http://dataid.dbpedia.org/ns/dmp#> ;
    rdfs:label "data management plan"@en ;
    rdfs:comment """Top level plan for data managemant purposes. Is related to (research) project and presents aggregated values of BudgetItems."""@en . 
    
dmp:PreservationPlan
	a owl:Class ;
	rdfs:subClassOf prov:Plan ;
    rdfs:isDefinedBy <http://dataid.dbpedia.org/ns/dmp#> ;
    rdfs:label "preservation plan"@en ;
    rdfs:comment """This plan describes the preservation provisions made for one or more datasets. It points out one or more repositories the described dataset is stored at and defines a time interval for which the preservation plan has to be complied with."""@en .
    
dmp:Repository
	a owl:Class ;
	rdfs:subClassOf prov:Entity, r3d:Repository, dlo:Repository ;
    rdfs:isDefinedBy <http://dataid.dbpedia.org/ns/dmp#> ;
    rdfs:label "repository"@en ;
    rdfs:comment """The repository is used for describing the conditions of storage of datasets under the custody of an institution. Most properties are imported from the re3data.org schema."""@en .
    
dmp:PlanBudgetItem
	a owl:Class ;
	rdfs:subClassOf prov:Plan ;
    rdfs:isDefinedBy <http://dataid.dbpedia.org/ns/dmp#> ;
    rdfs:label "preservation plan"@en ;
    rdfs:comment """States the costs involved for the execution of a plan in regard to an Activity, Entity or Responsibility when involved in that plan."""@en .
    
############# properties ################
dmp:proposedDmp
    a owl:ObjectProperty ;
    rdfs:isDefinedBy <http://dataid.dbpedia.org/ns/dmp#> ;
    rdfs:comment 	"Points out a Data Management Plan entity related to the DataID."@en ;
    rdfs:domain 	dataid:DataId ;
    rdfs:label 		"proposed data management plan"@en ;
    rdfs:range  	dmp:DataManagementPlan .
    
dmp:projectIdentifier
    a owl:ObjectProperty ;
    rdfs:subPropertyOf dct:identifier ;
    rdfs:isDefinedBy <http://dataid.dbpedia.org/ns/dmp#> ;
    rdfs:comment 	"Identifies the (research-) project the DMP is pertaining to."@en ;
    rdfs:domain 	dmp:DataManagementPlan ;
    rdfs:label 		"project identifier"@en ;
    rdfs:range  	dataid:Identifier .
    
dmp:projectName
    a owl:DatatypeProperty ;
    rdfs:isDefinedBy <http://dataid.dbpedia.org/ns/dmp#> ;
    rdfs:comment 	"Provides the name of the project the DMP is pertaining to."@en ;
    rdfs:domain 	dmp:DataManagementPlan ;
    rdfs:label 		"project name"@en ;
    rdfs:range  	rdfs:Literal .
    
dmp:approxCost
    a owl:DatatypeProperty ;
    rdfs:isDefinedBy <http://dataid.dbpedia.org/ns/dmp#> ;
    rdfs:comment 	"Should in general aggregate all BudgetItems of this and all sub-plans."@en ;
    rdfs:domain 	dmp:DataManagementPlan ;
    rdfs:label 		"approximated costs"@en ;
    rdfs:range  	xsd:decimal .
        
dmp:justification
    a owl:ObjectProperty ;
    rdfs:isDefinedBy <http://dataid.dbpedia.org/ns/dmp#> ;
    rdfs:comment 	"Free text (and reference link) stating why this plan has been adopted."@en ;
    rdfs:domain 	prov:Plan ;
    rdfs:label 		"justification"@en ;
    rdfs:range  	dataid:SimpleStatement .
    
dmp:preservationPlan
    a owl:ObjectProperty ;
    rdfs:subPropertyOf dataid-acp:hasSubPlan ;
    rdfs:isDefinedBy <http://dataid.dbpedia.org/ns/dmp#> ;
    rdfs:comment 	"A Data Management Plan might have multiple preservation plans (e.g. one for each dataset)."@en ;
    rdfs:domain 	dmp:DataManagementPlan ;
    rdfs:label 		"preservation plan"@en ;
    rdfs:range  	dmp:PreservationPlan .
    
dmp:preservation
    a owl:ObjectProperty ;
    rdfs:isDefinedBy <http://dataid.dbpedia.org/ns/dmp#> ;
    rdfs:comment 	"A Dataset has usually one preservation plan pointed out via this property."@en ;
    rdfs:domain 	dataid:Dataset ;
    rdfs:label 		"preservation"@en ;
    rdfs:range  	dmp:PreservationPlan .
    
dmp:budgetItem
    a owl:ObjectProperty ;
    rdfs:isDefinedBy <http://dataid.dbpedia.org/ns/dmp#> ;
    rdfs:comment 	"Points out a cost centre in a plan. "@en ;
    rdfs:domain 	prov:Plan ;
    rdfs:label 		"budget item"@en ;
    rdfs:range  	dmp:PlanBudgetItem .
        
dmp:budgetPlan
    a owl:ObjectProperty ;
    owl:inverseOf dmp:budgetItem ;
    rdfs:isDefinedBy <http://dataid.dbpedia.org/ns/dmp#> ;
    rdfs:comment 	"Points out the plan a budget item is attributed to. "@en ;
    rdfs:label 		"budget plan"@en .
    
    
dmp:item
    a owl:ObjectProperty ;
    rdfs:isDefinedBy <http://dataid.dbpedia.org/ns/dmp#> ;
    rdfs:comment 	"Points out an Entity, Activity or Responsibility responsible for a BudgetItem. "@en ;
    rdfs:domain 	dmp:PlanBudgetItem ;
    rdfs:label 		"item"@en .
    
dmp:isCoveredBy
    a owl:ObjectProperty ;
    rdfs:isDefinedBy <http://dataid.dbpedia.org/ns/dmp#> ;
    rdfs:comment 	"The expected monetary source out of which the BudgetItem is covered in a plan."@en ;
    rdfs:domain 	dmp:PlanBudgetItem ;
    rdfs:label 		"is covered by"@en .
    
dmp:currency
    a owl:ObjectProperty ;
    rdfs:isDefinedBy <http://dataid.dbpedia.org/ns/dmp#> ;
    rdfs:comment 	"The currency used for a BudgetItem."@en ;
    rdfs:domain 	dmp:PlanBudgetItem ;
    rdfs:label 		"currency"@en ;
    rdfs:range  	obeu:Currency .
    
dmp:amount
    a owl:DatatypeProperty ;
    rdfs:isDefinedBy <http://dataid.dbpedia.org/ns/dmp#> ;
    rdfs:comment 	"The monetary amount for a BudgetItem."@en ;
    rdfs:domain 	dmp:PlanBudgetItem ;
    rdfs:label 		"amount"@en ;
    rdfs:range  	xsd:decimal .
    
dmp:isProjection
    a owl:DatatypeProperty ;
    rdfs:isDefinedBy <http://dataid.dbpedia.org/ns/dmp#> ;
    rdfs:comment 	"Points out if a BudgetItem is still a projection or has already materialized."@en ;
    rdfs:domain 	dmp:PlanBudgetItem ;
    rdfs:label 		"is projection"@en ;
    rdfs:range  	xsd:decimal .
        
dmp:contrivedBy
    a owl:ObjectProperty ;
    rdfs:subPropertyOf dataid-acp:involved ;
    rdfs:isDefinedBy <http://dataid.dbpedia.org/ns/dmp#> ;
    rdfs:comment 	"The agent(s) responsible for forging the plan."@en ;
    rdfs:domain 	prov:Plan ;
    rdfs:label 		"contrived by"@en ;
    rdfs:range  	dataid:Agent .
        
dmp:granter
    a owl:ObjectProperty ;
    rdfs:subPropertyOf dataid-acp:involved ;
    rdfs:isDefinedBy <http://dataid.dbpedia.org/ns/dmp#> ;
    rdfs:comment 	"An Agent which granted money for a project/plan."@en ;
    rdfs:domain 	prov:Plan ;
    rdfs:label 		"granter"@en ;
    rdfs:range  	dataid:Agent .
        
dmp:organisation
    a owl:ObjectProperty ;
    rdfs:subPropertyOf dataid-acp:involved ;
    rdfs:isDefinedBy <http://dataid.dbpedia.org/ns/dmp#> ;
    rdfs:comment 	"The umbrella-organisation under which a project/plan is conducted"@en ;
    rdfs:domain 	prov:Plan ;
    rdfs:label 		"organisation"@en ;
    rdfs:range  	dataid:Agent .
        
dmp:projectPi
    a owl:ObjectProperty ;
    rdfs:subPropertyOf dataid-acp:involved ;
    rdfs:isDefinedBy <http://dataid.dbpedia.org/ns/dmp#> ;
    rdfs:comment 	"The principal investigator leading a plan or project."@en ;
    rdfs:domain 	prov:Plan ;
    rdfs:label 		"project PI"@en ;
    rdfs:range  	dataid:Agent .
        
dmp:isStoredBy
    a owl:ObjectProperty ;
    owl:inverseOf	dlo:stores ;
    rdfs:isDefinedBy <http://dataid.dbpedia.org/ns/dmp#> ;
    rdfs:comment 	"Points out the Repository storing this Distribution of a dataset."@en ;
    rdfs:domain 	dataid:Distribution ;
    rdfs:label 		"is stored by"@en ;
    rdfs:range  	dmp:Repository .
