@prefix rdf: <http://www.w3.org/1999/02/22-rdf-syntax-ns#> .
@prefix dataid: <http://dataid.dbpedia.org/ns/core#> .
@prefix dcat: <http://www.w3.org/ns/dcat#> .
@prefix dct: <http://purl.org/dc/terms/> .
@prefix odrl: <http://www.w3.org/ns/odrl/2/> .
@prefix owl: <http://www.w3.org/2002/07/owl#> .
@prefix prov: <http://www.w3.org/ns/prov#> .
@prefix rdfs: <http://www.w3.org/2000/01/rdf-schema#> .
@prefix void: <http://rdfs.org/ns/void#> .
@prefix xml: <http://www.w3.org/XML/1998/namespace> .
@prefix xsd: <http://www.w3.org/2001/XMLSchema#> .
@prefix foaf: <http://xmlns.com/foaf/0.1/> . 
@prefix lvont: <http://lexvo.org/ontology#> .
@prefix vann: <http://purl.org/vocab/vann/> .
@prefix r3d: <http://www.re3data.org/schema/2-2/> .
@prefix dataid-ps: <http://dataid.dbpedia.org/ns/ps#> .

#first draft version

<http://dataid.dbpedia.org/ns/ld#>
    a owl:Ontology ;
    vann:preferredNamespaceUri <http://dataid.dbpedia.org/ns/ps#> ;
    vann:preferredNamespacePrefix "dataid"^^xsd:string ;
    rdfs:isDefinedBy <http://dataid.dbpedia.org/ns/ps#> ;
    owl:versionInfo "0.0.1" ; 
    rdfs:comment "This is the Preservation extension for the DataID ontology <http://dataid.dbpedia.org/ns/core#>, describing provisions made for the purpose of long time preservation of data, including detailed descriptions of repositories."@en ;
    rdfs:label "DataID - Preservation"@en ;
    owl:imports <http://dataid.dbpedia.org/ns/core#> .

dataid-ps:PreservationPlan
	o owl:Class;
	rdfs:isDefinedBy <http://dataid.dbpedia.org/ns/ps#> ;
    rdfs:comment "This class describes the different provisions made to ensure a long time preservation of a connected dataset or the whole data of a DataID (dataid-ps:preservation)."@en ;
    rdfs:label "Preservation Plan"@en ;
    rdfs:range dataid-ps:PreservationPlan;
    rdfs:domain [ a owl:Class;
    	owl:unionOf (dataid:Dataid, dataid:Dataset)];
	rdfs:subClassOf [ 
			a owl:Restriction;

		].

dataid-ps:PreservationPlan
	o owl:Class;
	rdfs:isDefinedBy <http://dataid.dbpedia.org/ns/ps#> ;
    rdfs:comment "This class describes the different provisions made to ensure a long time preservation of a connected dataset or the whole data of a DataID (dataid-ps:preservation)."@en ;
    rdfs:label "Preservation Plan"@en ;
	rdfs:subClassOf [ 
	        a owl:Restriction ;
	        owl:cardinality "1"^^xsd:nonNegativeInteger ;
	        owl:onProperty dct:description
		].

dataid-ps:preservation
	a owl:ObjectProperty;
	rdfs:isDefinedBy <http://dataid.dbpedia.org/ns/ps#> ;
    rdfs:comment "Connects a Dataset or DataID to a preservation plan describing how to preserve the data described."@en ;
    rdfs:label "preservation"@en ;
    rdfs:range dataid-ps:PreservationPlan;
    rdfs:domain [ a owl:Class;
    	owl:unionOf (dataid:Dataid, dataid:Dataset)].

dataid-ps:Repository
	o owl:Class;
	rdfs:isDefinedBy <http://dataid.dbpedia.org/ns/ps#> ;
    rdfs:comment ""@en ;
    rdfs:label "Repository"@en ;
	rdfs:subClassOf r3d:Repository, [ 
	        a owl:Restriction ;
	        owl:cardinality "1"^^xsd:nonNegativeInteger ;
	        owl:onProperty dct:description
		].

dataid-ps:repository
	a owl:ObjectProperty;
	rdfs:isDefinedBy <http://dataid.dbpedia.org/ns/ps#> ;
    rdfs:comment "Points out a repository used by a preservation plan to store data."@en ;
    rdfs:label "repository"@en ;
    rdfs:range dataid-ps:Repository;
    rdfs:domain dataid-ps:PreservationPlan.

dataid-ps:archives
	a owl:ObjectProperty;
	rdfs:isDefinedBy <http://dataid.dbpedia.org/ns/ps#> ;
    rdfs:comment "Points out a dcat:Catalog stored within a Repository."@en ;
    rdfs:label "archives"@en ;
    rdfs:range dcat:Catalog;
    rdfs:domain dataid-ps:Repository.

dataid-ps:begins
	a owl:DatatypeProperty;
	rdfs:isDefinedBy <http://dataid.dbpedia.org/ns/ps#> ;
    rdfs:comment "The date on which a preservation plan takes effect."@en ;
    rdfs:label "begins"@en ;
    rdfs:range xsd:date;
    rdfs:domain dataid-ps:PreservationPlan.

dataid-ps:ends
	a owl:DatatypeProperty;
	rdfs:isDefinedBy <http://dataid.dbpedia.org/ns/ps#> ;
    rdfs:comment "The date until a preservation plan has to be adhered to."@en ;
    rdfs:label "ends"@en ;
    rdfs:range xsd:date;
    rdfs:domain dataid-ps:PreservationPlan.