@prefix dataid: <http://dataid.dbpedia.org/ns/core#> .
@prefix dcat: <http://www.w3.org/ns/dcat#> .
@prefix prov: <http://www.w3.org/ns/prov#> .
@prefix void: <http://rdfs.org/ns/void#> .
@prefix rdf: <http://www.w3.org/1999/02/22-rdf-syntax-ns#> .
@prefix rdfs: <http://www.w3.org/2000/01/rdf-schema#> .
@prefix owl: <http://www.w3.org/2002/07/owl#> .
@prefix xml: <http://www.w3.org/XML/1998/namespace> .
@prefix xsd: <http://www.w3.org/2001/XMLSchema#> .
@prefix dct: <http://purl.org/dc/terms/> .
@prefix foaf: <http://xmlns.com/foaf/0.1/> . 
@prefix skos: <http://www.w3.org/2004/02/skos/core#> .
@prefix lvont: <http://lexvo.org/ontology#> .
@prefix vann: <http://purl.org/vocab/vann/> .
@prefix odrl: <http://www.w3.org/ns/odrl/2/> .
@prefix spdx: <http://spdx.org/rdf/terms/#> .
@prefix datacite: <http://purl.org/spar/datacite/> .
@prefix litre: <http://www.essepuntato.it/2010/06/literalreification/> .

@base <http://dataid.dbpedia.org/ns/core#> .

dataid:
    a owl:Ontology ;
    vann:preferredNamespaceUri "http://dataid.dbpedia.org/ns/core#" ;
    vann:preferredNamespacePrefix "dataid" ;
    owl:versionInfo "2.0.0" ; 
    dct:modified "2016-07-21" ;
    rdfs:comment """The DataID core ontology is the central part of the DataID multi-layered metadata system. 
Its goal is to extensively describes datasets and their different manifestations in a uniform way, 
as well as relations to agents like persons or organisations, in regard to their rights and responsibilities. 
Established vocabularies like DCAT, VoID, Prov-O are used for maximum compatibility.
We introduced a multilayer concept of supporting ontologies extending DataID core to fit different 
use case scenarios (for Linked Data, providing statistical data about datasets etc.).
By describing datasets including content, authors, licenses and provenance via RDF, thereby making data 
accessible to others, is the basic idea of Linked Open Data and is your contribution to a 
universal data give and take. You can create your own DataID files for any type of data at http://dataid.dbpedia.org.
Validating and delivering metadata files in a uniform way, as well as providing the ability to query for datasets, 
are main objectives of the DBpedia/DataID project."""@en ;
    rdfs:label "DataID"@en ;
    foaf:depiction 	<https://raw.githubusercontent.com/dbpedia/DataId-Ontology/master/DataIdOntology.png> ;
	dct:license <http://purl.org/NET/rdflicense/cc-by4.0> ;
	dct:creator <http://wiki.dbpedia.org/Association/Persons/Freudenberg> ;
    owl:imports dcat:, prov:, void: .
    #owl:imports <http://www.w3.org/ns/dcat>, rdfs: , <http://www.w3.org/ns/prov-o-20130430> , foaf: ,void: , dct: .
    
<http://wiki.dbpedia.org/Association/Persons/Freudenberg>
    a                        dataid:Agent ;
    foaf:mbox                "freudenberg@informatik.uni-leipzig.de" ;
    foaf:homepage			<http://wiki.dbpedia.org/Association/Persons/Freudenberg> ;
    foaf:name                "Markus Freudenberg" .
    
########### classes ##########
    
dataid:DataId
	a owl:Class ;
    rdfs:isDefinedBy <http://dataid.dbpedia.org/ns/core#> ;
    rdfs:label "DataId"@en ;
	rdfs:comment "A DataId Induvidual serves as a root Entity for every DataID document describing one or more datasets. As a subclass of dcat:CatalogRecord / void:DatasetDescription it describes not a dataset itself but provides metadata about its entry in a dcat:Catalog and/or its relations to repositories or other data collections ."@en ;
	rdfs:subClassOf void:DatasetDescription, dcat:CatalogRecord, prov:Entity,
		[
	        a owl:Restriction ;
	        owl:allValuesFrom dataid:Dataset ;
	        owl:onProperty foaf:primaryTopic
	    ],[
	        a owl:Restriction ;
	        owl:allValuesFrom dataid:DataId ;
	        owl:onProperty dataid:nextVersion
	    ],[
	        a owl:Restriction ;
	        owl:allValuesFrom dataid:DataId ;
	        owl:onProperty dataid:previousVersion
	    ],[
	        a owl:Restriction ;
	        owl:allValuesFrom dataid:DataId ;
	        owl:onProperty dataid:latestVersion
	    ],[
	        a owl:Restriction ;
	        owl:allValuesFrom odrl:Policy;
	        owl:onProperty dct:license
	    ],[
	        a owl:Restriction ;
	        owl:allValuesFrom lvont:Language ;
	        owl:onProperty dct:language
	    ].	    

dataid:Dataset
    a owl:Class ;
    rdfs:isDefinedBy <http://dataid.dbpedia.org/ns/core#> ;
    rdfs:label "Dataset"@en ;
    rdfs:comment """A collection of data, available for access in one or more formats. Dataset resources describe the 
    concept of the dataset, not it's manifestation (the data itself), which can be acquired as a dataid:Distribution.
    Datasets are prov:Entities and can be generated by prov:Activities."""@en ;
    rdfs:subClassOf void:Dataset, dcat:Dataset, prov:Entity,
    	[
	        a owl:Restriction ;
	        owl:allValuesFrom dataid:DataId ;
	        owl:onProperty foaf:isPrimaryTopicOf
	    ],[
	        a owl:Restriction ;
	        owl:allValuesFrom dataid:Dataset ;
	        owl:onProperty dataid:nextVersion
	    ],[
	        a owl:Restriction ;
	        owl:allValuesFrom dataid:Dataset ;
	        owl:onProperty dataid:previousVersion
	    ],[
	        a owl:Restriction ;
	        owl:allValuesFrom dataid:Dataset ;
	        owl:onProperty dataid:latestVersion
	    ],[
	        a owl:Restriction ;
	        owl:allValuesFrom odrl:Policy ;
	        owl:onProperty dct:license
	    ],[
	        a owl:Restriction ;
	        owl:allValuesFrom lvont:Language ;
	        owl:onProperty dct:language
	    ],[ 
			a owl:Restriction ;
			owl:onProperty dct:isPartOf ;
		 	owl:allValuesFrom dataid:Dataset
	 	],[ 
			a owl:Restriction ;
			owl:onProperty void:subset ;
		 	owl:allValuesFrom dataid:Dataset
	 	],[
	        a owl:Restriction ;
	        owl:onProperty dcat:distribution ;
	        owl:allValuesFrom dataid:Distribution 
	    ],[
	        a owl:Restriction ;
	        owl:allValuesFrom <http://www.w3.org/2006/time#Interval> ;
	        owl:onProperty dct:temporal
	    ],[
	        a owl:Restriction ;
	        owl:allValuesFrom <http://www.geonames.org/ontology#Feature> ;
	        owl:onProperty dct:spatial
	    ].

dataid:Distribution
    a owl:Class ;
    rdfs:isDefinedBy <http://dataid.dbpedia.org/ns/core#> ;
    rdfs:comment "Distributions describe a single manifestation of the pertaining Dataset (for example; its data format/serialization or a service endpoint including the procedure required to acces the data)."@en ;
    rdfs:label "Distribution"@en ;
    rdfs:subClassOf dcat:Distribution, prov:Entity,
    	[
	        a owl:Restriction ;
	        owl:allValuesFrom dataid:Distribution ;
	        owl:onProperty dataid:nextVersion
	    ],[
	        a owl:Restriction ;
	        owl:allValuesFrom dataid:Distribution ;
	        owl:onProperty dataid:previousVersion
	    ],[
	        a owl:Restriction ;
	        owl:allValuesFrom dataid:Distribution ;
	        owl:onProperty dataid:latestVersion
	    ],[
	        a owl:Restriction ;
	        owl:allValuesFrom odrl:Policy ;
	        owl:onProperty dct:license
	    ],[
	        a owl:Restriction ;
	        owl:allValuesFrom lvont:Language ;
	        owl:onProperty dct:language
	    ].

dataid:ServiceEndpoint
    a owl:Class ;
    rdfs:isDefinedBy <http://dataid.dbpedia.org/ns/core#> ;
    rdfs:comment "A specific distribution, which is accessible via an access url and provides data as a web service in a certain format."@en ;
    rdfs:label "Service Endpoint"@en ;
    rdfs:subClassOf dataid:Distribution. 

dataid:SingleFile
    a owl:Class ;
    rdfs:isDefinedBy <http://dataid.dbpedia.org/ns/core#> ;
    rdfs:comment "A single data dump file representing the whole dataset, in a certain format/serialization."@en ;
    rdfs:label "Single File"@en ;
    rdfs:subClassOf dataid:Distribution.

dataid:Directory
    a owl:Class ;
    rdfs:isDefinedBy <http://dataid.dbpedia.org/ns/core#> ;
    rdfs:comment "A dedicated directory holding (multiple) files of the same dataset, which, when put together, make up the whole dataset."@en ;
    rdfs:label "Directory"@en ;
    rdfs:subClassOf dataid:Distribution.

dataid:FileCollection
    a owl:Class ;
    rdfs:isDefinedBy <http://dataid.dbpedia.org/ns/core#> ;
    rdfs:comment "Multiple files constituting one (complete) dataset (files in different locations are possible)."@en ;
    rdfs:label "File Collection"@en ;
    rdfs:subClassOf dataid:Distribution.
    
dataid:Agent
    a owl:Class ;
    rdfs:isDefinedBy <http://dataid.dbpedia.org/ns/core#> ;
    rdfs:comment "Agents are general entities representing persons, legal persons or organisations."@en ;
    rdfs:label "Agent"@en ;
    rdfs:subClassOf prov:Agent, foaf:Agent, dct:Agent.

dataid:Authorization
	a owl:Class ;
    rdfs:isDefinedBy <http://dataid.dbpedia.org/ns/core#> ;
    rdfs:label "Authorization"@en ;
	rdfs:comment """This concept is a mediator between a set of entities (or scope) defines by the property dataid:authorizedFor,
	a set of AgentRoles defining rights and responsibilities and Agents, fulfilling the AgentRoles, in regard to the collection of entities.
	This subclass of prov:Attribution qualifies the relation prov:wasAttributedTo between prov:Entity and prov:Agent with the AgentRoles 
	and AuthorizedActions of the DataID-domain."""@en ;
	rdfs:subClassOf prov:Attribution .

dataid:AgentRole
	a owl:Class ;
    rdfs:isDefinedBy <http://dataid.dbpedia.org/ns/core#> ;
    rdfs:label "Agent Role"@en ;
	rdfs:comment """Agent roles are defined by a set of rights and responsibilities (see AuthorizedAction) an agent, assigned with this role, has to address or can execute."""@en ;
	rdfs:subClassOf prov:Role, skos:Concept .

dataid:AuthorizedAction
	a owl:Class ;
	rdfs:subClassOf skos:Concept ;
    rdfs:isDefinedBy <http://dataid.dbpedia.org/ns/core#> ;
    rdfs:label "Authorized Action"@en ;
    rdfs:comment """Authorized actions may constiute either of activities an Agent can execute in regard to a collection of prov:Entities or of 
    responsibilities an Agent should act upon (e.g. make certain decisions if necessary or act upon certain events)."""@en .

dataid:ResponsibleAction
	a owl:Class ;
    rdfs:isDefinedBy <http://dataid.dbpedia.org/ns/core#> ;
    rdfs:label "Responsible Action"@en ;
	rdfs:comment """AgentRoles provide rights as well as responsibilities an agent has to attend to in order to fulfill this role. 
	Responsible actions should describe actions pertaining to responsibilities an agent is supposed to do when holding a specific AgentRole."""@en ;
	rdfs:subClassOf dataid:AuthorizedAction ;
	owl:disjointWith dataid:EntitledAction .

dataid:EntitledAction
	a owl:Class ;
    rdfs:isDefinedBy <http://dataid.dbpedia.org/ns/core#> ;
    rdfs:label "Entitled Action"@en ;
	rdfs:comment """EntitledActions describe actions an Agent is allowed to perform when holding a certain AgentRole. 
	These actions may address restricted matters like access, modification rights and others."""@en ;
	rdfs:subClassOf dataid:AuthorizedAction ;
	owl:disjointWith dataid:ResponsibleAction .
	
dataid:SimpleStatement
	a owl:Class;
	rdfs:isDefinedBy <http://dataid.dbpedia.org/ns/core#> ;
	rdfs:label "Simple Statement"@en ;
	rdfs:comment """A SimpleStatement either a primitive literal containing unstructured text (see dataid:statement), or a web reference to a statment (using dct:references).
	This class implements several classes of Dublin Core which are not further specified within DC."""@en ;
	rdfs:subClassOf dct:ProvenanceStatement, dct:RightsStatement, dct:Standard , litre:Literal, 
	[
        a owl:Restriction ;
        owl:allValuesFrom foaf:Document ;
        owl:onProperty dct:references
    ].

dataid:Identifier
	a owl:Class ;
	rdfs:isDefinedBy <http://dataid.dbpedia.org/ns/core#> ;
	rdfs:label "Identifier"@en ;
	rdfs:comment """Uniquely identifies any resource, given an identifier as literal (see dataid:statement) and a corresponding aid/pid scheme 
(ORCID, ResearcherID etc. pointed out via datacite:usesIdentifierScheme). Optionally it can point out a reference document on the web (about this identifier) using dct:references."""@en ;
	rdfs:subClassOf datacite:Identifier,
	[
        a owl:Restriction ;
        owl:allValuesFrom foaf:Document ;
        owl:onProperty dct:references
    ].
	    
dataid:MediaType
	a owl:Class;
	rdfs:isDefinedBy <http://dataid.dbpedia.org/ns/core#> ;
	rdfs:label "Media Type"@en ;
	rdfs:comment """Extends the dct:MediaType class of Dublin Core, providing the Iana media type description (or mime type) and common file extensions used. 
A pointer to an inner media types can describe (multiple) layers of compressions and all internal media types."""@en ;
	rdfs:subClassOf dct:MediaType.
		
########## properties #########
		
dataid:accessProcedure
	a owl:ObjectProperty ;
	rdfs:isDefinedBy <http://dataid.dbpedia.org/ns/core#> ;
	rdfs:comment "Describes the steps which have to be taken to gain access to the described data at the location of a Distribution (e.g. register an account to gain dct:accessRights)."@en ;
    rdfs:domain dataid:Distribution ;
    rdfs:label "access procedure"@en ;
    rdfs:range dataid:SimpleStatement .

dataid:isDistributionOf
	a	owl:ObjectProperty ;
	rdfs:isDefinedBy <http://dataid.dbpedia.org/ns/core#> ;
	rdfs:label "is distribution of"@en ;
	rdfs:comment "Inverse property of dcat:distribution, linking a Distribution to a Dataset"@en ;
	owl:inverseOf	dcat:distribution;
	rdfs:domain		dataid:Distribution;
	rdfs:range		dataid:Dataset.

dataid:inCatalog
	a	owl:ObjectProperty ;
	rdfs:isDefinedBy <http://dataid.dbpedia.org/ns/core#> ;
	rdfs:label "in catalog"@en ;
	rdfs:comment "The inverse property of dcat:record, pointing back to the dcat:Catalog."@en ;
	owl:inverseOf	dcat:record;
	rdfs:domain		dataid:DataId;
	rdfs:range		dcat:Catalog.
	
dataid:uncompressedByteSize
	a	owl:DatatypeProperty ;
	rdfs:subPropertyOf dcat:byteSize ;
	rdfs:isDefinedBy <http://dataid.dbpedia.org/ns/core#> ;
	rdfs:label "uncompressed byte size"@en ;
	rdfs:comment "Records the byte size of the uncompressed content of an archive file."@en ;
	rdfs:domain		dataid:Distribution ;
    rdfs:range      xsd:integer.

dataid:similarDataset
    a owl:ObjectProperty ;
    rdfs:subPropertyOf dct:relation ;
    rdfs:isDefinedBy <http://dataid.dbpedia.org/ns/core#> ;
    rdfs:comment 	"Points to other dataset containing related data."@en ;
    rdfs:domain 	dataid:Dataset ;
    rdfs:label 		"similar dataset"@en ;
    rdfs:range  	dcat:Dataset .

dataid:preview
    a owl:ObjectProperty ;
    rdfs:isDefinedBy <http://dataid.dbpedia.org/ns/core#> ;
    rdfs:comment 	"Provides the url of a short preview of the data provided by a distribution, helpful when conveying type and format of the data provided."@en ;
    rdfs:domain 	dataid:Distribution ;
    rdfs:label 		"preview"@en ;
    rdfs:range  	foaf:Document .
    
dataid:associatedAgent
    a owl:ObjectProperty ;
    rdfs:subPropertyOf prov:wasAttributedTo ;
    rdfs:isDefinedBy <http://dataid.dbpedia.org/ns/core#> ;
    rdfs:comment "An agent which is generally connected to the dataset, their exact function in regard to the Entity has to be specified by the qualification dataid:Authorization."@en ;
    rdfs:domain prov:Entity ;
    rdfs:label "associated agent"@en ;
    rdfs:range dataid:Agent ;
    owl:propertyChainAxiom (
	   dataid:underAuthorization
	   dataid:authorizedAgent
	) .

dataid:softwareRquirement
    a owl:ObjectProperty ;
    rdfs:isDefinedBy <http://dataid.dbpedia.org/ns/core#> ;
    rdfs:comment "Software needed to access the data provided via this Distribution or otherwise relevant for consuming the data."@en ;
    rdfs:domain dataid:Distribution ;
    rdfs:label "software requirement"@en ;
    rdfs:range dataid:SimpleStatement .
    
dataid:checksum
    a owl:ObjectProperty ;
    rdfs:isDefinedBy <http://dataid.dbpedia.org/ns/core#> ;
    rdfs:comment "The Checksum value allows the contents of a file to be authenticated, since it shifts even with small changes to the file."@en ;
    rdfs:domain dataid:Distribution	;
    rdfs:label "checksum"@en ;
    rdfs:range spdx:Checksum .

dataid:nextVersion
    a owl:ObjectProperty ;
    rdfs:isDefinedBy <http://dataid.dbpedia.org/ns/core#> ;
    rdfs:comment "Next version of a DataID/Dataset/Distribution."@en ;
    rdfs:domain prov:Entity ;
    rdfs:label "next version"@en ;
    rdfs:range prov:Entity .

dataid:previousVersion
    a owl:ObjectProperty ;
    rdfs:isDefinedBy <http://dataid.dbpedia.org/ns/core#> ;
    rdfs:comment "Previous version of a DataID/Dataset/Distribution."@en ;
    rdfs:domain prov:Entity ;
    rdfs:label "previous version"@en ;
    rdfs:range prov:Entity .

dataid:latestVersion
    a owl:ObjectProperty ;
    rdfs:isDefinedBy <http://dataid.dbpedia.org/ns/core#> ;
    rdfs:comment "Latest version of a DataID/Dataset/Distribution."@en ;
    rdfs:domain prov:Entity ;
    rdfs:label "latest version"@en ;
    rdfs:range prov:Entity .

dataid:innerMediaType a owl:ObjectProperty, owl:FunctionalProperty ;
	rdfs:subPropertyOf dcat:mediaType;
	rdfs:isDefinedBy <http://dataid.dbpedia.org/ns/core#> ;
    rdfs:comment "Points out the MediaType of the (compressed) file inside another file (relevant for archive files)."@en ;
    rdfs:domain dataid:MediaType ;
    rdfs:label "inner media type"@en ;
    rdfs:range dataid:MediaType .
    
dataid:typeTemplate
	a owl:DatatypeProperty, owl:FunctionalProperty ;
	rdfs:isDefinedBy <http://dataid.dbpedia.org/ns/core#> ;
	rdfs:comment "The template (or mime type string) of a MediaType."@en ;
    rdfs:domain dataid:MediaType ;
    rdfs:label "media type template"@en ;
    rdfs:range rdfs:Literal .
    
dataid:typeReference
	a owl:ObjectProperty;
	rdfs:subPropertyOf	foaf:page ;
	rdfs:isDefinedBy <http://dataid.dbpedia.org/ns/core#> ;
	rdfs:comment "Refers to a standard document of the mime type described."@en ;
    rdfs:domain dataid:MediaType ;
    rdfs:label "media type reference"@en .
    
dataid:typeExtension
	a owl:DatatypeProperty;
	rdfs:isDefinedBy <http://dataid.dbpedia.org/ns/core#> ;
	rdfs:comment "Lists file extensions commonly used with this mime type."@en ;
    rdfs:domain dataid:MediaType ;
    rdfs:label "media type file extension"@en ;
    rdfs:range rdfs:Literal .
	    
dataid:typeName
	a owl:DatatypeProperty;
	rdfs:isDefinedBy <http://dataid.dbpedia.org/ns/core#> ;
	rdfs:comment "Names the MediaType described."@en ;
    rdfs:domain dataid:MediaType ;
    rdfs:label "media type name"@en ;
    rdfs:range rdfs:Literal .
    
dataid:statement
	a owl:DatatypeProperty ;
	rdfs:subPropertyOf litre:hasLiteralValue ;
	rdfs:isDefinedBy <http://dataid.dbpedia.org/ns/core#> ;
    rdfs:comment 	"An actual textual statement (or string)."@en ;
    rdfs:label "statement"@en ;
    rdfs:range rdfs:Literal.

dataid:identifier
    a owl:InverseFunctionalProperty ;
    rdfs:subPropertyOf datacite:hasIdentifier, foaf:isPrimaryTopicOf ;
    rdfs:isDefinedBy <http://dataid.dbpedia.org/ns/core#> ;
    rdfs:comment "An unique identifier for an Agent or Entity (for other, non DataID related identifiers)."@en ;
    rdfs:label "identifier"@en ;
    rdfs:range datacite:Identifier .

dataid:authorizedAgent
   	a owl:ObjectProperty ;
    rdfs:subPropertyOf prov:agent ;
   	rdfs:isDefinedBy <http://dataid.dbpedia.org/ns/core#> ;
    rdfs:comment "Points out an Agent which holds the rights granted by a dataid:Authorization (e.g. to modify the metadata of a Dataset)."@en ;
    rdfs:domain prov:AgentInfluence ;
    rdfs:label "authorized agent"@en ;
    rdfs:range dataid:Agent .

dataid:hasAuthorization
   	a owl:ObjectProperty ;
   	owl:inverseOf dataid:authorizedAgent ;
   	rdfs:isDefinedBy <http://dataid.dbpedia.org/ns/core#> ;
    rdfs:comment "Provides an dataid:Agent with the dataid:Authorization for a given scope of Entities (e.g. Dataset, Distribution etc.), granting rights to certain AuthorizedActions."@en ;
    rdfs:label "has authorization"@en .
    
dataid:authorityAgentRole
   	a owl:ObjectProperty ;
    rdfs:subPropertyOf prov:hadRole ;
    rdfs:isDefinedBy <http://dataid.dbpedia.org/ns/core#> ;
    rdfs:comment "Provides a role an Agent fills out in the scope provided by the dataid:Authorization, thereby allowing for certain AuthorizedActions an agent can execute."@en ;
    rdfs:domain prov:AgentInfluence ;
    rdfs:label "authority agent role"@en ;
    rdfs:range dataid:AgentRole .

dataid:allowsFor
   	a owl:ObjectProperty ;
    rdfs:isDefinedBy <http://dataid.dbpedia.org/ns/core#> ;
    rdfs:comment "An dataid:AgentRole allows an agent to execute certain AuthorizedActions."@en ;
    rdfs:domain dataid:AgentRole ;
    rdfs:label "allows for"@en ;
    rdfs:range dataid:AuthorizedAction .

dataid:authorizedAction
   	a owl:ObjectProperty ;
    rdfs:isDefinedBy <http://dataid.dbpedia.org/ns/core#> ;
    rdfs:comment "Points out AuthorizedActions, Agents are allowed to execute under a given dataid:Authorization (and its chosen AgentRoles)."@en ;
    rdfs:domain prov:AgentInfluence ;
    rdfs:label "authorized action"@en ;
    rdfs:range dataid:AuthorizedAction ;
    owl:propertyChainAxiom (
	   dataid:authorityAgentRole
	   dataid:allowsFor
	) .
	
dataid:identifierScheme
    a owl:ObjectProperty ;
    rdfs:isDefinedBy <http://dataid.dbpedia.org/ns/core#> ;
    rdfs:comment "Points out which scheme of identifiers is used to uniquely identify resources inside a Dataset."@en ;
    rdfs:label "identifier scheme"@en ;
    rdfs:domain dataid:Dataset ;
    rdfs:range datacite:IdentifierScheme .

dataid:usefulness 
	a owl:ObjectProperty ;
	rdfs:isDefinedBy <http://dataid.dbpedia.org/ns/dmp#> ;
	rdfs:label "usefulness"@en ;
	rdfs:comment "Description of to whom the data could be useful, and whether it underpins a scientific publication."@en ;
	rdfs:domain dataid:Dataset ;
	rdfs:range dataid:SimpleStatement .

dataid:similarData 
	a owl:ObjectProperty ;
	rdfs:isDefinedBy <http://dataid.dbpedia.org/ns/dmp#> ;
   	rdfs:label "similar data"@en ;
   	rdfs:comment "Information on the existence (or not) of similar data (see also dataid:similarDataset)."@en ;
   	rdfs:domain dataid:Dataset ;
   	rdfs:range dataid:SimpleStatement .

dataid:reuseAndIntegration 
	a owl:ObjectProperty ;
	rdfs:isDefinedBy <http://dataid.dbpedia.org/ns/dmp#> ;
	rdfs:label "reuse and integration"@en ;
	rdfs:comment "Information on the possibilities for integration and reuse of the dataset."@en ;
	rdfs:domain dataid:Dataset ;
	rdfs:range dataid:SimpleStatement .

dataid:growth 
	a owl:ObjectProperty ;
	rdfs:isDefinedBy <http://dataid.dbpedia.org/ns/dmp#> ;
	rdfs:label "growth"@en ;
	rdfs:comment "Indication of what size the approximated end volume of the data is."@en ;
	rdfs:domain dataid:Dataset ;
	rdfs:range dataid:SimpleStatement .

dataid:openness 
	a owl:ObjectProperty ;
	rdfs:isDefinedBy <http://dataid.dbpedia.org/ns/dmp#> ;
	rdfs:label "openness"@en ;
	rdfs:comment """General description of how data will be shared. 
	For example: embargo periods (if any), outlines of technical mechanisms for dissemination or a definition of whether access will be widely open or restricted to specific groups. 
	In case the dataset cannot be shared, the reasons for this should be mentioned (e.g. ethical, rules of personal data, intellectual property, commercial, privacy-related, security-related)."""@en ;
	rdfs:domain dataid:Dataset ;
	rdfs:range dataid:SimpleStatement .

dataid:dataDescription
	a owl:ObjectProperty ;
	rdfs:isDefinedBy <http://dataid.dbpedia.org/ns/dmp#> ;
	rdfs:label "data description"@en ;
	rdfs:comment "Provides a general description of the data represented by this dataset."@en ;
	rdfs:domain dataid:Dataset ;
	rdfs:range dataid:SimpleStatement .

dataid:validFrom
    a owl:DatatypeProperty, owl:FunctionalProperty ;
    rdfs:isDefinedBy <http://dataid.dbpedia.org/ns/core#> ;
    rdfs:comment 	"The influence an agent has over an Entity is valid from a certain point in time."@en ;
    rdfs:domain 	prov:AgentInfluence ;
    rdfs:label 		"valid from"@en ;
    rdfs:range  	xsd:datetime .
    
dataid:validUntil
    a owl:DatatypeProperty, owl:FunctionalProperty ;
    rdfs:isDefinedBy <http://dataid.dbpedia.org/ns/core#> ;
    rdfs:comment 	"The influence an agent has over an Entity is valid until a certain point in time."@en ;
    rdfs:domain 	prov:AgentInfluence ;
    rdfs:label 		"valid until"@en ;
    rdfs:range  	xsd:datetime .

dataid:isInheritable
	a	owl:DatatypeProperty, owl:FunctionalProperty ;
	rdfs:isDefinedBy <http://dataid.dbpedia.org/ns/core#> ;
	rdfs:label "is inheritable"@en ;
	rdfs:comment "Indicated whether this dataid:Authorization will be valid after an update to the DataID or a scope element (by default this property should be 'true')."@en ;
	rdfs:domain		dataid:Authorization ;
    rdfs:range      xsd:boolean.

#The follwing section defines the spread of an Authorization of multiple entities.	
dataid:authorizedFor
	a owl:ObjectProperty ;
    rdfs:isDefinedBy <http://dataid.dbpedia.org/ns/core#> ;
    rdfs:comment """Defines the scope of a dataid:Authorization. An Agent has the right to execute AuthorizedActions for all Entities of this scope. 
The property chain axioms in its subproperties define how the scope of an dataid:Authorization is spread to other Entities."""@en ;
    rdfs:label "authorized for"@en ;
    rdfs:domain dataid:Authorization ;
    rdfs:range  prov:Entity .

dataid:underAuthorization
    a owl:ObjectProperty ;
    rdfs:subPropertyOf prov:qualifiedAttribution ;
    owl:inverseOf dataid:authorizedFor ;
    rdfs:isDefinedBy <http://dataid.dbpedia.org/ns/core#> ;
    rdfs:comment "Points out a dataid:Authorization which grants some degree of authority over this resource (inverse property of dataid:authorizedFor)."@en ;
    rdfs:label "under authorization"@en ;
    rdfs:domain	prov:Entity ;
    rdfs:range dataid:Authorization .

dataid:needsSpecialAuthorization
    a owl:ObjectProperty ;
    rdfs:subPropertyOf dataid:underAuthorization ;
    rdfs:isDefinedBy <http://dataid.dbpedia.org/ns/core#> ;
    rdfs:comment "Points out a dataid:Authorization which grants some degree of authority over this resource to the exclusion of other dataid:Authorizations which are not specified with this property."@en ;
    rdfs:label "needs special authorization"@en ;
    rdfs:domain	prov:Entity ;
    rdfs:range dataid:Authorization .

#Defining void:subset as a transitive property allows for inferring dataid:authorizedFor over dataset hierarchies of multiple levels.
dataid:transitiveSubset	
	a	owl:ObjectProperty, owl:TransitiveProperty ;
	rdfs:isDefinedBy <http://dataid.dbpedia.org/ns/core#> ;
	rdfs:label "transitive super property of void:subset"@en ;
	rdfs:comment "Transitive super property of void:subset. This property is used to infer dataid:authorizedFor statements transitively over dataset hierarchies of arbitrary depth."@en .	
	
void:subset rdfs:subPropertyOf dataid:transitiveSubset.

#The follwing properties are only inferred by the the existence of property paths of foaf:primaryTopc, void:subset dcat:distribution and dataid:authorizedFor.
#They make up the super property dataid:authorizedFor and define how an Authorization is spread amongst different entities of DataID, Dataset and Distribution. 
dataid:authoritySubChain1	
	a	owl:ObjectProperty ;
	rdfs:subPropertyOf dataid:authorizedFor ;
	rdfs:isDefinedBy <http://dataid.dbpedia.org/ns/core#> ;
    rdfs:comment "This sub-property of dataid:authorizedFor provides a property chain axiom, extending the reach of dataid:authorizedFor to other entities."@en ;
    owl:propertyChainAxiom (
		dataid:authorizedFor
		foaf:primaryTopic	
		dataid:transitiveSubset
		dcat:distribution
	) .
	
dataid:authoritySubChain2	
	a	owl:ObjectProperty ;
	rdfs:subPropertyOf dataid:authorizedFor ;
	rdfs:isDefinedBy <http://dataid.dbpedia.org/ns/core#> ;
    rdfs:comment "This sub-property of dataid:authorizedFor provides a property chain axiom, extending the reach of dataid:authorizedFor to other entities."@en ;
    owl:propertyChainAxiom (
		dataid:authorizedFor
		foaf:primaryTopic	
		dcat:distribution
	) .
	
dataid:authoritySubChain3	
	a	owl:ObjectProperty ;
	rdfs:subPropertyOf dataid:authorizedFor ;
	rdfs:isDefinedBy <http://dataid.dbpedia.org/ns/core#> ;
    rdfs:comment "This sub-property of dataid:authorizedFor provides a property chain axiom, extending the reach of dataid:authorizedFor to other entities."@en ;
    owl:propertyChainAxiom (
		dataid:authorizedFor
		dataid:transitiveSubset	
		dcat:distribution
	) .
	
dataid:authoritySubChain4	
	a	owl:ObjectProperty ;
	rdfs:subPropertyOf dataid:authorizedFor ;
	rdfs:isDefinedBy <http://dataid.dbpedia.org/ns/core#> ;
    rdfs:comment "This sub-property of dataid:authorizedFor provides a property chain axiom, extending the reach of dataid:authorizedFor to other entities."@en ;
    owl:propertyChainAxiom (
		dataid:authorizedFor
		dataid:transitiveSubset	
	) .
	
dataid:authoritySubChain5	
	a	owl:ObjectProperty ;
	rdfs:subPropertyOf dataid:authorizedFor ;
	rdfs:isDefinedBy <http://dataid.dbpedia.org/ns/core#> ;
    rdfs:comment "This sub-property of dataid:authorizedFor provides a property chain axiom, extending the reach of dataid:authorizedFor to other entities."@en ;
    owl:propertyChainAxiom (
		dataid:authorizedFor
		foaf:primaryTopic	
	) .
	
dataid:authoritySubChain6	
	a	owl:ObjectProperty ;
	rdfs:subPropertyOf dataid:authorizedFor ;
	rdfs:isDefinedBy <http://dataid.dbpedia.org/ns/core#> ;
    rdfs:comment "This sub-property of dataid:authorizedFor provides a property chain axiom, extending the reach of dataid:authorizedFor to other entities."@en ;
    owl:propertyChainAxiom (
		dataid:authorizedFor
		dcat:distribution
	) .
	
dataid:authoritySubChain7	
	a	owl:ObjectProperty ;
	rdfs:subPropertyOf dataid:authorizedFor ;
	rdfs:isDefinedBy <http://dataid.dbpedia.org/ns/core#> ;
    rdfs:comment "This sub-property of dataid:authorizedFor provides a property chain axiom, extending the reach of dataid:authorizedFor to other entities."@en ;
    owl:propertyChainAxiom (
		dataid:authorizedFor
		foaf:primaryTopic	
		dataid:transitiveSubset	
	) .
	
################### Individuals ####################

## Both ConceptSchemes are just examples in how to use AgentRoles and AuthorizedActions in the context of hierarchies.
## These Schemes are used to describe responsibilities of agents in the context of DataIDs and their Datasets.
## TopConcepts contain all actions (or roles) via the relations of skos:narrowerTransitive, skos:broaderTransitive.
dataid:AuthorizedActionScheme
	a owl:NamedIndividual, skos:ConceptScheme;
	skos:hasTopConcept dataid:AllResponsibilities, dataid:AllEntitlements ;
	rdfs:label "authorized action scheme"@en;
	rdfs:comment "Description of the authorized action hierarchy."@en .
	
dataid:AllResponsibilities
	a owl:NamedIndividual, dataid:ResponsibleAction ;
	rdfs:isDefinedBy <http://dataid.dbpedia.org/ns/core#> ;
	rdfs:comment "Encompasses all responsibilities."@en ;
	skos:prefLabel "all responsibilities"@en ;
	skos:topConceptOf dataid:AuthorizedActionScheme ;
	rdfs:label "all responsibilities"@en .
	
dataid:ResponseToContact
	a owl:NamedIndividual, dataid:ResponsibleAction ;
	rdfs:isDefinedBy <http://dataid.dbpedia.org/ns/core#> ;
	rdfs:comment "The responsibility to respond to contact attempts by external agents. A contact point for the entity."@en ;
	skos:prefLabel "response to contact attempt"@en ;
	skos:inScheme dataid:AuthorizedActionScheme ;
	skos:broader dataid:AllResponsibilities ;
	rdfs:label "response to contact attempt"@en .

dataid:ResponseToLifeCycleEvent
	a owl:NamedIndividual, dataid:ResponsibleAction ;
	rdfs:isDefinedBy <http://dataid.dbpedia.org/ns/core#> ;
	rdfs:comment "The responsibility to manage changes and react to bugs and issues that are reported"@en ;
	skos:prefLabel "response to life-cycle event"@en ;
	skos:inScheme dataid:AuthorizedActionScheme ;
	skos:broader dataid:AllResponsibilities ;
	rdfs:label "response to life-cycle event"@en .

dataid:PublishingDecision
	a owl:NamedIndividual, dataid:ResponsibleAction ;
	rdfs:isDefinedBy <http://dataid.dbpedia.org/ns/core#> ;
	rdfs:comment "The responsibility decide if the entity should be published"@en ;
	skos:prefLabel "publishing decision"@en ;
	skos:inScheme dataid:AuthorizedActionScheme ;
	skos:broader dataid:AllResponsibilities ;
	rdfs:label "publishing decision"@en .

dataid:UpdateDataId
	a owl:NamedIndividual, dataid:ResponsibleAction ;
	rdfs:isDefinedBy <http://dataid.dbpedia.org/ns/core#> ;
	rdfs:comment "The responsibility to update dataset metadata."@en ;
	skos:prefLabel "update DataId"@en ;
	skos:inScheme dataid:AuthorizedActionScheme ;
	skos:broader dataid:AllResponsibilities ;
	rdfs:label "update DataId"@en .

dataid:AgentSupervision
	a owl:NamedIndividual, dataid:ResponsibleAction ;
	rdfs:isDefinedBy <http://dataid.dbpedia.org/ns/core#> ;
	rdfs:comment "The responsibility to supervise other agents."@en ;
	skos:prefLabel "agent supervision"@en ;
	skos:inScheme dataid:AuthorizedActionScheme ;
	skos:broader dataid:AllResponsibilities ;
	rdfs:label "agent supervision"@en .
	
dataid:AllEntitlements
	a owl:NamedIndividual, dataid:ResponsibleAction ;
	rdfs:isDefinedBy <http://dataid.dbpedia.org/ns/core#> ;
	rdfs:comment "Encompasses all entitlements."@en ;
	skos:prefLabel "all entitlements"@en ;
	skos:topConceptOf dataid:AuthorizedActionScheme ;
	rdfs:label "all entitlements"@en .

dataid:ReadDataId
	a owl:NamedIndividual, dataid:EntitledAction;
	rdfs:isDefinedBy <http://dataid.dbpedia.org/ns/core#> ;
	rdfs:comment "Entitled action to read the DataID dataset metadata"@en ;
	skos:prefLabel "read DataID right"@en ;
	skos:inScheme dataid:AuthorizedActionScheme ;
	skos:broader dataid:AllEntitlements ;
	rdfs:label "read DataID right"@en .

dataid:ReadContent
	a owl:NamedIndividual, dataid:EntitledAction;
	rdfs:isDefinedBy <http://dataid.dbpedia.org/ns/core#> ;
	rdfs:comment "Entitled action to read the content of an entity."@en ;
	skos:prefLabel "read content right"@en ;
	skos:inScheme dataid:AuthorizedActionScheme ;
	skos:broader dataid:ModifyContent ;
	rdfs:label "read content right"@en .

dataid:ModifyContent
	a owl:NamedIndividual, dataid:EntitledAction;
	rdfs:isDefinedBy <http://dataid.dbpedia.org/ns/core#> ;
	rdfs:comment "Entitled action to modify the content of an entity."@en ;
	skos:prefLabel "modify content right"@en ;
	skos:inScheme dataid:AuthorizedActionScheme ;
	skos:broader dataid:DeleteContent ;
	rdfs:label "modify content right"@en .

dataid:DeleteContent
	a owl:NamedIndividual, dataid:EntitledAction;
	rdfs:isDefinedBy <http://dataid.dbpedia.org/ns/core#> ;
	rdfs:comment "Entitled action to delete some content of an entity."@en ;
	skos:prefLabel "delete content right"@en ;
	skos:inScheme dataid:AuthorizedActionScheme ;
	skos:broader dataid:AllEntitlements ;
	rdfs:label "delete content right"@en .

dataid:ModifyAuthorizedAgents
	a owl:NamedIndividual, dataid:EntitledAction ;
	rdfs:comment "Entitled action to modify which agents are authorized on certain entities."@en ;
	rdfs:isDefinedBy <http://dataid.dbpedia.org/ns/core#> ;
	skos:prefLabel "modify authorized agents"@en ;
	skos:inScheme dataid:AuthorizedActionScheme ;
	skos:broader dataid:AllEntitlements ;
	rdfs:label "modify authorized agents"@en .

dataid:ModifyAuthorization
	a owl:NamedIndividual, dataid:EntitledAction ;
	rdfs:comment "Entitled action to modify an authorization."@en ;
	rdfs:isDefinedBy <http://dataid.dbpedia.org/ns/core#> ;
	skos:prefLabel "modify authorization"@en ;
	skos:inScheme dataid:AuthorizedActionScheme ;
	skos:broader dataid:AllEntitlements ;
	rdfs:label "modify authorization"@en .

dataid:ModifyAgentRoles
	a owl:NamedIndividual, dataid:EntitledAction ;
	rdfs:comment "Entitled action to modify the role of agents on certain entities."@en ;
	rdfs:isDefinedBy <http://dataid.dbpedia.org/ns/core#> ;
	skos:prefLabel "modify agent roles"@en ;
	skos:inScheme dataid:AuthorizedActionScheme ;
	skos:broader dataid:AllEntitlements ;
	rdfs:label "modify agent roles"@en .

dataid:AgentRoleScheme
	a owl:NamedIndividual, skos:ConceptScheme ;
	skos:hasTopConcept dataid:Creator ;
	rdfs:label "agent role scheme"@en;
	rdfs:comment "Description of the agent role hierarchy."@en .

dataid:Creator
	a owl:NamedIndividual, dataid:AgentRole;
	rdfs:isDefinedBy <http://dataid.dbpedia.org/ns/core#> ;
	dataid:allowsFor dataid:AllResponsibilities, dataid:AllEntitlements ;
    rdfs:comment "Creator of the resource. An agent that is credited with a main part in the initial creation of the resource."@en ;
    skos:prefLabel "creator"@en ;
	skos:topConceptOf dataid:AgentRoleScheme ;
	rdfs:label "creator"@en .

dataid:Publisher
	a owl:NamedIndividual, dataid:AgentRole;
	rdfs:isDefinedBy <http://dataid.dbpedia.org/ns/core#> ;
	dataid:allowsFor dataid:ReadDataId;
	dataid:allowsFor dataid:UpdateDataId;
	dataid:allowsFor dataid:ModifyContent;
	dataid:allowsFor dataid:DeleteContent;
	dataid:allowsFor dataid:ReadContent;
	dataid:allowsFor dataid:ModifyAuthorizedAgents;
	dataid:allowsFor dataid:ResponseToLifeCycleEvent;
	dataid:allowsFor dataid:ResponseToContact;
	dataid:allowsFor dataid:AgentSupervision;
	dataid:allowsFor dataid:PublishingDecision;
	dataid:allowsFor dataid:ModifyAuthorization;
    rdfs:comment "Publisher of the dataset. An agent that makes the dataset accessible online on a server or repository without necessarily being involved in its creation."@en ;
    skos:prefLabel "publisher"@en ;
	skos:inScheme dataid:AgentRoleScheme ;
	skos:broader dataid:Creator ;
	rdfs:label "publisher"@en .

dataid:Maintainer
	a owl:NamedIndividual, dataid:AgentRole;
	rdfs:isDefinedBy <http://dataid.dbpedia.org/ns/core#> ;
	dataid:allowsFor dataid:ReadDataId;
	dataid:allowsFor dataid:UpdateDataId;
	dataid:allowsFor dataid:ModifyContent;
	dataid:allowsFor dataid:DeleteContent;
	dataid:allowsFor dataid:ReadContent;
	dataid:allowsFor dataid:ModifyAuthorizedAgents;
	dataid:allowsFor dataid:ResponseToLifeCycleEvent;
	dataid:allowsFor dataid:ResponseToContact;
    rdfs:comment "Maintainer of the dataset. An agent that ensures the technical correctness, accessibility and up-to-dateness of a dataset."@en ;
    skos:prefLabel "maintainer"@en ;
	skos:inScheme dataid:AgentRoleScheme ;
	skos:broader dataid:Creator ;
	rdfs:label "maintainer"@en .

dataid:Contributor
	a owl:NamedIndividual, dataid:AgentRole;
	rdfs:isDefinedBy <http://dataid.dbpedia.org/ns/core#> ;
	dataid:allowsFor dataid:ReadDataId;
	dataid:allowsFor dataid:ReadContent;
	rdfs:comment "Contributor to the resource. An agent that was involved in creating or maintaining the resource but does not have the main part in this activity."@en ;
	skos:prefLabel "contributor"@en ;
	skos:inScheme dataid:AgentRoleScheme ;
	skos:broader dataid:Publisher ;
	rdfs:label "contributor"@en .

dataid:Contact
	a owl:NamedIndividual, dataid:AgentRole;
	rdfs:isDefinedBy <http://dataid.dbpedia.org/ns/core#> ;
	dataid:allowsFor dataid:ReadDataId;
	dataid:allowsFor dataid:ModifyContent;
	dataid:allowsFor dataid:ReadContent;
	dataid:allowsFor dataid:ResponseToContact;
    rdfs:comment "Contact agent. An agent that can be contacted for general requests about the resource."@en ;
    skos:prefLabel "contact"@en ;
	skos:inScheme dataid:AgentRoleScheme ;
	skos:broader dataid:Publisher, dataid:Maintainer ;
	rdfs:label "contact"@en .

dataid:Guest
	a owl:NamedIndividual, dataid:AgentRole;
	dataid:allowsFor dataid:ReadDataId;
	dataid:allowsFor dataid:ReadContent;
	rdfs:isDefinedBy <http://dataid.dbpedia.org/ns/core#> ;
    rdfs:comment "A visitor/anonymous agent has only read rights on public and semi-private documents"@en ;
    skos:prefLabel "guest"@en ;
	skos:inScheme dataid:AgentRoleScheme ;
	skos:broader dataid:Contributor ;
	rdfs:label "guest"@en .

#defining the generic Agent for any Agent not specifically defined
dataid:GuestAgent
    a owl:NamedIndividual, dataid:Agent;
    rdfs:isDefinedBy <http://dataid.dbpedia.org/ns/core#> ;
    rdfs:comment "Use this agent as a stand in for any agent not specifically defined in a domain, granting public access to an entity."@en ;
    rdfs:label "guest agent"@en ;
    foaf:mbox 		<mailto:address@alibi.com> ;
    foaf:homepage  <http://dataid.dbpedia.org>;
    foaf:name   "Guest Agent".
    
dataid:GuestAuthorization
	a owl:NamedIndividual, dataid:Authorization ;
    rdfs:isDefinedBy <http://dataid.dbpedia.org/ns/core#> ;
	dataid:isInheritable true ;
	dataid:authorizedAgent dataid:GuestAgent ;
	dataid:authorityAgentRole dataid:Guest ;
	rdfs:label "guest authority"@en ;
	rdfs:comment "This authorization can be used to point out that the content of an entity is public an can be read by anyone (see also dataid:Guest)."@en .
	
	
        
######## Single Axioms ########

## to make use of dct:spatial together with geonames#Feature:
<http://www.geonames.org/ontology#Feature>	rdfs:subClassOf	dct:Location .

## to make use of dct:temporat together with time:Interval
<http://www.w3.org/2006/time#Interval>		rdfs:subClassOf	dct:PeriodOfTime .